@prefix : <http://purl.org/holy/ns#> .
@prefix cc: <https://creativecommons.org/ns#> .
@prefix dc: <http://purl.org/dc/elements/1.1/> .
@prefix wn: <http://wordnet-rdf.princeton.edu/ontology#> .
@prefix dbc: <http://dbpedia.org/page/Category:> .
@prefix dbo: <http://dbpedia.org/ontology/> .
@prefix dbr: <http://dbpedia.org/resource/> .
@prefix dct: <http://purl.org/dc/terms/> .
@prefix ebg: <http://data.businessgraph.io/ontology#> .
@prefix m4i: <http://w3id.org/nfdi4ing/metadata4ing#> .
@prefix mod: <https://w3id.org/mod#> .
@prefix org: <http://www.w3.org/ns/org#> .
@prefix owl: <http://www.w3.org/2002/07/owl#> .
@prefix rdf: <http://www.w3.org/1999/02/22-rdf-syntax-ns#> .
@prefix rov: <http://www.w3.org/ns/regorg#> .
@prefix xml: <http://www.w3.org/XML/1998/namespace> .
@prefix xsd: <http://www.w3.org/2001/XMLSchema#> .
@prefix bibo: <http://purl.org/ontology/bibo/> .
@prefix foaf: <http://xmlns.com/foaf/0.1/> .
@prefix holy: <http://purl.org/holy/ns#> .
@prefix rdfs: <http://www.w3.org/2000/01/rdf-schema#> .
@prefix skos: <http://www.w3.org/2004/02/skos/core#> .
@prefix vann: <http://purl.org/vocab/vann/> .
@prefix schema: <http://schema.org/> .
@base <http://purl.org/holy/ns#> .

<http://purl.org/holy/ns#> rdf:type owl:Ontology ;
                            owl:versionIRI <http://purl.org/holy/ns#> ;
                            dct:created "2022"^^xsd:gYear ;
                            dct:creator [ schema:affiliation [ foaf:homepage <https://www.th-nuernberg.de> ;
                                                               foaf:name "Technische Hochschule Nürnberg Georg Simon Ohm"
                                                             ] ;
                                          foaf:homepage <https://orcid.org/0000-0001-9312-208X> ;
                                          foaf:name "Christoph Neunsinger"
                                        ] ,
                                        [ schema:affiliation [ foaf:homepage <https://www.th-nuernberg.de/einrichtungen-gesamt/fraunhofer-forschungsgruppen/future-engineering/> ;
                                                               foaf:name "Future Engineering Research Group"
                                                             ] ;
                                          rdfs:seeAlso <https://www.th-nuernberg.de/person/ascencion-arevalo-kiara-marnitt/> ;
                                          foaf:homepage <https://orcid.org/0000-0002-4158-9478> ;
                                          foaf:name "Kiara Marnitt Ascencion Arevalo"
                                        ] ;
                            dct:description "This is the Hydrogen Ontology (HOLY). HOLY is a domain ontology for describing the complex structure of hydrogen-based markets. HOLY contributes to the systemic modeling of the hydrogen domain with a focus on its value chain. Hence, it provides a foundation for retrieval, storage, and delivery of market insights.  "@en ;
                            dct:issued "2022-12-16"^^xsd:date ;
                            dct:license <https://creativecommons.org/licenses/by-sa/4.0/> ;
                            dct:publisher [ foaf:homepage <https://www.th-nuernberg.de> ;
                                            foaf:name "Technische Hochschule Nürnberg Georg Simon Ohm"
                                          ] ;
                            dct:title "Hydrogen Ontology"@en ;
                            bibo:doi <https://doi.org/10.5281/zenodo.7447958> ;
                            vann:preferredNamespacePrefix "holy" ;
                            vann:preferredNamespaceURI "http://purl.org/holy/ns#" ;
                            owl:versionInfo 1.0 ;
                            foaf:depiction <http://purl.org/holy/schema_diagram> ;
                            cc:license <https://creativecommons.org/licenses/by-sa/4.0/> ;
                            mod:acronym "HOLY" ;
                            mod:competencyQuestion <http://purl.org/holy/repository/cq> ;
                            mod:hasSyntax <http://www.w3.org/ns/formats/Turtle> .

#################################################################
#    Annotation properties
#################################################################

###  http://purl.org/dc/terms/created
dct:created rdf:type owl:AnnotationProperty .


###  http://purl.org/dc/terms/creator
dct:creator rdf:type owl:AnnotationProperty .


###  http://purl.org/dc/terms/description
dct:description rdf:type owl:AnnotationProperty .


###  http://purl.org/dc/terms/issued
dct:issued rdf:type owl:AnnotationProperty .


###  http://purl.org/dc/terms/license
dct:license rdf:type owl:AnnotationProperty .


###  http://purl.org/dc/terms/publisher
dct:publisher rdf:type owl:AnnotationProperty .


###  http://purl.org/dc/terms/references
dct:references rdf:type owl:AnnotationProperty .


###  http://purl.org/dc/terms/title
dct:title rdf:type owl:AnnotationProperty .


###  http://purl.org/ontology/bibo/doi
bibo:doi rdf:type owl:AnnotationProperty .


###  http://purl.org/vocab/vann/preferredNamespacePrefix
vann:preferredNamespacePrefix rdf:type owl:AnnotationProperty .


###  http://purl.org/vocab/vann/preferredNamespaceURI
vann:preferredNamespaceURI rdf:type owl:AnnotationProperty .


###  http://schema.org/affiliation
schema:affiliation rdf:type owl:AnnotationProperty .


###  http://wordnet-rdf.princeton.edu/ontology#hyponym
wn:hyponym rdf:type owl:AnnotationProperty .


###  http://www.w3.org/2000/01/rdf-schema#comment
rdfs:comment rdf:type owl:AnnotationProperty ;
             skos:definition "Used for listing additional information for the user."@en .


###  http://www.w3.org/2000/01/rdf-schema#label
rdfs:label rdf:type owl:AnnotationProperty ;
           skos:definition "Name of a class, object property or instance."@en .


###  http://www.w3.org/2000/01/rdf-schema#seeAlso
rdfs:seeAlso rdf:type owl:AnnotationProperty .


###  http://www.w3.org/2002/07/owl#sameAs
owl:sameAs rdf:type owl:AnnotationProperty .


###  http://www.w3.org/2002/07/owl#versionInfo
owl:versionInfo rdf:type owl:AnnotationProperty .


###  http://www.w3.org/2004/02/skos/core#altLabel
skos:altLabel rdf:type owl:AnnotationProperty .


###  http://www.w3.org/2004/02/skos/core#definition
skos:definition rdf:type owl:AnnotationProperty ;
                skos:definition "Definition of a class."@en .


###  http://www.w3.org/2004/02/skos/core#example
skos:example rdf:type owl:AnnotationProperty ;
             skos:definition "Example of an instance within a class. Used for pipeline extraction."@en .


###  http://www.w3.org/2004/02/skos/core#hiddenLabel
skos:hiddenLabel rdf:type owl:AnnotationProperty .


###  http://xmlns.com/foaf/0.1/depiction
foaf:depiction rdf:type owl:AnnotationProperty .


###  http://xmlns.com/foaf/0.1/homepage
foaf:homepage rdf:type owl:AnnotationProperty .


###  http://xmlns.com/foaf/0.1/name
foaf:name rdf:type owl:AnnotationProperty .


###  https://creativecommons.org/ns#license
cc:license rdf:type owl:AnnotationProperty .


###  https://w3id.org/mod#acronym
mod:acronym rdf:type owl:AnnotationProperty .


###  https://w3id.org/mod#competencyQuestion
mod:competencyQuestion rdf:type owl:AnnotationProperty .


###  https://w3id.org/mod#hasSyntax
mod:hasSyntax rdf:type owl:AnnotationProperty .


#################################################################
#    Datatypes
#################################################################

###  http://www.w3.org/1999/02/22-rdf-syntax-ns#PlainLiteral
rdf:PlainLiteral rdf:type rdfs:Datatype .


###  http://www.w3.org/2001/XMLSchema#date
xsd:date rdf:type rdfs:Datatype .


###  http://www.w3.org/2001/XMLSchema#gYear
xsd:gYear rdf:type rdfs:Datatype .


###  http://www.w3.org/2001/XMLSchema#string
xsd:string rdf:type rdfs:Datatype .


#################################################################
#    Object Properties
#################################################################

###  http://dbpedia.org/ontology/continent
dbo:continent rdf:type owl:ObjectProperty ,
                       owl:FunctionalProperty ,
                       owl:IrreflexiveProperty ;
              rdfs:domain schema:Country ;
              rdfs:range schema:Continent ;
              rdfs:label "continent"@en ;
              skos:definition "Links a country to the continent it belongs to."@en .


###  http://dbpedia.org/ontology/country
dbo:country rdf:type owl:ObjectProperty ,
                     owl:FunctionalProperty ,
                     owl:IrreflexiveProperty ;
            rdfs:domain holy:GeographicMarket ;
            rdfs:range schema:Country ;
            rdfs:label "country"@en ;
            skos:definition "Links a continent to a country."@en .


###  http://purl.org/dc/terms/hasPart
dct:hasPart rdf:type owl:ObjectProperty ;
            owl:inverseOf dct:isPartOf ;
            rdf:type owl:AsymmetricProperty ,
                     owl:IrreflexiveProperty ;
            dct:references dct: ;
            rdfs:comment "This property is intended to be used with non-literal values. This property is an inverse property of Is Part Of."@en ;
            rdfs:label "Has Part"@en ;
            skos:definition "A related resource that is included either physically or logically in the described resource."@en .


###  http://purl.org/dc/terms/isPartOf
dct:isPartOf rdf:type owl:ObjectProperty ,
                      owl:AsymmetricProperty ,
                      owl:IrreflexiveProperty ;
             dct:references dct: ;
             rdfs:comment "This property is intended to be used with non-literal values. This property is an inverse property of Has Part."@en ;
             rdfs:label "Is Part Of" ;
             skos:definition "A related resource in which the described resource is physically or logically included." .


###  http://purl.org/holy/ns#applicationSoldIn
holy:applicationSoldIn rdf:type owl:ObjectProperty ;
                       owl:inverseOf holy:hasApplication ;
                       rdf:type owl:AsymmetricProperty ,
                                owl:IrreflexiveProperty ;
                       rdfs:domain holy:Application ;
                       rdfs:range holy:GeographicMarket ;
                       rdfs:label "application sold in"@en ;
                       skos:altLabel "available in"@en ;
                       skos:definition "Defines in which geographic market an application is sold or available for use."@en .


###  http://purl.org/holy/ns#hasApplication
holy:hasApplication rdf:type owl:ObjectProperty ,
                             owl:AsymmetricProperty ,
                             owl:IrreflexiveProperty ;
                    rdfs:domain holy:GeographicMarket ;
                    rdfs:range holy:Application ;
                    rdfs:label "has Application"@en ;
                    skos:definition "Relates to the geographic location of applications in the market."@en .


###  http://purl.org/holy/ns#hasIndicator
holy:hasIndicator rdf:type owl:ObjectProperty ,
                           owl:AsymmetricProperty ,
                           owl:IrreflexiveProperty ;
                  rdfs:domain [ rdf:type owl:Class ;
                                owl:unionOf ( holy:Application
                                              holy:GeographicMarket
                                              holy:Product
                                              schema:Project
                                              org:Organization
                                            )
                              ] ;
                  rdfs:range holy:Indicator ;
                  rdfs:comment "In the hydrogen ontology, all major classes (organization, project, application, geographical market and product) are linked to the class indicator."@en ;
                  rdfs:label "has Indicator"@en ;
                  skos:definition "Refers to indicators which are related to a certain class."@en .


###  http://purl.org/holy/ns#hasOrganization
holy:hasOrganization rdf:type owl:ObjectProperty ;
                     owl:inverseOf holy:participatesIn ;
                     rdf:type owl:AsymmetricProperty ,
                              owl:IrreflexiveProperty ;
                     rdfs:domain holy:GeographicMarket ;
                     rdfs:range org:Organization ;
                     owl:propertyChainAxiom ( [ owl:inverseOf dbo:continent
                                              ]
                                              holy:hasOrganization
                                            ) ;
                     rdfs:label "has Organization"@en ;
                     skos:definition "Indicates a direkt link from a geographic location to an organization. It shows where a organization is located."@en .


###  http://purl.org/holy/ns#hasProduct
holy:hasProduct rdf:type owl:ObjectProperty ;
                owl:inverseOf holy:productSoldIn ;
                rdf:type owl:AsymmetricProperty ,
                         owl:IrreflexiveProperty ;
                rdfs:domain holy:GeographicMarket ;
                rdfs:range holy:Product ;
                rdfs:label "has Product"@en ;
                skos:definition "Indicates a direkt link from a geographic location to a product. It shows where a product is located."@en .


###  http://purl.org/holy/ns#hasProject
holy:hasProject rdf:type owl:ObjectProperty ,
                         owl:AsymmetricProperty ,
                         owl:IrreflexiveProperty ;
                rdfs:domain holy:GeographicMarket ;
                rdfs:range schema:Project ;
                rdfs:label "has Project"@en ;
                skos:definition "Relates to the geographic location of projects in the market."@en .


###  http://purl.org/holy/ns#isProducedBy
holy:isProducedBy rdf:type owl:ObjectProperty ;
                  owl:inverseOf holy:producesProduct ;
                  rdf:type owl:AsymmetricProperty ,
                           owl:IrreflexiveProperty ;
                  rdfs:domain holy:Product ;
                  rdfs:range org:Organization ;
                  rdfs:comment "The inverse of holy:producesProduct"@en ;
                  rdfs:label "is produced by"@en ;
                  skos:definition "Indicates which products are manufactured by a given organization."@en .


###  http://purl.org/holy/ns#isProvidedBy
holy:isProvidedBy rdf:type owl:ObjectProperty ;
                  owl:inverseOf holy:providesApplication ;
                  rdf:type owl:AsymmetricProperty ,
                           owl:IrreflexiveProperty ;
                  rdfs:domain holy:Application ;
                  rdfs:range org:Organization ;
                  rdfs:comment "The inverse of holy:providesApplication"@en ;
                  rdfs:label "is provided by"@en ;
                  skos:definition "Indicates which applications are related to an organization in terms of manufacturing, operating, licensing, leasing..."@en .


###  http://purl.org/holy/ns#isUsedIn
holy:isUsedIn rdf:type owl:ObjectProperty ;
              rdfs:subPropertyOf owl:topObjectProperty ;
              owl:inverseOf holy:usesProduct ,
                            holy:usesSource ,
                            holy:usesTechnology ;
              rdf:type owl:AsymmetricProperty ,
                       owl:IrreflexiveProperty ;
              rdfs:domain holy:Product ;
              rdfs:range holy:Application ;
              rdfs:comment "Inverse of holy:usesProduct and holy:usesTechnology"@en ;
              rdfs:label "is used in"@en ;
              skos:definition "Defines for which purpose a product is used in."@en .


###  http://purl.org/holy/ns#participatesIn
holy:participatesIn rdf:type owl:ObjectProperty ,
                             owl:AsymmetricProperty ,
                             owl:IrreflexiveProperty ;
                    rdfs:domain org:Organization ;
                    rdfs:range holy:GeographicMarket ;
                    rdfs:label "participates in"@en ;
                    skos:definition "Defines that an organization participates with presence in a certain geographic market."@en .


###  http://purl.org/holy/ns#producesProduct
holy:producesProduct rdf:type owl:ObjectProperty ,
                              owl:AsymmetricProperty ,
                              owl:IrreflexiveProperty ;
                     rdfs:domain org:Organization ;
                     rdfs:range holy:Product ;
                     rdfs:label "produces Product"@en ;
                     skos:definition "Indicates which organization manufactures a given product."@en .


###  http://purl.org/holy/ns#productSoldIn
holy:productSoldIn rdf:type owl:ObjectProperty ,
                            owl:AsymmetricProperty ,
                            owl:IrreflexiveProperty ;
                   rdfs:domain holy:Product ;
                   rdfs:range holy:GeographicMarket ;
                   rdfs:comment "The inverse of holy:hasProduct"@en ;
                   rdfs:label "product sold in"@en ;
                   skos:definition "Defines in which geographic market a product is sold or available for use."@en .


###  http://purl.org/holy/ns#providesApplication
holy:providesApplication rdf:type owl:ObjectProperty ,
                                  owl:AsymmetricProperty ,
                                  owl:IrreflexiveProperty ;
                         rdfs:domain org:Organization ;
                         rdfs:range holy:Application ;
                         rdfs:comment "The inverse of holy:isProvidedBy"@en ;
                         rdfs:label "provides Application"@en ;
                         skos:definition "Indicates which organizations are directly providing applications (the end-usage) to the market either by manufacturing the application or operating, licensing, leasing... it."@en .


###  http://purl.org/holy/ns#relatesToApplication
holy:relatesToApplication rdf:type owl:ObjectProperty ,
                                   owl:AsymmetricProperty ,
                                   owl:IrreflexiveProperty ;
                          rdfs:domain schema:Project ;
                          rdfs:range holy:Application ;
                          rdfs:label "relates to Application"@en ;
                          skos:definition "Defines that a certain project is in terms of outcome related to an application."@en .


###  http://purl.org/holy/ns#relatesToProduct
holy:relatesToProduct rdf:type owl:ObjectProperty ,
                               owl:AsymmetricProperty ,
                               owl:IrreflexiveProperty ;
                      rdfs:domain schema:Project ;
                      rdfs:range holy:Product ;
                      rdfs:label "relates to Product"@en ;
                      skos:definition "Defines that a certain project is in terms of its outcome related to a product."@en .


###  http://purl.org/holy/ns#usesProduct
holy:usesProduct rdf:type owl:ObjectProperty ;
                 rdfs:subPropertyOf holy:usesSource ;
                 rdf:type owl:IrreflexiveProperty ;
                 rdfs:domain holy:Application ;
                 rdfs:range holy:Product ;
                 rdfs:comment "Inverse of holy:isUsedIn - Disjoint with holy:usesTechnology"@en ;
                 rdfs:label "uses Product"@en ;
                 skos:definition "Defines the product used in a particular application"@en .


###  http://purl.org/holy/ns#usesSource
holy:usesSource rdf:type owl:ObjectProperty ,
                         owl:IrreflexiveProperty ;
                rdfs:domain holy:Application ;
                rdfs:range holy:Product ;
                rdfs:comment "Main Property for holy:usesProduct and holy:usesTechnology."@en ;
                rdfs:label "uses Source"@en .


###  http://purl.org/holy/ns#usesTechnology
holy:usesTechnology rdf:type owl:ObjectProperty ;
                    rdfs:subPropertyOf holy:usesSource ;
                    rdf:type owl:IrreflexiveProperty ;
                    rdfs:domain holy:Application ;
                    rdfs:range holy:Product ;
                    rdfs:comment "Inverse of holy:isUsedIn - Disjoint with holy:usesApplication"@en ;
                    rdfs:label "uses Technology"@en ;
                    skos:definition "Defines the technology used in a particular application."@en .


###  http://w3id.org/nfdi4ing/metadata4ing#inProject
m4i:inProject rdf:type owl:ObjectProperty ;
              rdfs:subPropertyOf owl:topObjectProperty ;
              owl:inverseOf m4i:projectParticipant ;
              rdf:type owl:AsymmetricProperty ,
                       owl:IrreflexiveProperty ;
              rdfs:domain org:Organization ;
              rdfs:range schema:Project ;
              dct:references m4i: ;
              rdfs:comment "An object property comming from the Metadata4Ing ontology for describing the generation of research data, projects and scientific projects. The ontology was released recently on the 22.02.2022 and could be useful for future expansion of the hydrogen ontology."@en ,
                           "The inverse of m4i:projectParticipant"@en ;
              rdfs:label "associated to project"@en ;
              skos:altLabel "responsible for"@en ,
                            "sponsor of project"@en ;
              skos:definition "A property that connects a person or an organization with a project."@en .


###  http://w3id.org/nfdi4ing/metadata4ing#projectParticipant
m4i:projectParticipant rdf:type owl:ObjectProperty ,
                                owl:AsymmetricProperty ,
                                owl:IrreflexiveProperty ;
                       rdfs:domain schema:Project ;
                       rdfs:range org:Organization ;
                       dct:references m4i: ;
                       rdfs:comment "An object property comming from the Metadata4Ing ontology for describing the generation of research data, projects and scientific projects. The ontology was released recently on the 22.02.2022 and could be useful for future expansion of the hydrogen ontology."@en ,
                                    "The inverse of m4i:associatesToProject"@en ;
                       rdfs:label "project participant"@en ;
                       skos:altLabel "project partner"@en ;
                       skos:definition "A property that connects a project with a person or an organisation."@en .


###  http://www.w3.org/ns/org#classification
org:classification rdf:type owl:ObjectProperty ;
                   rdfs:subPropertyOf owl:topObjectProperty ;
                   rdf:type owl:AsymmetricProperty ,
                            owl:IrreflexiveProperty ;
                   rdfs:domain org:Organization ;
                   rdfs:range skos:Concept ;
                   dct:references org: ;
                   rdfs:comment "Main property of rov:orgActivity"@en ;
                   rdfs:label "classification"@en ;
                   skos:definition "Indicates a classification for this Organization within some classification scheme."@en .


###  http://www.w3.org/ns/org#hasPrimarySite
org:hasPrimarySite rdf:type owl:ObjectProperty ;
                   rdfs:subPropertyOf org:hasSite ;
                   rdf:type owl:FunctionalProperty ,
                            owl:AsymmetricProperty ,
                            owl:IrreflexiveProperty ;
                   rdfs:domain org:Organization ;
                   rdfs:range holy:GeographicMarket ;
                   dct:references org: ;
                   rdfs:label "primary Site"@en ;
                   skos:definition "Indicates a primary site for the Organization, this is the default means by which an Organization can be contacted and is not necessarily the formal headquarters."@en .


###  http://www.w3.org/ns/org#hasSite
org:hasSite rdf:type owl:ObjectProperty ;
            owl:inverseOf org:siteOf ;
            rdf:type owl:AsymmetricProperty ,
                     owl:IrreflexiveProperty ;
            rdfs:domain org:Organization ;
            rdfs:range holy:GeographicMarket ;
            dct:references org: ;
            rdfs:label "has site"@en ;
            skos:definition "Indicates a site at which the Organization has some presence even if only indirect (e.g. virtual office or a professional service which is acting as the registered address for a company)."@en .


###  http://www.w3.org/ns/org#hasSubOrganization
org:hasSubOrganization rdf:type owl:ObjectProperty ;
                       owl:inverseOf org:subOrganizationOf ;
                       rdf:type owl:AsymmetricProperty ,
                                owl:TransitiveProperty ,
                                owl:IrreflexiveProperty ;
                       rdfs:domain org:Organization ;
                       rdfs:range org:Organization ;
                       dct:references org: ;
                       rdfs:label "has SubOrganization"@en ;
                       skos:definition "Represents hierarchical containment of Organizations or OrganizationalUnits; indicates an organization which is a sub-part or child of this organization."@en .


###  http://www.w3.org/ns/org#linkedTo
org:linkedTo rdf:type owl:ObjectProperty ,
                      owl:SymmetricProperty ;
             rdfs:domain org:Organization ;
             rdfs:range org:Organization ;
             dct:references org: ;
             rdfs:comment "In the current stage of the Hydrogen Domain Ontology it is used to indicate mainly business relationships outside of the project scope."@en ;
             rdfs:label "linked to"@en ;
             skos:definition "Indicates an arbitrary relationship between two organizations."@en .


###  http://www.w3.org/ns/org#siteOf
org:siteOf rdf:type owl:ObjectProperty ;
           rdfs:subPropertyOf owl:topObjectProperty ;
           rdfs:domain holy:GeographicMarket ;
           rdfs:range org:Organization ;
           dct:references <http://www.w3.org/ns/org> ;
           rdfs:label "site of"@en ;
           skos:definition "Indicates an Organization which has some presence at the given site. This is the inverse of `org:hasSite`."@en .


###  http://www.w3.org/ns/org#subOrganizationOf
org:subOrganizationOf rdf:type owl:ObjectProperty ;
                      rdfs:subPropertyOf owl:topObjectProperty ;
                      rdf:type owl:AsymmetricProperty ,
                               owl:TransitiveProperty ;
                      rdfs:domain org:Organization ;
                      rdfs:range org:Organization ;
                      dct:references org: ;
                      rdfs:label "sub-Organization of"@en ;
                      skos:definition "Represents hierarchical containment of Organizations or OrganizationalUnits; indicates an Organization which contains this Organization."@en .


###  http://www.w3.org/ns/regorg#orgActivity
rov:orgActivity rdf:type owl:ObjectProperty ;
                rdfs:subPropertyOf org:classification ;
                rdf:type owl:AsymmetricProperty ,
                         owl:IrreflexiveProperty ;
                rdfs:domain rov:RegisteredOrganization ;
                rdfs:range skos:Concept ;
                dct:references org: ;
                rdfs:comment "Relates to the economic activity of an organization based on international classification standards such as NACE (EU) ISIC4 (US) or the UK SIC codes."@en ;
                rdfs:label "company activity"@en ;
                skos:definition "The activity of an organization should be recorded using a controlled vocabulary. Several such vocabularies exist, many of which map to the UN's ISIC codes [ ISIC4 ]. Where a particular controlled vocabulary is in use within a given context, such as SIC codes in the UK, it is acceptable to use these, however, the preferred choice for European interoperability is NACE [ NACE ]. As with company type and status, activity codes should be expressed as SKOS Concept Schemes."@en .


###  http://www.w3.org/ns/regorg#orgStatus
rov:orgStatus rdf:type owl:ObjectProperty ,
                       owl:AsymmetricProperty ,
                       owl:IrreflexiveProperty ;
              rdfs:domain org:Organization ;
              rdfs:range skos:Concept ;
              dct:references rov: ;
              rdfs:comment "rov:orgStatus provides a first attempt -used in the Registered Organization Vocabulary- to identify the status of an organization."@en ;
              rdfs:label "company status"@en ;
              skos:definition """Extracting the status of an organization presents the same issues as its type. The terms 'insolvent', 'bankrupt' and 'in receivership,' for example, are likely to mean slightly different things with different legal implications in different jurisdictions.

Taking advice from XBRL Europe as a starting point, however, the term 'Normal Activity' does appear to have cross-border usefulness and this should be used in preference to terms like 'trading' or 'operating.'

Best Practice for recording various other status levels is to use the relevant jurisdiction's terms and to encode these in a SKOS Concept Scheme."""@en .


###  http://www.w3.org/ns/regorg#orgType
rov:orgType rdf:type owl:ObjectProperty ,
                     owl:AsymmetricProperty ,
                     owl:IrreflexiveProperty ;
            rdfs:domain org:Organization ;
            rdfs:range skos:Concept ;
            dct:references rov: ;
            rdfs:label "company type"@en ;
            skos:definition """This property records the type of company. Familiar types are SA, PLC, LLC, GmbH etc. At the time of publication, there is no agreed set of company types that crosses borders. The term 'SA' is used in Poland and France for example although they mean slightly different things. The UK's LLP and Greece's EPE provide further example of close, but not exact, matches.

That said, each jurisdiction will have a limited set of recognized company types and these should be expressed in a consistent manner in a SKOS Concept Scheme."""@en .


#################################################################
#    Data properties
#################################################################

###  http://data.businessgraph.io/ontology#isPubliclyTraded
ebg:isPubliclyTraded rdf:type owl:DatatypeProperty ;
                     rdfs:domain rov:RegisteredOrganization ;
                     rdfs:range xsd:boolean ;
                     dct:references ebg: ;
                     rdfs:label "is publicly traded"@en ;
                     skos:definition "Whether a company is publicly traded (listed at a stock exchange)."@en .


###  http://data.businessgraph.io/ontology#isStartup
ebg:isStartup rdf:type owl:DatatypeProperty ;
              rdfs:domain rov:RegisteredOrganization ;
              rdfs:range xsd:boolean ;
              dct:references ebg: ;
              rdfs:label "is startup"@en ;
              skos:definition "Whether a company is a startup."@en .


###  http://data.businessgraph.io/ontology#isStateOwned
ebg:isStateOwned rdf:type owl:DatatypeProperty ;
                 rdfs:domain rov:RegisteredOrganization ;
                 rdfs:range xsd:boolean ;
                 dct:references ebg: ;
                 rdfs:label "is state owned"@en ;
                 skos:definition "Whether a company is owned by the government, a government agency, municipality, city or other public entity."@en .


###  http://dbpedia.org/ontology/projectEndDate
dbo:projectEndDate rdf:type owl:DatatypeProperty ;
                   owl:equivalentProperty m4i:endOfProject ;
                   rdfs:domain schema:Project ;
                   rdfs:range xsd:date ;
                   rdfs:label "project end date"@en ;
                   skos:definition "The end date of the project."@en .


###  http://dbpedia.org/ontology/projectKeyword
dbo:projectKeyword rdf:type owl:DatatypeProperty ;
                   rdfs:domain schema:Project ;
                   rdfs:range xsd:string ;
                   rdfs:label "project Keyword"@en ;
                   skos:definition "A key word of the project."@en .


###  http://dbpedia.org/ontology/projectStartDate
dbo:projectStartDate rdf:type owl:DatatypeProperty ;
                     owl:equivalentProperty m4i:startOfProject ;
                     rdfs:domain schema:Project ;
                     rdfs:range xsd:date ;
                     rdfs:label "project start date"@en ;
                     skos:definition "The start date of the project."@en .


###  http://w3id.org/nfdi4ing/metadata4ing#endOfProject
m4i:endOfProject rdf:type owl:DatatypeProperty ;
                 rdfs:domain schema:Project ;
                 rdfs:range xsd:date ;
                 dct:references m4i: ;
                 rdfs:label "project end date"@en ;
                 skos:definition "end date of a project"@en .


###  http://w3id.org/nfdi4ing/metadata4ing#startOfProject
m4i:startOfProject rdf:type owl:DatatypeProperty ;
                   rdfs:domain schema:Project ;
                   rdfs:range xsd:date ;
                   dct:references m4i: ;
                   rdfs:label "project start date"@en ;
                   skos:definition "start date of a project"@en .


#################################################################
#    Classes
#################################################################

###  http://purl.org/holy/ns#AirCompressor
holy:AirCompressor rdf:type owl:Class ;
                   rdfs:subClassOf holy:HydrogenFuelCellComponent ;
                   dct:references <https://www.energy.gov/eere/fuelcells/fuel-cell-systems> ;
                   rdfs:label "Air Compressor"@en ;
                   skos:altLabel "Air Compressor"@en ;
                   skos:definition "A pressure regulating system for enhancing fuel cell improvement by increasing pressure of reactant gases."@en .


###  http://purl.org/holy/ns#Aircraft
holy:Aircraft rdf:type owl:Class ;
              rdfs:subClassOf holy:AviaticApplication ;
              dct:references <http://wordnetweb.princeton.edu/perl/webwn?s=plane&sub=Search+WordNet&o2=&o0=1&o8=1&o1=1&o7=&o5=&o9=&o6=&o3=&o4=&h=0000> ,
                             <https://dictionary.cambridge.org/dictionary/english/aircraft> ;
              wn:hyponym "Aeroplane"@en ,
                         "Airplane"@en ,
                         "Cargo Plane"@en ,
                         "Drone"@en ,
                         "Helicopter"@en ,
                         "Long-duration aircraft"@en ,
                         "Long-endurance aircraft"@en ,
                         "Passenger Plane"@en ,
                         "STOL"@en ,
                         "Short Takeoff and Landing Aircraft"@en ,
                         "UAV"@en ,
                         "Unmanned Aerial Vehicle"@en ,
                         "Unmanned Long-duration Aircraft"@en ,
                         "Zero-emission Aircraft"@en ,
                         "long-haul aircraft"@en ;
              rdfs:label "Aircraft"@en ;
              skos:altLabel "Aircraft"@en ;
              skos:definition "A vehicle which can fly and carry goods or passengers. It has fixed wings and is powered by propellers or jets."@en ;
              skos:example "A321neo"@en ;
              skos:hiddenLabel "Plane"@en .


###  http://purl.org/holy/ns#AlkalineBattery
holy:AlkalineBattery rdf:type owl:Class ;
                     rdfs:subClassOf holy:Battery ;
                     dct:references "https://doi.org/10.1016/B978-044452745-5.00854-6"@en ;
                     rdfs:label "Alkaline Battery"@en ;
                     skos:altLabel "Alkaline Battery"@en ;
                     skos:definition "A battery which uses a chemical substance composed of zinc (Zn) and manganese dioxide (MnO2). The separator in alkaline batteries is made totally or at least partially of nonwoven materials." .


###  http://purl.org/holy/ns#AlkalineFuelCell
holy:AlkalineFuelCell rdf:type owl:Class ;
                      rdfs:subClassOf holy:HydrogenReconversion ;
                      dct:references <https://www.energy.gov/eere/fuelcells/types-fuel-cells> ;
                      rdfs:label "Alkaline Fuel Cell"@en ;
                      skos:altLabel "AMFC"@en ,
                                    "Alkaline Electrolyzer"@en ,
                                    "Alkaline Fuel CEll"@en ,
                                    "Alkaline Membrane Fuel Cells"@en ;
                      skos:definition "A fuel cell which uses potassium hydroxide in water as the electrolyte for powering, using a variety of non-precious metals as a catalyst at the anode and cathode."@en .


###  http://purl.org/holy/ns#AmmoniaFuelCell
holy:AmmoniaFuelCell rdf:type owl:Class ;
                     rdfs:subClassOf holy:SubstituteFuelCell ;
                     dct:references <https://www.fuelcellstore.com/blog-section/alternative-liquid-fuel-types-fuel-cells> ;
                     rdfs:label "Ammonia Fuel Cell"@en ;
                     skos:altLabel "Ammonia Fuel Cell"@en ,
                                   "DAFC"@en ,
                                   "Direct Ammonia Fuel Cell"@en ;
                     skos:definition "A fuel cell using ammonia as its fuel."@en .


###  http://purl.org/holy/ns#AnionExchangeMembraneFuelCell
holy:AnionExchangeMembraneFuelCell rdf:type owl:Class ;
                                   rdfs:subClassOf holy:HydrogenReconversion ;
                                   rdfs:label "Anion Exchange Membrane Fuel Cell"@en ;
                                   skos:altLabel "AEM"@en ,
                                                 "AEMFC"@en ,
                                                 "Anion Exchange Membrane Fuel Cell"@en ,
                                                 "Anion exchange membrane"@en ;
                                   skos:definition "A PEMFC-like fuel cell technology which needs less precious metals as catalysts in order to trigger chemical reaction."@en .


###  http://purl.org/holy/ns#Application
holy:Application rdf:type owl:Class ;
                 rdfs:subClassOf owl:Thing ;
                 owl:disjointWith holy:GeographicMarket ;
                 dct:references <http://wordnetweb.princeton.edu/perl/webwn?s=application&sub=Search+WordNet&o2=&o0=1&o8=1&o1=1&o7=&o5=&o9=&o6=&o3=&o4=&h=0> ,
                                <http://www.chfca.ca/fuel-cells-hydrogen/hydrogen-fuel-cell-applications/> ,
                                <https://dictionary.cambridge.org/dictionary/english/application> ,
                                <https://wha-international.com/10-hydrogen-fuel-cell-applications-you-might-not-know/> ;
                 wn:hyponym "Fuel Cell Technology Industry Application"@en ,
                            "Hydrogen Energy Industry Application"@en ,
                            "Hydrogen Fuel Cell Application"@en ,
                            "Industry Applications of Hydrogen Fuel Cells"@en ,
                            "Practical Application"@en ;
                 rdfs:label "Application"@en ;
                 skos:altLabel "Application"@en ,
                               "Usance"@en ,
                               "Use Case"@en ,
                               "Utilization"@en ;
                 skos:definition "The intended end use of a hydrogen-based product or of the result of a hydrogen-related project."@en ;
                 skos:hiddenLabel "End Use"@en .


###  http://purl.org/holy/ns#AviaticApplication
holy:AviaticApplication rdf:type owl:Class ;
                        rdfs:subClassOf holy:MobileApplication ;
                        dct:references <https://dictionary.cambridge.org/dictionary/english/aviation> ;
                        rdfs:label "Aviatic Application"@en ;
                        skos:altLabel "Aeronautics"@en ,
                                      "Air Travel"@en ,
                                      "Airmanship"@en ,
                                      "Aviation"@en ;
                        skos:definition "An application related to the transport of people and/or goods by any form of aircraft or spacecraft."@en ;
                        skos:hiddenLabel "Air Power"@en .


###  http://purl.org/holy/ns#Battery
holy:Battery rdf:type owl:Class ;
             rdfs:subClassOf holy:SubstituteProduct ;
             dct:references <https://www.wiltronics.com.au/wiltronics-knowledge-base/different-types-of-batteries/> ;
             wn:hyponym "BESS"@en ,
                        "BTMS"@en ,
                        "Barge Battery System"@en ,
                        "Battery Cell"@en ,
                        "Battery Energy Storage System"@en ,
                        "Battery Thermal Management System"@en ,
                        "Battery Wall"@en ,
                        "Electric Battery"@en ,
                        "Electric Car Battery"@en ,
                        "Fully Electric Barge Battery Container"@en ,
                        "Hybrid Membrane Edges Flow Batteries"@en ,
                        "Lead Acid Battery"@en ,
                        "Perfluorinated Sulfonic Acid battery"@en ,
                        "Redox Flow Batteries"@en ,
                        "Vanadium Redox Flow Battery"@en ;
             rdfs:label "Battery"@en ;
             skos:altLabel "Battery"@en ;
             skos:definition "A collection of one or more cells which store electrical energy for powering electrical devices."@en ;
             skos:hiddenLabel "Hybrid Membrane"@en .


###  http://purl.org/holy/ns#BatteryComponent
holy:BatteryComponent rdf:type owl:Class ;
                      rdfs:subClassOf holy:SubstituteProductComponent ;
                      rdfs:comment "The subclass \"Battery Component\" can be expanded to focus on batteries as substitutes for hydrogen products. "@en ;
                      rdfs:label "Battery Component"@en ;
                      skos:definition "A basic component for batteries."@en .


###  http://purl.org/holy/ns#Bike
holy:Bike rdf:type owl:Class ;
          rdfs:subClassOf holy:RoadApplication ;
          dct:references <https://dictionary.cambridge.org/dictionary/english/bike> ;
          wn:hyponym "Bicycle"@en ,
                     "Electric Moped"@en ,
                     "Hydrogen Bicycle"@en ,
                     "Hydrogen Bike"@en ,
                     "Hydrogen Scooter"@en ,
                     "Hydrogen-powered Bike"@en ,
                     "Hydrogen-powered E-bike"@en ,
                     "Moped"@en ,
                     "Motorbike"@en ,
                     "Motorcycle"@en ,
                     "Race Bike"@en ,
                     "Road Bike"@en ,
                     "Scooter"@en ;
          rdfs:label "Bike"@en ;
          skos:altLabel "Bike"@en ;
          skos:definition "A motorbike, motorcycle or scooter."@en ;
          skos:example "Honda Grazia Repsol Honda Team Edition"@en ;
          skos:hiddenLabel "Cycling"@en .


###  http://purl.org/holy/ns#BipolarPlate
holy:BipolarPlate rdf:type owl:Class ;
                  rdfs:subClassOf holy:SupportiveHardware ;
                  dct:references <https://www.energy.gov/eere/fuelcells/parts-fuel-cell> ;
                  rdfs:label "Bipolar Plate"@en ;
                  skos:altLabel "Bipolar Plate"@en ;
                  skos:definition "A plate which provides electrical conduction between cells. Bipolar plates are used to separate cells within a fuel cell from each other and aim to provide physical strength to the stack of cells."@en .


###  http://purl.org/holy/ns#Bus
holy:Bus rdf:type owl:Class ;
         rdfs:subClassOf holy:RoadApplication ;
         dct:references <https://dictionary.cambridge.org/dictionary/english/bus> ;
         wn:hyponym "City Bus"@en ,
                    "Double-decker"@en ,
                    "Hydrogen Fuel Cell Electric Bus"@en ,
                    "Hydrogen-powered Bus"@en ,
                    "Minibus"@en ,
                    "Municipal Bus"@en ,
                    "PEM Fuel Cell Bus"@en ,
                    "School Bus"@en ,
                    "Transit Bus"@en ,
                    "Trolleybus"@en ,
                    "Zero-emission Bus"@en ;
         rdfs:label "Bus"@en ;
         skos:altLabel "Bus"@en ;
         skos:definition "A large motorzed vehicle with seats for many people."@en ;
         skos:example "Xcelsior CHARGE"@en .


###  http://purl.org/holy/ns#Car
holy:Car rdf:type owl:Class ;
         rdfs:subClassOf holy:RoadApplication ;
         dct:references <https://dictionary.cambridge.org/dictionary/english/car> ;
         wn:hyponym "Convertible"@en ,
                    "Coupe"@en ,
                    "Coupé"@en ,
                    "Electric SUV"@en ,
                    "Electric passenger vehicle"@en ,
                    "Hybrid Range Extender"@en ,
                    "Hybrid Vehicle"@en ,
                    "Hydrogen SUV"@en ,
                    "Jeep"@en ,
                    "Limousine"@en ,
                    "Passenger Car"@en ,
                    "Passenger Vehicle"@en ,
                    "SUV"@en ,
                    "Station Wagon"@en ;
         rdfs:label "Car"@en ;
         skos:altLabel "Auto"@en ,
                       "Automobile"@en ,
                       "Car"@en ;
         skos:definition "A road vehicle with an engine, four wheels, and seats for a small number of people."@en ;
         skos:example "Toyota Corolla"@en ,
                      "Toyota Mirai"@en ,
                      "Toyota Yaris"@en .


###  http://purl.org/holy/ns#CargoShip
holy:CargoShip rdf:type owl:Class ;
               rdfs:subClassOf holy:MarineApplication ;
               dct:references <https://www.marineinsight.com/types-of-ships/what-are-cargo-ships/> ;
               wn:hyponym "Container Ship"@en ,
                          "Freight Ship"@en ,
                          "Freight Vessel"@en ,
                          "Freighter"@en ,
                          "Oil Tanker"@en ,
                          "Supertanker"@en ,
                          "Zero-emission Cargo Ship"@en ;
               rdfs:label "Cargo Ship"@en ;
               skos:altLabel "Canal Boat"@en ,
                             "Cargo Vessel"@en ,
                             "Transport Ship"@en ;
               skos:definition "Any kind of a ship or any other vessel that transports heavy goods and materials from one port to another."@en ;
               skos:example "Ceiba Ship"@en ,
                            "Voilier Ceiba"@en .


###  http://purl.org/holy/ns#CargoTrain
holy:CargoTrain rdf:type owl:Class ;
                rdfs:subClassOf holy:Train ;
                dct:references <https://www.gymglish.com/en/gymglish/english-translation/cargo-train> ;
                wn:hyponym "Container Train"@en ,
                           "Intermodal Train"@en ;
                rdfs:label "Cargo Train"@en ;
                skos:altLabel "Cargo Train"@en ,
                              "Freight Train"@en ,
                              "Goods Train"@en ,
                              "Haulage Train"@en ;
                skos:definition "A train carrying mainly goods such as baggage, shipment or merchandise."@en ;
                skos:hiddenLabel "Nonpassenger Train"@en .


###  http://purl.org/holy/ns#CatalystLayer
holy:CatalystLayer rdf:type owl:Class ;
                   rdfs:subClassOf holy:MembraneElectrodeAssembly ;
                   dct:references <https://www.energy.gov/eere/fuelcells/parts-fuel-cell> ,
                                  "https://doi.org/10.1016/B978-044452745-5.00227-6" ;
                   rdfs:label "Catalyst Layer"@en ;
                   skos:altLabel "Catalyst Layer"@en ;
                   skos:definition "A layer of anodes and cathodes which are placed on opposite sites of the membrane. It is a three-dimensional porous structrure composed of catalyst particles and ionomer fragments."@en .


###  http://purl.org/holy/ns#ChemicalIndustrialProcessing
holy:ChemicalIndustrialProcessing rdf:type owl:Class ;
                                  rdfs:subClassOf holy:IndustrialProcessing ;
                                  dct:references <https://www.cisa.gov/sites/default/files/publications/Chemical-Sector-Profile_Final%20508.pdf> ;
                                  wn:hyponym "Ammonia Processing"@en ,
                                             "Methanol Production"@en ;
                                  rdfs:comment "Hydrogen is one of the key starting materials used in the chemical industry. It is a fundamental building block for the manufacturing of ammonia, fertilizers, and  methanol, which is used in the manufacture of many polymers."@en ;
                                  rdfs:label "Chemical Industrial Processing"@en ;
                                  skos:altLabel "Chemical Processing"@en ;
                                  skos:definition "Applications of hydrogen in the chemical industry creating chemical products for numerous sectors such as pharmaceutical, agricultural or consumer goods usage."@en .


###  http://purl.org/holy/ns#CircularEconomyProject
holy:CircularEconomyProject rdf:type owl:Class ;
                            rdfs:subClassOf holy:PurposeBasedProject ;
                            dct:references <https://clustercollaboration.eu/content/circular-economy-project-management-system-0> ;
                            wn:hyponym "Industrial Symbiosis Project"@en ;
                            rdfs:label "Circular Economy Project"@en ;
                            skos:altLabel "Circular Economy Project"@en ;
                            skos:definition "A project focusing on a circular system of reusing resources which were previously used for something."@en ;
                            skos:hiddenLabel "Ecodesign project"@en ,
                                             "Life Cycle Management Project"@en ,
                                             "Smart Farm Linked Hydrogen Fuel Cell Power Generation Project"@en .


###  http://purl.org/holy/ns#CruiseShip
holy:CruiseShip rdf:type owl:Class ;
                rdfs:subClassOf holy:MarineApplication ;
                dct:references <https://dictionary.cambridge.org/dictionary/english/cruise-ship> ;
                rdfs:label "Cruise Ship"@en ;
                skos:altLabel "Cruise Liner"@en ,
                              "Passenger Ship"@en ;
                skos:definition "A large ship like a hotel which people use for travel and pleasure."@en ;
                skos:hiddenLabel "Liner"@en .


###  http://purl.org/holy/ns#EnergySectorOrganization
holy:EnergySectorOrganization rdf:type owl:Class ;
                              rdfs:subClassOf rov:RegisteredOrganization ;
                              dct:references <https://ec.europa.eu/eurostat/documents/3859598/5902521/KS-RA-07-015-EN.PDF> ;
                              rdfs:label "Energy Sector Organization"@en ;
                              skos:altLabel "Energy Sector"@en ;
                              skos:definition "An organization who participates in the activity of providing electric power, natural gas, steam, hot water and the like through a permanent infrastructure (network) of lines, mains and pipes. The dimension of the network is not decisive; also included is the distribution of electricity, gas, steam, hot water and the like in industrial parks or residential buildings according to Section D of EC NACE Rev. 2."@en ;
                              skos:hiddenLabel "Renewable Fuel Producer"@en .


###  http://purl.org/holy/ns#EntryBarrier
holy:EntryBarrier rdf:type owl:Class ;
                  rdfs:subClassOf holy:Indicator ;
                  wn:hyponym "Market Permit"@en ,
                             "Political Constraint"@en ,
                             "Regulation"@en ;
                  rdfs:label "Entry Barrier"@en ;
                  skos:definition "An obstacle individuals face when participating in a particular market."@en ;
                  skos:hiddenLabel "ESG"@en ,
                                   "Environmental, Social and Corporate Governance"@en ,
                                   "Governmental Roadblock"@en .


###  http://purl.org/holy/ns#EthanolFuelCell
holy:EthanolFuelCell rdf:type owl:Class ;
                     rdfs:subClassOf holy:SubstituteFuelCell ;
                     dct:references <https://www.fuelcellstore.com/blog-section/alternative-liquid-fuel-types-fuel-cells> ,
                                    <https://www.sciencedirect.com/science/article/pii/B9780128186244000042> ;
                     rdfs:label "Ethanol Fuel Cell"@en ;
                     skos:altLabel "DEFC"@en ,
                                   "Direct Ethanol Fuel Cell"@en ,
                                   "Ethanol Fuel Cell"@en ;
                     skos:definition "A fuel cell using ethanol as its fuel."@en ;
                     skos:hiddenLabel "Ethanol Powered Engines"@en .


###  http://purl.org/holy/ns#Ferry
holy:Ferry rdf:type owl:Class ;
           rdfs:subClassOf holy:MarineApplication ;
           dct:references <https://dictionary.cambridge.org/dictionary/english/ferry> ;
           wn:hyponym "Car-ferry"@en ;
           rdfs:label "Ferry"@en ;
           skos:altLabel "Car Ferry"@en ,
                         "Ferryboat"@en ;
           skos:definition "A boat or ship for taking passengers and often vehicles across an area of water, especially as a regular service."@en .


###  http://purl.org/holy/ns#FinishedProject
holy:FinishedProject rdf:type owl:Class ;
                     rdfs:subClassOf holy:StateBasedProject ;
                     dct:references <https://www.referenceforbusiness.com/management/Pr-Sa/Project-Management.html> ;
                     rdfs:label "Finished Project"@en ;
                     skos:altLabel "Completed Project"@en ;
                     skos:definition "A project which has completed its intended purpose regardless of the level of success."@en ;
                     skos:hiddenLabel "Have Been Completed"@en ,
                                      "Project Was Deemed Succesful"@en ,
                                      "Was a Project"@en .


###  http://purl.org/holy/ns#FossilFuel
holy:FossilFuel rdf:type owl:Class ;
                rdfs:subClassOf holy:SubstituteProduct ;
                rdfs:comment "The subclass \"FossilFuel\" could be expanded to focus the domain scope to the creation of hydrogen concerning the value chain."@en ;
                rdfs:label "Fossil Fuel"@en ;
                skos:altLabel "Fossil Fuel"@en ;
                skos:definition "A conventional energy production method using fossil fuels as fuel."@en ;
                skos:hiddenLabel "Combustion Engine"@en ,
                                 "Fossil Fuel Tank"@en ,
                                 "Gasoline Engine"@en .


###  http://purl.org/holy/ns#FossilFuelComponent
holy:FossilFuelComponent rdf:type owl:Class ;
                         rdfs:subClassOf holy:SubstituteProductComponent ;
                         rdfs:comment "The subclass \"Fossil Fuel Component\" could be expanded to focus on the components of fossil fuel products classifying as substitutes for hydrogen products."@en ;
                         rdfs:label "Fossil Fuel Component"@en ;
                         skos:definition "A basic component for products using fossil fuels."@en .


###  http://purl.org/holy/ns#FuelCellStack
holy:FuelCellStack rdf:type owl:Class ;
                   rdfs:subClassOf holy:HydrogenFuelCellComponent ;
                   dct:references <https://www.energy.gov/eere/fuelcells/fuel-cell-systems> ;
                   rdfs:label "Fuel Cell Stack"@en ;
                   skos:altLabel "Fuel Cell Stack"@en ;
                   skos:definition "The heart of a fuel cell responsible for energy generation."@en .


###  http://purl.org/holy/ns#FuelProcessor
holy:FuelProcessor rdf:type owl:Class ;
                   rdfs:subClassOf holy:HydrogenFuelCellComponent ;
                   dct:references <https://www.energy.gov/eere/fuelcells/fuel-cell-systems> ;
                   rdfs:label "Fuel Processor"@en ;
                   skos:altLabel "Fuel Processor"@en ;
                   skos:definition "A converter which is necessary to convert fuel into a fuel cell-usable form."@en .


###  http://purl.org/holy/ns#GasDiffusionLayer
holy:GasDiffusionLayer rdf:type owl:Class ;
                       rdfs:subClassOf holy:MembraneElectrodeAssembly ;
                       dct:references <https://www.energy.gov/eere/fuelcells/parts-fuel-cell> ,
                                      "https://doi.org/10.1016/B978-044452745-5.00227-6" ;
                       rdfs:label "Gas Diffusion Layer"@en ;
                       skos:altLabel "GDL"@en ,
                                     "Gas Diffusion Layer"@en ;
                       skos:definition "A paper-like layer placed outside the catalyst layer which is responsible for transporting reactants into the catalyst layer by removing chemical reaction outcomes.  In most cases, the Gas Diffusion Layer consists of a bilayer structure consisting of a macroporous diffusion medium and microporous layer."@en .


###  http://purl.org/holy/ns#Gasket
holy:Gasket rdf:type owl:Class ;
            rdfs:subClassOf holy:SupportiveHardware ;
            dct:references <https://www.energy.gov/eere/fuelcells/parts-fuel-cell> ;
            wn:hyponym "EPDM gasket"@en ,
                       "EPDM-based gasket"@en ,
                       "Fuel Cell Cap"@en ,
                       "Low Temperature Fuel Cell Gasket"@en ,
                       "PTFE-based Gasket"@en ,
                       "PTFE-coated Basket"@en ,
                       "Sealing Gasket"@en ;
            rdfs:label "Gasket"@en ;
            skos:altLabel "Gasket"@en ;
            skos:definition "A part used for gas-tight sealing of the edges of the Membrane Electrode Assembly (MEA)."@en .


###  http://purl.org/holy/ns#GeographicMarket
holy:GeographicMarket rdf:type owl:Class ;
                      owl:disjointWith holy:Indicator ,
                                       holy:Product ,
                                       schema:Project ,
                                       org:Organization ;
                      dct:references <https://dictionary.cambridge.org/dictionary/english/market> ,
                                     <https://www.irena.org/publications/2022/Jan/Geopolitics-of-the-Energy-Transformation-Hydrogen> ,
                                     <https://www.yourdictionary.com/geographical-area> ;
                      rdfs:label "Geographic Market"@en ;
                      skos:altLabel "Geographic Market"@en ;
                      skos:definition "An area of land which can be classified for business or trade concerning a particular product or domain."@en ;
                      skos:hiddenLabel "Earth"@en ,
                                       "World"@en .


###  http://purl.org/holy/ns#Heating
holy:Heating rdf:type owl:Class ;
             rdfs:subClassOf holy:StationaryApplication ;
             dct:references <http://www.element-energy.co.uk/wordpress/wp-content/uploads/2020/01/Hy4Heat-WP6-Industrial-Heating-Equipment-Published-report-Element-Energy-2019.pdf> ;
             wn:hyponym "Fuel Cell Heating System"@en ,
                        "Heating System"@en ;
             rdfs:label "Heating"@en ;
             skos:altLabel "Heat Up"@en ,
                           "Heating Application"@en ;
             skos:definition "An application which generates heat for contributing to the heating of buildings or for use in industrial processes."@en ;
             skos:hiddenLabel "Boiler"@en ,
                              "Heat"@en ,
                              "Heating Plant"@en ,
                              "Melting"@en .


###  http://purl.org/holy/ns#Humidifier
holy:Humidifier rdf:type owl:Class ;
                rdfs:subClassOf holy:HydrogenFuelCellComponent ;
                dct:references <https://www.energy.gov/eere/fuelcells/fuel-cell-systems> ;
                rdfs:label "Humidifier"@en ;
                skos:altLabel "Humidifier"@en ;
                skos:definition "An item which regulates a certain level of humidity within a fuel cell."@en .


###  http://purl.org/holy/ns#HydrogenConversion
holy:HydrogenConversion rdf:type owl:Class ;
                        rdfs:subClassOf holy:HydrogenProduct ;
                        wn:hyponym "Biological Hydrogen Processes"@en ,
                                   "Biological Hydrogen Production"@en ,
                                   "Direct Solar Water Splitting Processes"@en ,
                                   "Electrolysis"@en ,
                                   "PEM water electrolysers"@en ,
                                   "Renewable Hydrogen Production"@en ,
                                   "Thermochemical Hydrogen Processesing"@en ,
                                   "Thermochemical Hydrogen Production"@en ;
                        rdfs:comment "The subclass \"Conversion\" can be expanded to focus the domain scope to the creation of hydrogen with respect to the value chain. "@en ;
                        rdfs:label "Hydrogen Conversion"@en ;
                        skos:altLabel "Hydrogen Conversion"@en ;
                        skos:definition "The processing of materials into hydrogen."@en ;
                        skos:hiddenLabel "Blue Hydrogen"@en ,
                                         "Electrolytic Processing"@en ,
                                         "Electrolytic Production"@en ,
                                         "Green Hydrogen"@en ,
                                         "Grey Hydrogen"@en ,
                                         "Hydrogen-based Fuel"@en ,
                                         "Low Carbon Transport Fuel"@en ,
                                         "PEMWE"@en .


###  http://purl.org/holy/ns#HydrogenConversionComponent
holy:HydrogenConversionComponent rdf:type owl:Class ;
                                 rdfs:subClassOf holy:HydrogenProductComponent ;
                                 rdfs:comment "The subclass \"Hydrogen Conversion Component\" could be expanded to focus the domain scope to the transport of hydrogen with respect to the value chain."@en ;
                                 rdfs:label "Hydrogen Conversion Component"@en ;
                                 skos:definition "A basic component for products which convert compounds to hydrogen."@en .


###  http://purl.org/holy/ns#HydrogenFuelCellComponent
holy:HydrogenFuelCellComponent rdf:type owl:Class ;
                               rdfs:subClassOf holy:HydrogenProductComponent ;
                               dct:references <https://www.energy.gov/eere/fuelcells/fuel-cell-systems#fuel%20cell%20stack> ;
                               rdfs:comment "Fuel Cell Component is directly alligned with sub-classes of 'Reconversion'."@en ;
                               rdfs:label "Hydrogen Fuel Cell Component"@en ;
                               skos:definition "A basic component of hydrogen fuel cell systems."@en .


###  http://purl.org/holy/ns#HydrogenProduct
holy:HydrogenProduct rdf:type owl:Class ;
                     rdfs:subClassOf holy:Product ;
                     rdfs:comment "Concerning the scope of focusing on fuel cells and more precisely on PEMFCs, the sub-class reconversion will be the most focused class. Transportation, Storage and Conversion subclasses would receive greater attention when shifting the ontology to other areas of the hydrogen value chain."@en ;
                     rdfs:label "Hydrogen Product"@en ;
                     skos:altLabel "Hydrogen Product"@en ;
                     skos:definition "A product that is manufactured or refined for sale which can be used to produce, transport, store or \"burn\"/reconvert hydrogen."@en ;
                     skos:hiddenLabel "Hydrogen Tech"@en ,
                                      "Hydrogen Technology"@en .


###  http://purl.org/holy/ns#HydrogenProductComponent
holy:HydrogenProductComponent rdf:type owl:Class ;
                              rdfs:subClassOf holy:Product ;
                              dct:references <https://dictionary.cambridge.org/dictionary/english/component> ;
                              rdfs:label "Hydrogen Product Component"@en ;
                              skos:definition "A part that, combined with other parts, makes up a hydrogen product."@en .


###  http://purl.org/holy/ns#HydrogenReconversion
holy:HydrogenReconversion rdf:type owl:Class ;
                          rdfs:subClassOf holy:HydrogenProduct ;
                          wn:hyponym "Fuel Cell Engine"@en ,
                                     "Fuel Cell Power Module"@en ,
                                     "Fuel Cell Product"@en ,
                                     "Fuel Cell System"@en ,
                                     "Hydrogen Engine Technology"@en ,
                                     "Hydrogen Fuel Cell"@en ,
                                     "Hydrogen Fuel Cell Electric"@en ,
                                     "Hydrogen Oxygen Fuel Cell"@en ,
                                     "Hydrogen and Fuel Cell System"@en ,
                                     "Hydrogen-fueled Gas Turbines"@en ,
                                     "Hydrogen-powered Fuel Cell"@en ;
                          rdfs:comment "Since reconversion solely happenes for energy creation using fuel cells, \"Reconversion\" is contributed to fuel cell systems."@en ;
                          rdfs:label "Hydrogen Reconversion"@en ;
                          rdfs:seeAlso "Fuel Cell Solution"@en ;
                          skos:altLabel "Reconversion"@en ;
                          skos:definition "The knowledge which deals with converting hydrogen to other elements. In case of hydrogen fuel cells, hydrogen is reconverted to H2O."@en ;
                          skos:example "GR Yaris engine"@en ;
                          skos:hiddenLabel "Fuel Cell"@en .


###  http://purl.org/holy/ns#HydrogenStorage
holy:HydrogenStorage rdf:type owl:Class ;
                     rdfs:subClassOf holy:HydrogenProduct ;
                     wn:hyponym "Cryogenic Tanks"@en ,
                                "High-pressure Gas Cylinders"@en ,
                                "Hydrogen Fuel Tank"@en ,
                                "Hydrogen Storage Tanks"@en ,
                                "Liquid Hydrogen Storage Tank"@en ;
                     rdfs:comment "The subclass \"Storage\" could be expanded to focus the domain scope to the creation of hydrogen with respect to the value chain. Future expansions could categorize between storage technologies within tanks or using absorbing materials."@en ;
                     rdfs:label "Hydrogen Storage"@en ;
                     skos:definition "The way that hydrogen can be stored for later usage."@en ;
                     skos:hiddenLabel "Fuel Tank"@en ,
                                      "Hydrogen Absorbation in Metal"@en .


###  http://purl.org/holy/ns#HydrogenStorageComponent
holy:HydrogenStorageComponent rdf:type owl:Class ;
                              rdfs:subClassOf holy:HydrogenProductComponent ;
                              rdfs:comment "The subclass \"Hydrogen Storage Component\" could be expanded to focus the domain scope to the creation of hydrogen with respect to the value chain."@en ;
                              rdfs:label "Hydrogen Storage Component"@en ;
                              skos:definition "A basic component of products capable of storing hydrogen."@en .


###  http://purl.org/holy/ns#HydrogenTransport
holy:HydrogenTransport rdf:type owl:Class ;
                       rdfs:subClassOf holy:HydrogenProduct ;
                       rdfs:comment "The subclass \"Transport\" could be expanded to focus the domain scope to the creation of hydrogen in respect to the value chain."@en ;
                       rdfs:label "Hydrogen Transport"@en ;
                       skos:altLabel "Hydrogen Transport"@en ;
                       skos:definition "The way that hydrogen can be transported from one place to another."@en .


###  http://purl.org/holy/ns#HydrogenTransportComponent
holy:HydrogenTransportComponent rdf:type owl:Class ;
                                rdfs:subClassOf holy:HydrogenProductComponent ;
                                rdfs:comment "The subclass \"Hydrogen Transport Component\" could be expanded to focus the domain scope to the transport of hydrogen with respect to the value chain."@en ;
                                rdfs:label "Hydrogen Transport Component"@en ;
                                skos:definition "A basic component of products designed for transporting hydrogen."@en .


###  http://purl.org/holy/ns#Indicator
holy:Indicator rdf:type owl:Class ;
               dct:references <https://dictionary.cambridge.org/dictionary/english/indicator> ;
               rdfs:comment "Class defined to list certain market indicators of the hydrogen domain."@en ;
               rdfs:label "Indicator"@en ;
               skos:altLabel "Index"@en ;
               skos:definition "Something, often a quanititative measure, which shows what a situation is like or how it is changing."@en ;
               skos:hiddenLabel "Environmental Social Governance"@en ,
                                "FIscal Year Report"@en ,
                                "FY Report"@en .


###  http://purl.org/holy/ns#IndustrialHeating
holy:IndustrialHeating rdf:type owl:Class ;
                       rdfs:subClassOf holy:Heating ;
                       dct:references <http://www.element-energy.co.uk/wordpress/wp-content/uploads/2020/01/Hy4Heat-WP6-Industrial-Heating-Equipment-Published-report-Element-Energy-2019.pdf> ;
                       wn:hyponym "Fuel Cell-based Warehouse Heating"@en ,
                                  "Heating Plant"@en ,
                                  "Kiln Heating"@en ;
                       rdfs:label "Industrial Heating"@en ;
                       skos:altLabel "Industrial heating"@en ;
                       skos:definition "Applications used to generate heat for industry usage, such as manufacturing processes where great heat is required, or to heat large areas such as warehouses."@en ;
                       skos:hiddenLabel "Burner"@en ,
                                        "Fuel Cell Burners"@en ,
                                        "Hydrogen Burners"@en ,
                                        "Kiln"@en ,
                                        "Oven"@en .


###  http://purl.org/holy/ns#IndustrialProcessing
holy:IndustrialProcessing rdf:type owl:Class ;
                          rdfs:subClassOf holy:StationaryApplication ;
                          dct:references <https://www.ipa.fraunhofer.de/en/industry-solutions/process-industry.html> ,
                                         <https://www.irena.org/publications/2022/Jan/Geopolitics-of-the-Energy-Transformation-Hydrogen> ;
                          wn:hyponym "Circular Production System"@en ,
                                     "Linear Production System"@en ,
                                     "Purification"@en ;
                          rdfs:label "Industrial Processing"@en ;
                          skos:definition "An application which is used for industrial processing. Industrial processing involves the manufacturing of semi-finished or high-quality end products by means of physical, mechanical and/or chemical processes."@en .


###  http://purl.org/holy/ns#InfrastructureProject
holy:InfrastructureProject rdf:type owl:Class ;
                           rdfs:subClassOf holy:PurposeBasedProject ;
                           dct:references <http://www.maxwideman.com/guests/typology/projects.htm> ,
                                          <https://dictionary.cambridge.org/dictionary/english/project> ,
                                          <https://www.bigrentz.com/blog/types-of-infrastructure> ;
                           wn:hyponym "Aviation Infrastructure Project"@en ,
                                      "Bridge Infrastructure Project"@en ,
                                      "Clean Transport Project"@en ,
                                      "Commercial Construction Project"@en ,
                                      "Energy Facility Construction Project"@en ,
                                      "Energy Infrastructure Project"@en ,
                                      "Energy Transport Transformation Project"@en ,
                                      "Hydrogen Facility Development Project"@en ,
                                      "Hydrogen Fuel Cell Power Generation Project"@en ,
                                      "Hydrogen Hub Development"@en ,
                                      "Industrial Construction Project"@en ,
                                      "Power Edison Partnership"@en ,
                                      "Power and Energy Infrastructure Project"@en ,
                                      "Private Construction Project"@en ,
                                      "Public Construction Project"@en ,
                                      "Public Transportation Project"@en ,
                                      "Railroad Infrastructure Project"@en ,
                                      "Renewable Energy Development Project"@en ,
                                      "Residential Construction"@en ,
                                      "Road Infrastructure Construction Project"@en ,
                                      "Road Infrastructure Project"@en ,
                                      "Transportation Project"@en ,
                                      "Water Infrastructure Project"@en ;
                           rdfs:label "Infrastructure Project"@en ;
                           skos:altLabel "Infrastructure Project"@en ;
                           skos:definition "A project which is focused on the development, creation, maintenance, or enhancement of structures and systems needed for a country, city, or organization to function properly."@en ;
                           skos:example "PATH4ZERO"@en ,
                                        "Paving the way for Zero Emission Inland Navigation"@en ,
                                        "Power Edison Partnership"@en .


###  http://purl.org/holy/ns#InternationalOrganization
holy:InternationalOrganization rdf:type owl:Class ;
                               rdfs:subClassOf rov:RegisteredOrganization ;
                               dct:references <https://ec.europa.eu/eurostat/documents/3859598/5902521/KS-RA-07-015-EN.PDF> ;
                               rdfs:label "International Organization"@en ;
                               skos:altLabel "International Organization"@en ;
                               skos:definition """An organization classified in activities of international organisations such as the United Nations and the specialised agencies of the United Nations system, regional bodies etc., the International Monetary Fund, the World Bank, the World Customs Organisation, the Organisation for Economic Co-operation and Development, the organisation of Petroleum Exporting Countries, the European Communities, the European Free Trade Association etc. according to Section U of EC NACE Rev. 2.

This class also includes:
- activities of diplomatic and consular missions when being determined by the country of their location rather than by the country they represent"""@en ;
                               skos:example "IMF"@en ,
                                            "IPCC"@en ,
                                            "UNECE"@en ,
                                            "United Nations"@en .


###  http://purl.org/holy/ns#Investment
holy:Investment rdf:type owl:Class ;
                rdfs:subClassOf holy:Indicator ;
                wn:hyponym "Arbitrage"@en ,
                           "Leverage"@en ,
                           "Spendings"@en ;
                rdfs:label "Investment"@en ;
                skos:altLabel "Investing"@en ;
                skos:definition "The amount of money invested by an entity for something like a project, product or application."@en ;
                skos:hiddenLabel "IPO"@en ,
                                 "Initial Public Offering"@en .


###  http://purl.org/holy/ns#LithiumBattery
holy:LithiumBattery rdf:type owl:Class ;
                    rdfs:subClassOf holy:Battery ;
                    dct:references "https://doi.org/10.1016/B978-044452745-5.00185-4" ,
                                   "https://doi.org/10.1016/B978-044452745-5.00186-6" ;
                    wn:hyponym "Lithium Cathode Material"@en ,
                               "Lithium Ion Battery"@en ,
                               "Lithium Ion Battery Cell"@en ;
                    rdfs:label "Lithium Battery"@en ;
                    skos:altLabel "Lithium Battery"@en ;
                    skos:definition "A battery which uses lithium ions as a key component of its electrochemistry using liquid electrolyte solutions. It consists of two current collectors, a negative and positive electrode, and a separator containing electrolytes. The primary lithium battery uses carbon fluoride, (CF)n, as a cathode and lithium metal as an anode. The negative electrode consists of either metallic lithium or lithium compounds."@en ;
                    skos:example "Tesla Powerwall"@en ;
                    skos:hiddenLabel "Li Ion Battery"@en .


###  http://purl.org/holy/ns#LongHaulTruck
holy:LongHaulTruck rdf:type owl:Class ;
                   rdfs:subClassOf holy:Truck ;
                   dct:references <https://locus.sh/resources/glossary/long-haul-trucking/> ;
                   rdfs:label "Long Haul Truck"@en ;
                   skos:altLabel "Long Haul Truck"@en ,
                                 "Long-distance Truck"@en ;
                   skos:definition "A large road vehicle which is used for long-distance transporation over 250 miles."@en .


###  http://purl.org/holy/ns#ManufacturingOrganization
holy:ManufacturingOrganization rdf:type owl:Class ;
                               rdfs:subClassOf rov:RegisteredOrganization ;
                               dct:references <https://ec.europa.eu/eurostat/documents/3859598/5902521/KS-RA-07-015-EN.PD> ;
                               wn:hyponym "Automotive Manufacturer"@en ,
                                          "Car Maker"@en ,
                                          "Car Manufacturer"@en ,
                                          "OEM"@en ,
                                          "Original Equipment Manufacturer"@en ,
                                          "Solar Panel Maker"@en ;
                               rdfs:label "Manufacturing Organization"@en ;
                               skos:altLabel "Maker"@en ,
                                             "Manufacturer"@en ,
                                             "Manufacturing Company"@en ,
                                             "Producer"@en ;
                               skos:definition "An organization classified in the field of manufacturing according to EC NACE 2 (2008) in Section C Division 10-33."@en ;
                               skos:example "Arboc"@en ,
                                            "Arboc Speciality Vehicles"@en ,
                                            "Hyzon Motors Inc."@en ,
                                            "MCI"@en ,
                                            "Motor Coach Industries"@en ,
                                            "Plaxton"@en ,
                                            "Plug Power Inc."@en ,
                                            "Rivian Automotive Inc."@en ,
                                            "Subaru Corp."@en ,
                                            "Toyota Motor Corp."@en ;
                               skos:hiddenLabel "Hyundai Motor Group"@en ,
                                                "PLUG"@en ,
                                                "Plug Power"@en ,
                                                "Toyota Motor"@en .


###  http://purl.org/holy/ns#MarineApplication
holy:MarineApplication rdf:type owl:Class ;
                       rdfs:subClassOf holy:MobileApplication ;
                       dct:references <https://dictionary.cambridge.org/dictionary/english/marine> ;
                       wn:hyponym "Coastal"@en ,
                                  "Deep-sea vessel"@en ,
                                  "Electric Marine Vessel"@en ,
                                  "Marine Industry"@en ,
                                  "Naval"@en ,
                                  "Seagoing Vehicle"@en ,
                                  "Ship"@en ;
                       rdfs:label "Marine Application"@en ;
                       skos:altLabel "Marine Application"@en ,
                                     "Marine Usage"@en ,
                                     "Maritime Application"@en ,
                                     "Nautical Application"@en ;
                       skos:definition "An application related to sea transport of people and/or goods."@en ;
                       skos:hiddenLabel "Aquatic"@en ,
                                        "Maritime"@en ,
                                        "Nautical"@en ,
                                        "Oceanic Use"@en .


###  http://purl.org/holy/ns#MarketShare
holy:MarketShare rdf:type owl:Class ;
                 rdfs:subClassOf holy:Indicator ;
                 rdfs:label "Market Share"@en ;
                 skos:altLabel "Market Percentage"@en ,
                               "Market Share"@en ;
                 skos:definition "The total number of buyers a company has for a certain product or in a certain segment compared to the total market size."@en ;
                 skos:hiddenLabel "Market Leader"@en ,
                                  "Market Position"@en .


###  http://purl.org/holy/ns#MarketSize
holy:MarketSize rdf:type owl:Class ;
                rdfs:subClassOf holy:Indicator ;
                rdfs:label "Market Size"@en ;
                skos:altLabel "Market Capacity"@en ,
                              "Market Size"@en ,
                              "Market Volume"@en ;
                skos:definition "The total number of potential buyers of a product or service within a given market and the total revenue that these sales may generate."@en ;
                skos:hiddenLabel "Biggest Market"@en ,
                                 "Key Market"@en ,
                                 "Largest Market"@en ,
                                 "Major Market"@en ,
                                 "Overall Market"@en ,
                                 "Second Largest Market"@en ,
                                 "Total Market"@en .


###  http://purl.org/holy/ns#MaterialHandlingVehicle
holy:MaterialHandlingVehicle rdf:type owl:Class ;
                             rdfs:subClassOf holy:RoadApplication ;
                             dct:references <https://www.mhi.org/fundamentals/material-handling> ;
                             wn:hyponym "AGV"@en ,
                                        "Automated Guided Vehicle"@en ,
                                        "Forklift"@en ,
                                        "Jitney"@en ,
                                        "Lift Truck"@en ,
                                        "Man Up Orderpicker"@en ,
                                        "Stand Up Counterbalanced Truck"@en ,
                                        "Stand Up reach Truck"@en ,
                                        "Turret Truck"@en ;
                             rdfs:label "Material Handling Vehicle"@en ;
                             skos:altLabel "Material Handling Equipment"@en ,
                                           "Material Handling Vehicle"@en ,
                                           "Warehouse Vehicle"@en ;
                             skos:definition "Vehicles which are intended to be used in a mobile context within the material handling process of organizations or private persons."@en ;
                             skos:hiddenLabel "Material Handling"@en ,
                                              "On-site Transportation"@en ,
                                              "Warehouse Logistics"@en .


###  http://purl.org/holy/ns#Membrane
holy:Membrane rdf:type owl:Class ;
              rdfs:subClassOf holy:MembraneElectrodeAssembly ;
              dct:references <https://www.energy.gov/eere/fuelcells/parts-fuel-cell> ,
                             "https://doi.org/10.1016/B978-044452745-5.00227-6" ;
              rdfs:label "Membrane"@en ;
              skos:altLabel "CE Membrane"@en ,
                            "Cation Exchange Membrane"@en ,
                            "PEM"@en ,
                            "PEM membrane"@en ,
                            "PFSA"@en ,
                            "PFSA based proton exchange membrane"@en ,
                            "PFSA membrane"@en ,
                            "Perfluorosulfonic Acid Membrane"@en ,
                            "Polymer Electrolyte Membrane"@de ,
                            "Proton Exchange Membrane"@en ,
                            "Proton Exchange Membrane Electrolyzer"@en ;
              skos:definition "A very thin membrane which conducts solely positively-charged ions and is able to block electrons. It serves as the electrolyte."@en .


###  http://purl.org/holy/ns#MembraneElectrodeAssembly
holy:MembraneElectrodeAssembly rdf:type owl:Class ;
                               rdfs:subClassOf holy:FuelCellStack ;
                               dct:references <https://www.energy.gov/eere/fuelcells/parts-fuel-cell> ,
                                              "https://doi.org/10.1016/B978-044452745-5.00227-6" ;
                               rdfs:label "Membrane Electrode Assembly"@en ;
                               skos:altLabel "Bipolar Membrane Electrode Assembly"@en ,
                                             "MEA"@en ,
                                             "Membrane Electrode Assembly"@en ;
                               skos:definition "The heart of the fuel cell and the place where the chemical reaction takes place. It consists of membrane, catalyst layers, and gas diffusion layers."@en .


###  http://purl.org/holy/ns#MethanolFuelCell
holy:MethanolFuelCell rdf:type owl:Class ;
                      rdfs:subClassOf holy:SubstituteFuelCell ;
                      dct:references <https://www.energy.gov/eere/fuelcells/types-fuel-cells> ,
                                     <https://www.fuelcellstore.com/blog-section/alternative-liquid-fuel-types-fuel-cells> ;
                      wn:hyponym "Direct Methanol Fuel Cell"@en ;
                      rdfs:label "Methanol Fuel Cell"@en ;
                      skos:altLabel "DMFC"@en ,
                                    "Methanol Fuel Cell"@en ;
                      skos:definition "A fuel cell which is powered by pure methanol. It is usually mixed with water and fed directly to the fuel cell anode."@en ;
                      skos:example "EFYO 150"@en ,
                                   "EFYO 80"@en .


###  http://purl.org/holy/ns#MobileApplication
holy:MobileApplication rdf:type owl:Class ;
                       rdfs:subClassOf holy:Application ;
                       dct:references <https://dictionary.cambridge.org/dictionary/english/mobile> ;
                       wn:hyponym "Cargo Transport"@en ,
                                  "Clean Transport"@en ,
                                  "Freight Transport"@en ,
                                  "Long-distance Transportation Unit"@en ,
                                  "Long-distance Travel"@en ,
                                  "Motorized Item"@en ,
                                  "Portable Fuel Cell Application"@en ,
                                  "Short-distance Transportation Unit"@en ,
                                  "Transportation Vehicle"@en ;
                       rdfs:label "Mobile Application"@en ;
                       skos:altLabel "Moving Application"@en ,
                                     "Transportation"@en ,
                                     "Mobile Application" ;
                       skos:definition "An application related to the movement of people and/or goods."@en ;
                       skos:hiddenLabel "Unstationary"@en .


###  http://purl.org/holy/ns#MoltenCarbonateFuelCell
holy:MoltenCarbonateFuelCell rdf:type owl:Class ;
                             rdfs:subClassOf holy:SubstituteFuelCell ;
                             dct:references <https://www.energy.gov/eere/fuelcells/types-fuel-cells> ,
                                            <https://www.tuev-nord.de/en/company/energy/hydrogen/hydrogen-fuel-cell/> ;
                             rdfs:label "Molten Carbonate Fuel Cell"@en ;
                             skos:altLabel "MCFC"@en ,
                                           "Molten Carbonate Fuel Cell"@en ;
                             skos:definition "A high temperature fuel cell using natural gas or biogas for powering. The fuel cell itself is able to convert hydrogen in a process called internal reforming."@en .


###  http://purl.org/holy/ns#NickelCadmiumBattery
holy:NickelCadmiumBattery rdf:type owl:Class ;
                          rdfs:subClassOf holy:Battery ;
                          dct:references "https://doi.org/10.1016/B978-0-12-813975-2.00005-3" ;
                          rdfs:label "Nickel Cadmium Battery"@en ;
                          skos:altLabel "Nickel Cadmium Battery"@en ;
                          skos:definition "A battery which uses nickel oxide hydroxide for the cathode, metallic cadmium as its anode, and an aqueous alkali solution as its electrolyte."@en .


###  http://purl.org/holy/ns#NickelMetalHydrideBattery
holy:NickelMetalHydrideBattery rdf:type owl:Class ;
                               rdfs:subClassOf holy:Battery ;
                               dct:references "https://doi.org/10.1016/B978-044452745-5.00158-1" ;
                               rdfs:label "Nickel Metal Hydride Battery"@en ;
                               skos:altLabel "Nickel Metal Hydride Battery"@en ;
                               skos:definition "A battery which uses nickel oxide for the cathode. The negative active material is hydrogen in form of a metal hydride. The electrolyte is aqueous potassium hydroxide with lithium hydroxide additive to improve the charging efficiency of the positive electrode by reducing oxygen evolution."@en .


###  http://purl.org/holy/ns#OngoingProject
holy:OngoingProject rdf:type owl:Class ;
                    rdfs:subClassOf holy:StateBasedProject ;
                    dct:references <https://www.referenceforbusiness.com/management/Pr-Sa/Project-Management.html> ;
                    rdfs:label "Ongoing Project"@en ;
                    skos:altLabel "Currently Running Project"@en ,
                                  "Currently Running Venture"@en ;
                    skos:definition "A currently-running project which has been started but is not marked as finished or completed."@en .


###  http://purl.org/holy/ns#PassengerTrain
holy:PassengerTrain rdf:type owl:Class ;
                    rdfs:subClassOf holy:Train ;
                    dct:references <https://dictionary.cambridge.org/dictionary/english/passenger?q=passenger+train> ;
                    wn:hyponym "Bullet Train"@en ,
                               "High-speed Train"@en ,
                               "Light Rail"@en ,
                               "Tram"@en ;
                    rdfs:label "Passenger Train"@en ;
                    skos:altLabel "Coach Train"@en ,
                                  "Commuter Train"@en ,
                                  "Passenger Train"@en ;
                    skos:definition "A train carrying mostly people."@en .


###  http://purl.org/holy/ns#Patent
holy:Patent rdf:type owl:Class ;
            rdfs:subClassOf holy:Indicator ;
            rdfs:label "Patent"@en ;
            skos:definition "The total number of patents attributed to a class individual."@en ;
            skos:hiddenLabel "Copyright"@en ,
                             "Intellectual Property"@en ,
                             "Trademark"@en .


###  http://purl.org/holy/ns#PhosphoricAcidFuelCell
holy:PhosphoricAcidFuelCell rdf:type owl:Class ;
                            rdfs:subClassOf holy:HydrogenReconversion ;
                            dct:references <https://www.energy.gov/eere/fuelcells/types-fuel-cells> ,
                                           <https://www.tuev-nord.de/en/company/energy/hydrogen/hydrogen-fuel-cell/> ;
                            rdfs:label "Phosphoric Acid Fuel Cell"@en ;
                            skos:altLabel "PAFC"@en ,
                                          "Phosphoric Acid Fuel Cell"@en ;
                            skos:definition "A fuel cell which uses phosporic acid as an electrolyte. It can be powered by hydrogen, natural gas, or biogas."@en .


###  http://purl.org/holy/ns#PickupTruck
holy:PickupTruck rdf:type owl:Class ;
                 rdfs:subClassOf holy:Truck ;
                 dct:references <https://dictionary.cambridge.org/dictionary/english/pickup-truck> ;
                 rdfs:label "Pickup Truck"@en ;
                 skos:altLabel "Pickup Truck"@en ;
                 skos:definition "A small vehicle with an open part at the back in which goods can be carried."@en ;
                 skos:hiddenLabel "Pick-up"@en ,
                                  "Pickup"@en .


###  http://purl.org/holy/ns#PlannedProject
holy:PlannedProject rdf:type owl:Class ;
                    rdfs:subClassOf holy:StateBasedProject ;
                    dct:references <https://www.referenceforbusiness.com/management/Pr-Sa/Project-Management.html> ;
                    rdfs:label "Planned Project"@en ;
                    skos:definition "A project which has not been realised or started but is expected to start in the future."@en .


###  http://purl.org/holy/ns#PolymerElectrolyteMembraneFuelCell
holy:PolymerElectrolyteMembraneFuelCell rdf:type owl:Class ;
                                        rdfs:subClassOf holy:HydrogenReconversion ;
                                        dct:references <https://www.energy.gov/eere/fuelcells/types-fuel-cells> ;
                                        wn:hyponym "High Temperature PEMFC"@en ,
                                                   "High Temperature Proton Exchange Membrane Fuel Cel"@en ,
                                                   "Low Temperature PEMFC"@en ,
                                                   "Low Temperature Proton Exchange Membrane Fuel Cel"@en ,
                                                   "PEMFC module"@en ;
                                        rdfs:label "Polymer Electrolyte Membrane Fuel Cell"@en ;
                                        skos:altLabel "Electrolyte Fuel Cell"@en ,
                                                      "Exchange Membrane Fuel Cell"@en ,
                                                      "PEFC"@en ,
                                                      "PEM Fuel Cell"@en ,
                                                      "PEMFC"@en ,
                                                      "Polymer Elektrolyt Membrane Fuel Cell"@en ,
                                                      "Polymer Elektrolyte Fuel Cell"@en ;
                                        skos:definition "A fuel cell which uses a solid polymer as an electrolyte and porous carbon electrodes containing a platinum or platinum alloy catalyst. It only needs hydrogen, oxygen from the air, and water to operate."@en ;
                                        skos:example "FCmoveTM"@en ,
                                                     "FCwaveTM"@en ;
                                        skos:hiddenLabel "Fuel Cell Power Product"@en .


###  http://purl.org/holy/ns#PowerConditioner
holy:PowerConditioner rdf:type owl:Class ;
                      rdfs:subClassOf holy:HydrogenFuelCellComponent ;
                      dct:references <https://www.energy.gov/eere/fuelcells/fuel-cell-systems> ;
                      wn:hyponym "AVR"@en ,
                                 "Automatic Voltage Regulator"@en ,
                                 "Electrical Grid Stabilization"@en ,
                                 "UPS System"@en ,
                                 "Uninterruptible Power Supply System"@en ,
                                 "VRM"@en ,
                                 "Voltage Regulator Module"@en ;
                      rdfs:label "Power Conditioner"@en ;
                      skos:altLabel "Power Conditioner"@en ;
                      skos:definition "An electrical current regulator needed for managing power."@en ;
                      skos:hiddenLabel "FCCU"@en ,
                                       "Fuel Cell Control Unit"@en .


###  http://purl.org/holy/ns#PowerGeneration
holy:PowerGeneration rdf:type owl:Class ;
                     rdfs:subClassOf holy:StationaryApplication ;
                     dct:references <https://www.cummins.com/generators/power-generation> ;
                     wn:hyponym "Backup Generator"@en ,
                                "Backup Power"@en ,
                                "Clean Energy Production"@en ,
                                "Coal Power Station"@en ,
                                "Coal-fired Power"@en ,
                                "Fossil Fuel Electricity"@en ,
                                "Fuel Flex Generator"@en ,
                                "Fuel Flexible Power Generator"@en ,
                                "Grid Scale Energy Storage"@en ,
                                "H2 Gas Turbine"@en ,
                                "Hydrogen Fuel Cell Power Plant"@en ,
                                "Industrial Power Generation"@en ,
                                "Local Energy Generation"@en ,
                                "Power Plant"@en ,
                                "Power Plant Generator"@en ,
                                "Renewable Energy Generation"@en ,
                                "Renewable Energy Production"@en ,
                                "Residential Power Generation"@en ,
                                "Small-scale Power Grid"@en ,
                                "Solar Electricity"@en ,
                                "Solar Energy"@en ,
                                "Solar Farm"@en ,
                                "Solar Generation"@en ;
                     rdfs:label "Power Generation"@en ;
                     skos:definition "An application which is used in the field of electricity production via power generating equipment or as fuel."@en .


###  http://purl.org/holy/ns#Product
holy:Product rdf:type owl:Class ;
             dct:references <https://www.iedunote.com/types-of-products> ;
             wn:hyponym "Product Article"@en ;
             rdfs:comment "The connection to \"Application\" would refer to \"realized usage\". A product has a creator. However, since technology and product are difficult to distinguish, technology and product will be seen as one class. Since organizations can also buy component parts, the product class has sub-classes containing components for fuel cells."@en ;
             rdfs:label "Product"@en ;
             skos:altLabel "Product"@en ;
             skos:definition "An article that is manufactured or refined for sale. A distinction will be made between the different value chain positions of a product which can be sold and/or bought."@en ;
             skos:hiddenLabel "Alternative Energy Technology"@en ,
                              "Green Tech"@en ,
                              "Homegrown Technology"@en ,
                              "Renewable Fuel"@en ,
                              "Technology"@en .


###  http://purl.org/holy/ns#ProductDevelopmentProject
holy:ProductDevelopmentProject rdf:type owl:Class ;
                               rdfs:subClassOf holy:PurposeBasedProject ;
                               wn:hyponym "Battery Storage Project"@en ,
                                          "Breakthrough Project"@en ,
                                          "Enhacement Project"@en ,
                                          "Hybrid  Project"@en ;
                               rdfs:label "Product Development Project"@en ;
                               skos:altLabel "Product Design Project"@en ,
                                             "Product Development Project"@en ;
                               skos:definition "A project focused on the development of new products or the refinement of existing ones."@en ;
                               skos:hiddenLabel "Product Development Cooperation"@en .


###  http://purl.org/holy/ns#PublicAdministrationAndDefenseOrganization
holy:PublicAdministrationAndDefenseOrganization rdf:type owl:Class ;
                                                rdfs:subClassOf rov:RegisteredOrganization ;
                                                dct:references <https://ec.europa.eu/eurostat/documents/3859598/5902521/KS-RA-07-015-EN.PDF> ;
                                                rdfs:label "Public Administration and Defense Organization"@en ;
                                                skos:altLabel "Public Administration Office"@en ;
                                                skos:definition "An organization classified in the field of public administration and defense according to EC NACE 2 (2008) in Section O Division 84."@en ;
                                                skos:example "DARPA"@en ,
                                                             "Defense Advanced Research Projects Agency"@en .


###  http://purl.org/holy/ns#PurposeBasedProject
holy:PurposeBasedProject rdf:type owl:Class ;
                         rdfs:subClassOf schema:Project ;
                         dct:references <http://www.maxwideman.com/guests/typology/projects.htm> ,
                                        <https://docs.oracle.com/cd/E18727_01/doc.121/e13567/T237204T237210.htm> ,
                                        <https://t2informatik.de/en/smartpedia/project-type/> ;
                         rdfs:label "Purpose-based Project"@en ;
                         skos:definition "A project classification defined during implementation that specifies essential project attributes and purpose."@en .


###  http://purl.org/holy/ns#RefineryIndustrialProcessing
holy:RefineryIndustrialProcessing rdf:type owl:Class ;
                                  rdfs:subClassOf holy:IndustrialProcessing ;
                                  dct:references <https://www.sciencedirect.com/topics/earth-and-planetary-sciences/refining-industry> ;
                                  wn:hyponym "Hydrocracking"@en ,
                                             "Hydrogenation"@en ,
                                             "Hydrogenolysis"@en ,
                                             "Petroleum Production"@en ,
                                             "Petroleum Refining"@en ;
                                  rdfs:label "Refinery Industrial Processing"@en ;
                                  skos:altLabel "Refining Process"@en ;
                                  skos:definition "Applications of hydrogen in the refinery industry dedicated to process oil to create different types of oil and oil products."@en ;
                                  skos:hiddenLabel "Petrochemical Market"@en .


###  http://purl.org/holy/ns#RegionalTruck
holy:RegionalTruck rdf:type owl:Class ;
                   rdfs:subClassOf holy:Truck ;
                   dct:references <https://www.azuga.com/blog/what-is-a-short-haul-truck-driver> ;
                   wn:hyponym "All-electric Van"@en ,
                              "Box Truck"@en ,
                              "Garbage Truck"@en ,
                              "Hydrogen-powered Van"@en ,
                              "Medium Duty Truck"@en ,
                              "Refuse Truck"@en ,
                              "Straught Truck"@en ;
                   rdfs:label "Regional Truck"@en ;
                   skos:altLabel "Regional Truck"@en ;
                   skos:definition "A road vehicle which is small to large-sized and used for the transportation of goods within an area of 150 miles."@en ;
                   skos:hiddenLabel "Van"@en .


###  http://purl.org/holy/ns#ResearchOrganization
holy:ResearchOrganization rdf:type owl:Class ;
                          rdfs:subClassOf rov:RegisteredOrganization ;
                          dct:references <https://ec.europa.eu/eurostat/documents/3859598/5902521/KS-RA-07-015-EN.PDF> ;
                          wn:hyponym "Professional Scientific And Technical Activity"@en ,
                                     "Technical Testing and Analysis"@en ,
                                     "University"@en ,
                                     "University of Applied Sciences"@en ;
                          rdfs:label "Research Organization"@en ;
                          skos:altLabel "Research Institution"@en ,
                                        "Research Organization"@en ,
                                        "Research and Development Center"@en ;
                          skos:definition "Organizations classified in the field of scientific and technical activities according to EC NACE 2 (2008) in Section M Division 69-75."@en ;
                          skos:example "MARii"@en ,
                                       "Malaysia Automotive Robotics and IoT Institute"@en ,
                                       "PNNL"@en ,
                                       "Pacific Northwest National Laboratory"@en ,
                                       "The European Interoperability Centre for Electric Vehicles and Smart Grids"@en ;
                          skos:hiddenLabel "ISIC 7120"@en ,
                                           "NACE 71.20"@en ,
                                           "Scientific Research and Development"@en .


###  http://purl.org/holy/ns#ResidentialHeating
holy:ResidentialHeating rdf:type owl:Class ;
                        rdfs:subClassOf holy:Heating ;
                        dct:references <https://www.boilerguide.co.uk/articles/hydrogen-boilers-alternative-gas-central-heating> ;
                        wn:hyponym "Combined Heat and Power station"@en ,
                                   "Fuel Cell Boiler"@en ,
                                   "Fuel Cell CHP"@en ,
                                   "Fuel Cell Heater"@en ,
                                   "Fuel-Cell Boiler"@en ,
                                   "Fuel-cell Heating System"@en ,
                                   "Gas Boiler"@en ,
                                   "Heat and Power Station"@en ,
                                   "Heat and Power Unit"@en ,
                                   "PEM Fuel Cell Boiler"@en ,
                                   "PEM Fuel Cell Heater"@en ,
                                   "PEM Heater"@en ,
                                   "Polymer Electrolyte Membrane Fuel Cell Boiler"@en ,
                                   "Polymer Electrolyte Membrane Fuel Cell Heater"@en ,
                                   "Residential Fuel Cell System"@en ;
                        rdfs:label "Residential Heating"@en ;
                        skos:altLabel "Apartment Heating"@en ,
                                      "Domestic Heating"@en ,
                                      "Home Heating"@en ,
                                      "Residential Heating"@en ;
                        skos:definition "Applications used for heating a domestic house or residential area (multiple domestic houses)."@en ;
                        skos:hiddenLabel "Boiler"@en ,
                                         "CHP"@en ,
                                         "Furnace"@en ,
                                         "Radiant"@en .


###  http://purl.org/holy/ns#Revenue
holy:Revenue rdf:type owl:Class ;
             rdfs:subClassOf holy:Indicator ;
             wn:hyponym "Total Sales"@en ;
             rdfs:label "Revenue"@en ;
             skos:altLabel "Earning"@en ,
                           "Gross Revenue"@en ,
                           "Income"@en ,
                           "Sales"@en ;
             skos:definition "The amount of money generated within a certain class in a certain period of time."@en ;
             skos:hiddenLabel "Absolute Sales"@en .


###  http://purl.org/holy/ns#RoadApplication
holy:RoadApplication rdf:type owl:Class ;
                     rdfs:subClassOf holy:MobileApplication ;
                     dct:references <https://www.marineinsight.com/types-of-ships/what-are-cargo-ships/> ;
                     wn:hyponym "BEV"@en ,
                                "Battery Electric Vehicle"@en ,
                                "EV"@en ,
                                "EVIC"@en ,
                                "EVs"@en ,
                                "Electric Vehicle"@en ,
                                "Electrical Vehicle"@en ,
                                "Energy Efficient Vehicle"@en ,
                                "Ethanol Hybrid Vehicle"@en ,
                                "Ethanol ICE Vehicles"@en ,
                                "FCVs"@en ,
                                "Flex Ethanol Hybrids"@en ,
                                "Flex Fuel Vehicle"@en ,
                                "Fuel Cell Vehicle"@en ,
                                "H2ICE"@en ,
                                "HFCEVs"@en ,
                                "Highway Usage"@en ,
                                "Hydrogen Fuel Cell Electric Vehicles"@en ,
                                "Hydrogen Fuel Cell Vehicle"@en ,
                                "Hydrogen ICE vehicle"@en ,
                                "ICE vehicle"@en ,
                                "Internal Combustion Engine Vehicle"@en ,
                                "Long-distance Vehicle"@en ,
                                "Passenger Electric"@en ,
                                "Passenger Electric Vehicle"@en ,
                                "Personal Vehicle"@en ,
                                "Ultra clean vehicle"@en ,
                                "ZEV"@en ,
                                "Zero-emission Vehicle"@en ;
                     rdfs:label "Road Application"@en ;
                     skos:altLabel "Hydrogen Internal Combustion Engine Vehicle"@en ,
                                   "Road Usage"@en ,
                                   "Vehicle"@en ;
                     skos:definition "An application related to the transport of people and/or goods on land."@en ;
                     skos:example "Ballard Powered Vehicle"@en .


###  http://purl.org/holy/ns#SolidOxideFuelCell
holy:SolidOxideFuelCell rdf:type owl:Class ;
                        rdfs:subClassOf holy:HydrogenReconversion ;
                        dct:references <https://onlinelibrary.wiley.com/doi/full/10.1002/fuce.202070602> ;
                        wn:hyponym "High Temperature Fuel Cell Gasket"@en ;
                        rdfs:comment "Caution, SOFC`s must not be mixed up with SOEC's (Solid Oxide Electrolyser). SOFC`s are fuel cells using hydrogen as a fuel to generate energy. SOEC's are used for hydrogen generation using the reversed process of an SOFC. For this ontology an SOEC would be a part of the conversion class. However, since conversion is out of scope, SOEC are not mentioned in a class structure under the subclass \"Conversion\"."@en ;
                        rdfs:label "Solid Oxide Fuel Cell"@en ;
                        skos:altLabel "SOFC"@en ,
                                      "Solid Oxide Fuel Cell"@en ;
                        skos:definition "A fuel cell which uses a hard, non-porous ceramic compound as the electrolyte. It can reach temperatures up to 1000°C (1830°F). It can be powered by natural gas, coal gas, biogas or hydrogen."@en .


###  http://purl.org/holy/ns#SolidStateBattery
holy:SolidStateBattery rdf:type owl:Class ;
                       rdfs:subClassOf holy:Battery ;
                       dct:references <https://www.samsungsdi.com/column/technology/detail/56462.html?listType=gallery> ;
                       rdfs:label "Solid State Battery"@en ;
                       skos:altLabel "Solid State Battery"@en ,
                                     "Solid State Battery Technology"@en ;
                       skos:definition "A battery which uses solid lithium as an electrolyte, not liquid."@en .


###  http://purl.org/holy/ns#Spacecraft
holy:Spacecraft rdf:type owl:Class ;
                rdfs:subClassOf holy:AviaticApplication ;
                dct:references <http://wordnetweb.princeton.edu/perl/webwn?s=spacecraft&sub=Search+WordNet&o2=&o0=1&o8=1&o1=1&o7=&o5=&o9=&o6=&o3=&o4=&h=000000000> ,
                               <https://dictionary.cambridge.org/dictionary/english/spacecraft> ;
                rdfs:label "Spacecraft"@en ;
                skos:altLabel "Rocketship"@en ,
                              "Satellite Launcher"@en ,
                              "Space Capsule"@en ,
                              "Space Shuttle"@en ,
                              "Space Vehicle"@en ,
                              "Spacecraft"@en ,
                              "Spaceship"@en ;
                skos:definition "A vehicle designed for use and travel in space."@en ;
                skos:hiddenLabel "Rocket"@en ,
                                 "Satellite"@en ,
                                 "Shuttle"@en .


###  http://purl.org/holy/ns#StateBasedProject
holy:StateBasedProject rdf:type owl:Class ;
                       rdfs:subClassOf schema:Project ;
                       dct:references <https://www.referenceforbusiness.com/management/Pr-Sa/Project-Management.html> ;
                       rdfs:label "State-based Project"@en ;
                       skos:altLabel "State Based Project"@en ;
                       skos:definition "State Based Project as a subclass of Project defines the level of progress for a project. It can be categorized according to the temporary stage such as planned, ongoing or finished."@en .


###  http://purl.org/holy/ns#StationaryApplication
holy:StationaryApplication rdf:type owl:Class ;
                           rdfs:subClassOf holy:Application ;
                           dct:references <http://www.chfca.ca/fuel-cells-hydrogen/hydrogen-fuel-cell-applications/> ;
                           wn:hyponym "Charging Station"@en ,
                                      "Charging System"@en ,
                                      "Charging hub"@en ,
                                      "Clean Energy Storage"@en ,
                                      "EV Charger"@en ,
                                      "Electric Vehicle Charger"@en ,
                                      "Electric Vehicle Charging Hub"@en ,
                                      "Energy Storage Solution"@en ,
                                      "Grid Scale Energy Storage"@en ,
                                      "Hydrogen Electrolyser"@en ,
                                      "Hydrogen Fueling Station"@en ,
                                      "Hydrogen Station"@en ,
                                      "Hydrogen Vehicle Refueling Station"@en ,
                                      "Mobile Energy Storage Solution"@en ,
                                      "Stationary Fuel Cell Application"@en ,
                                      "Vehicle Charging Hub"@en ;
                           rdfs:label "Stationary Application"@en ;
                           skos:altLabel "Immobile"@en ,
                                         "Stationary Application"@en ,
                                         "Stationary Unit"@en ;
                           skos:definition "An application which is intended to be placed at one location without the possibility of physically being moved when used."@en ;
                           skos:hiddenLabel "Fast Charger"@en ,
                                            "Heavy Industry"@en ,
                                            "Heavy Machine"@en ,
                                            "Stationary Sector"@en .


###  http://purl.org/holy/ns#SteelIndustrialProcessing
holy:SteelIndustrialProcessing rdf:type owl:Class ;
                               rdfs:subClassOf holy:IndustrialProcessing ;
                               dct:references <https://www.infoplease.com/encyclopedia/social-science/economy/business/steel-industry> ;
                               wn:hyponym "AHW"@en ,
                                          "Atomic Hydrogen Welding"@en ,
                                          "EAF"@en ,
                                          "Electric Arc Furnace"@en ,
                                          "Iron Flashmaking"@en ,
                                          "Metal Alloying"@en ,
                                          "Metal Purification"@en ;
                               rdfs:label "Steel Industrial Processing"@en ;
                               skos:altLabel "Steel Fabrication"@en ,
                                             "Steel Manufacturing"@en ,
                                             "Steel Production"@en ;
                               skos:definition "Applications of hydrogen or hydrogen products in the steel industry with respect to the processing of iron ore into certain types of steel."@en .


###  http://purl.org/holy/ns#Submarine
holy:Submarine rdf:type owl:Class ;
               rdfs:subClassOf holy:MarineApplication ;
               dct:references <https://dictionary.cambridge.org/dictionary/english/submarine> ;
               rdfs:label "Submarine"@en ;
               skos:altLabel "Steel Sub"@en ,
                             "Submersible"@en ,
                             "U-boat"@en ,
                             "Underwater Craft"@en ;
               skos:definition "A ship that can travel underwater."@en .


###  http://purl.org/holy/ns#SubstituteFuelCell
holy:SubstituteFuelCell rdf:type owl:Class ;
                        rdfs:subClassOf holy:SubstituteProduct ;
                        dct:references <https://www.fuelcellstore.com/blog-section/alternative-liquid-fuel-types-fuel-cells> ;
                        rdfs:comment "The subclass \"SubstituteFuelCell\" could be expanded to focus the domain scope to the creation of hydrogen concerning the value chain."@en ;
                        rdfs:label "Substitute Fuel Cell"@en ;
                        skos:definition "A fuel cell which uses different resources as its anode gas than hydrogen."@en .


###  http://purl.org/holy/ns#SubstituteFuelCellComponent
holy:SubstituteFuelCellComponent rdf:type owl:Class ;
                                 rdfs:subClassOf holy:SubstituteProductComponent ;
                                 rdfs:comment "The subclass \"Substitute Fuel Cell Component\" could be expanded to focus on substitute fuel cells. "@en ;
                                 rdfs:label "Substitute Fuel Cell Component"@en ;
                                 skos:definition "A basic component for substitute fuel cells."@en .


###  http://purl.org/holy/ns#SubstituteProduct
holy:SubstituteProduct rdf:type owl:Class ;
                       rdfs:subClassOf holy:Product ;
                       rdfs:comment "For the domain scope, Substitute Product currently only defines products which are substitutes for hydrogen fuel cells."@en ,
                                    "The subclass \"Substitute Product\" could be expanded to focus the domain scope."@en ;
                       rdfs:label "Substitute Product"@en ;
                       skos:definition "A product that is manufactured or refined for sale which is using other resources than hydrogen to fulfill its purpose."@en .


###  http://purl.org/holy/ns#SubstituteProductComponent
holy:SubstituteProductComponent rdf:type owl:Class ;
                                rdfs:subClassOf holy:Product ;
                                dct:references <https://dictionary.cambridge.org/dictionary/english/component> ;
                                rdfs:comment "The subclass \"Substitute Product Component\" could be expanded to focus on substitute products of hydrogen products."@en ;
                                rdfs:label "Substitute Product Component"@en ;
                                skos:definition "A part that combined with other parts make a product which is a substitute to hydrogen products."@en .


###  http://purl.org/holy/ns#SupportiveHardware
holy:SupportiveHardware rdf:type owl:Class ;
                        rdfs:subClassOf holy:FuelCellStack ;
                        dct:references <https://dictionary.cambridge.org/dictionary/english/hardware> ,
                                       <https://www.energy.gov/eere/fuelcells/parts-fuel-cell> ;
                        rdfs:label "Supportive Hardware"@en ;
                        skos:altLabel "Supportive Hardware"@en ;
                        skos:definition "A component such as equipment, material, or metal which enables efficient energy generation."@en .


###  http://purl.org/holy/ns#Train
holy:Train rdf:type owl:Class ;
           rdfs:subClassOf holy:RoadApplication ;
           dct:references <https://dictionary.cambridge.org/dictionary/english/train> ;
           wn:hyponym "Ammonia Powered Locomotive"@en ,
                      "Hydrogen Fuel Cell-powered Train"@en ,
                      "Hydrogen-powered Train"@en ,
                      "Powertrain"@en ;
           rdfs:label "Train"@en ;
           skos:altLabel "Railroad Train"@en ,
                         "Train"@en ;
           skos:definition "A vehicle for roads made of railways using an engine and carriages to transport people or goods."@en ;
           skos:hiddenLabel "Rail"@en .


###  http://purl.org/holy/ns#TransportationAndStorageOrganization
holy:TransportationAndStorageOrganization rdf:type owl:Class ;
                                          rdfs:subClassOf rov:RegisteredOrganization ;
                                          dct:references <https://ec.europa.eu/eurostat/documents/3859598/5902521/KS-RA-07-015-EN.PDF> ;
                                          rdfs:label "Transportation And Storage Organization"@en ;
                                          skos:definition "An organization classified in the field of transportation and storage according to EC NACE 2 (2008) in Section H Division 49-53."@en ;
                                          skos:example "TC Energy"@en .


###  http://purl.org/holy/ns#Trend
holy:Trend rdf:type owl:Class ;
           rdfs:subClassOf holy:Indicator ;
           wn:hyponym "Clean Energy Megatrend"@en ,
                      "European Mobility Expo"@en ,
                      "Hydrogen Adoption"@en ,
                      "Hydrogen Economy Area"@en ;
           rdfs:label "Trend"@en ;
           skos:definition "A general development or change of a situation in terms of behavior which can manifest itself in being discussed in forums, conferences or expos."@en ;
           skos:example "Hydrogen Impact 2021 Conference"@en ,
                        "Hydrogen Technology Expo Europe"@en ,
                        "Hydrogen Transition Summit"@en ,
                        "POWERGEN International"@en ,
                        "The Automotive & Tire Industry Forum"@en ,
                        "The COP 26 Climate Summit"@en ,
                        "The China International Import Expo"@en ,
                        "The LA Auto Show"@en ,
                        "The World Climate Conference"@en ,
                        "United Nations Conference on Climate Change"@en ;
           skos:hiddenLabel "Forum Tomorrow in Motion"@en ,
                            "Green Car Korea"@en .


###  http://purl.org/holy/ns#Truck
holy:Truck rdf:type owl:Class ;
           rdfs:subClassOf holy:RoadApplication ;
           dct:references <https://dictionary.cambridge.org/dictionary/english/truck> ;
           wn:hyponym "Battery Electric Semi Truck"@en ,
                      "Clean Truck"@en ,
                      "Electric Truck"@en ,
                      "HFCET"@en ,
                      "Heavy Duty Truck"@en ,
                      "Heavy Hydrogen Truck"@en ,
                      "Heavy Truck"@en ,
                      "Hydrogen Fuel Cell Electric Truck"@en ,
                      "Hydrogen Mining Truck"@en ,
                      "Hydrogen Road Truck"@en ,
                      "Hydrogen-fueled Tractor Unit"@en ,
                      "LGV"@en ,
                      "Large Goods Vehicle"@en ,
                      "Logistic Truck"@en ,
                      "Logistic Vehicle"@en ,
                      "Road Truck"@en ;
           rdfs:comment "Trucks are categorized in this ontology by distance and not by categories such as size or transportation limit."@en ;
           rdfs:label "Truck"@en ;
           skos:altLabel "Truck"@en ;
           skos:definition "A large road vehicle that is used for transporting large amounts of goods."@en ;
           skos:hiddenLabel "LT Truck"@en ,
                            "LVS"@en ,
                            "Tractor"@en .


###  http://purl.org/holy/ns#WorkForce
holy:WorkForce rdf:type owl:Class ;
               rdfs:subClassOf holy:Indicator ;
               wn:hyponym "Employee"@en ,
                          "Worker"@en ;
               rdfs:label "Work Force"@en ;
               skos:altLabel "Labor Force"@en ,
                             "Workforce"@en ;
               skos:definition "The number of persons working for an organization."@en ;
               skos:hiddenLabel "Labor"@en .


###  http://schema.org/Continent
schema:Continent rdf:type owl:Class ;
                 rdfs:subClassOf holy:GeographicMarket ,
                                 [ rdf:type owl:Restriction ;
                                   owl:onProperty dbo:continent ;
                                   owl:allValuesFrom schema:Continent
                                 ] ;
                 dct:references schema: ;
                 rdfs:label "Continent"@en ;
                 skos:definition "One of the seven large land masses on the earth's surface, surrounded, or mainly surrounded, by sea and usually consisting of various countries."@en .


###  http://schema.org/Country
schema:Country rdf:type owl:Class ;
               rdfs:subClassOf holy:GeographicMarket ;
               dct:references schema: ;
               rdfs:label "Country"@en ;
               skos:definition "An area of land that has its own government, army, etc."@en .


###  http://schema.org/Project
schema:Project rdf:type owl:Class ;
               dct:references schema: ,
                              <http://www.maxwideman.com/guests/typology/projects.htm> ,
                              <https://dictionary.cambridge.org/dictionary/english/project> ,
                              <https://www.referenceforbusiness.com/management/Pr-Sa/Project-Management.html> ;
               wn:hyponym "Alliance Project"@en ,
                          "Hydrogen Project"@en ,
                          "Partnered Project"@en ;
               rdfs:comment "A project can be defined as a piece of planned work consisting of interrelated activities which intends to fulfill a particular purpose within a certain period of time. A project can fulfill several purposes such as in the area of research (research projects), projects dedicated to product development, infrastructure-related projects and more."@en ;
               rdfs:label "Project"@en ;
               skos:altLabel "Project"@en ;
               skos:definition "An enterprise (potentially individual but typically collaborative), planned to achieve a particular aim."@en ;
               skos:hiddenLabel "Venture"@en .


###  http://schema.org/ResearchProject
schema:ResearchProject rdf:type owl:Class ;
                       rdfs:subClassOf holy:PurposeBasedProject ;
                       dct:references <http://dx.doi.org/10.13140/RG.2.1.1432.6245> ,
                                      schema: ,
                                      <http://www.maxwideman.com/guests/typology/projects.htm> ,
                                      "https://dbpedia.org/ontology/ResearchProject"@en ,
                                      "https://schema.org/ResearchProject"@en ;
                       wn:hyponym "Meta Project"@en ,
                                  "Qualitative Project"@en ,
                                  "Quantitative Project"@en ;
                       rdfs:comment "The Schema.org defintion of Research Project is 'A Research Project'"@en ;
                       rdfs:label "Research Project"@en ;
                       skos:altLabel "Experimental Project"@en ,
                                     "R&D Project"@en ,
                                     "Research Project"@en ,
                                     "Research and Advanced Development Project"@en ;
                       skos:definition "A scientific investigation, usually using scientific methods, to achieve defined objectives."@en .


###  http://www.w3.org/2002/07/owl#Thing
owl:Thing rdf:type owl:Class ;
          rdfs:comment "The ontology is dedicated to store information of the hydrogen fuel cell domain. Since all sub-classes are providing detailed information to the general subject, 'owl:Thing' can be seen here as the Hydrogen Fuel Cell Domain."@en ;
          skos:altLabel "Hydrogen Fuel Cell Domain"@en .


###  http://www.w3.org/2004/02/skos/core#Concept
skos:Concept rdf:type owl:Class ;
             rdfs:comment "skos:concept is required for establishing a relationship for the object property rov:orgActivity."@en ;
             rdfs:label "Concept"@en ;
             skos:definition "A SKOS concept can be viewed as an idea or notion; a unit of thought. However, what constitutes a unit of thought is subjective, and this definition is meant to be suggestive, rather than restrictive."@en .


###  http://www.w3.org/ns/org#FormalOrganization
org:FormalOrganization rdf:type owl:Class ;
                       rdfs:subClassOf org:Organization ;
                       dct:references org: ;
                       rdfs:label "Formal Organization"@en ;
                       skos:definition "An organization which is recognized in the world at large, in particular in legal jurisdictions, with associated rights and responsibilities. Examples include a corporation, charity, government or church."@en .


###  http://www.w3.org/ns/org#Organization
org:Organization rdf:type owl:Class ;
                 dct:references org: ;
                 wn:hyponym "Enterprise"@en ,
                            "Institute"@en ,
                            "Institution"@en ,
                            "NGO"@en ;
                 rdfs:label "Organization"@en ;
                 skos:altLabel "Company"@en ,
                               "Organisation"@en ,
                               "Organization"@en ;
                 skos:definition "Represents a collection of people organized together into a community or other social, commercial or political structure. The group has some common purpose or reason for existence which goes beyond the set of people belonging to it and can act as an agent. Organizations are often decomposable into hierarchical structures."@en .


###  http://www.w3.org/ns/regorg#RegisteredOrganization
rov:RegisteredOrganization rdf:type owl:Class ;
                           rdfs:subClassOf org:FormalOrganization ;
                           dct:references rov: ,
                                          <https://ec.europa.eu/eurostat/documents/3859598/5902521/KS-RA-07-015-EN.PDF> ;
                           rdfs:comment "Inspired by the usage of the Registered Organization Vocabulary in the euBusinessGraph Ontology including links to The Organization Ontology."@en ;
                           rdfs:label "Registered Organization"@en ;
                           skos:altLabel "Registered Organization"@en ;
                           skos:definition "A registered company or other group of people that work together in a certain economic field with the purpose to compete in a certain market. The economic field of activity is defined by statistical standardization numbers such as primarily EC NACE 2, ISIC and SIC."@en .


#################################################################
#    Individuals
#################################################################

###  http://dbpedia.org/ontology/project
dbo:project rdf:type owl:NamedIndividual ,
                     schema:Project ;
            rdfs:comment "A project is a temporary endeavor undertaken to achieve defined objectives."@en ;
            rdfs:label "Project"@en .


###  http://dbpedia.org/ontology/research_project
dbo:research_project rdf:type owl:NamedIndividual ,
                              schema:ResearchProject ;
                     rdfs:comment "A research project is a scientific investigation, usually using scientific methods, to achieve defined objectives."@en ;
                     rdfs:label "Research Project"@en .


###  http://dbpedia.org/page/Category:Electric_vehicle_battery_manufacturers
dbc:Electric_vehicle_battery_manufacturers rdf:type owl:NamedIndividual ,
                                                    holy:ManufacturingOrganization .


###  http://dbpedia.org/page/Category:Fuel_cell_manufacturers
dbc:Fuel_cell_manufacturers rdf:type owl:NamedIndividual ,
                                     holy:ManufacturingOrganization .


###  http://dbpedia.org/page/Category:Fuel_cell_vehicles
dbc:Fuel_cell_vehicles rdf:type owl:NamedIndividual ,
                                holy:RoadApplication ;
                       rdfs:label "Fuel cell vehicles"@en .


###  http://dbpedia.org/page/Category:Heating
dbc:Heating rdf:type owl:NamedIndividual ,
                     holy:Heating ;
            rdfs:label "Heating"@en .


###  http://dbpedia.org/page/Category:Hydrogen_technologies
dbc:Hydrogen_technologies rdf:type owl:NamedIndividual ,
                                   holy:HydrogenProduct .


###  http://dbpedia.org/page/Category:Material_Handling
dbc:Material_Handling rdf:type owl:NamedIndividual ,
                               holy:MaterialHandlingVehicle ;
                      rdfs:comment "Material handling involves short-distance movement within the confines of a building or between a building and a transportation vehicle. It uses a wide range of manual, semi-automated, and automated equipment and includes consideration of the protection, storage, and control of materials throughout their manufacturing, warehousing, distribution, consumption, and disposal. Material handling can be used to create time and place utility through the handling, storage, and control of waste, as distinct from manufacturing, which creates form utility by changing the shape, form, and makeup of material."@en .


###  http://dbpedia.org/page/Category:Residential_heating_appliances
dbc:Residential_heating_appliances rdf:type owl:NamedIndividual ,
                                            holy:ResidentialHeating ;
                                   rdfs:label "Residential heating appliances"@en .


###  http://dbpedia.org/page/Category:Heating,_ventilation_and_air_conditioning
<http://dbpedia.org/page/Category:Heating,_ventilation_and_air_conditioning> rdf:type owl:NamedIndividual ,
                                                                                      holy:Heating ;
                                                                             rdfs:label "Heating, ventilation, and air conditioning"@en .


###  http://dbpedia.org/resource/Afghanistan
dbr:Afghanistan rdf:type owl:NamedIndividual ;
                owl:sameAs holy:Afghanistan .


###  http://purl.org/holy/ns#Afghanistan

###  http://dbpedia.org/resource/Africa
dbr:Africa rdf:type owl:NamedIndividual ;
           owl:sameAs holy:Africa .


###  http://purl.org/holy/ns#Africa

###  http://dbpedia.org/resource/Airbus
dbr:Airbus rdf:type owl:NamedIndividual ,
                    holy:ManufacturingOrganization ;
           m4i:inProject holy:ZEROe ;
           rdfs:comment "Airbus SE is a European multinational aerospace corporation. Airbus designs, manufactures and sells civil and military aerospace products worldwide and manufactures aircraft in Europe and various countries outside Europe. The company has three divisions: Commercial Aircraft (Airbus S.A.S.), Defence and Space, and Helicopters, the third being the largest in its industry in terms of revenues and turbine helicopter deliveries."@en ;
           rdfs:label "Airbus"@en .


###  http://dbpedia.org/resource/Albania
dbr:Albania rdf:type owl:NamedIndividual ;
            owl:sameAs holy:Albania .


###  http://purl.org/holy/ns#Albania

###  http://dbpedia.org/resource/Algeria
dbr:Algeria rdf:type owl:NamedIndividual ;
            owl:sameAs holy:Algeria .


###  http://purl.org/holy/ns#Algeria

###  http://dbpedia.org/resource/Alkaline_fuel_cell
dbr:Alkaline_fuel_cell rdf:type owl:NamedIndividual ,
                                holy:AlkalineFuelCell .


###  http://dbpedia.org/resource/Alstom
dbr:Alstom rdf:type owl:NamedIndividual ,
                    holy:ManufacturingOrganization ;
           holy:providesApplication dbr:Alstom_Coradia_iLint ;
           rdfs:comment "Alstom SA is a French multinational rolling stock manufacturer operating worldwide in rail transport markets, active in the fields of passenger transportation, signalling, and locomotives, with products including the AGV, TGV, Eurostar, Avelia and New Pendolino high-speed trains, in addition to suburban, regional and metro trains, and Citadis trams. In 2004, Alstom was again in financial difficulties, having incurred massive unexpected costs (€4 billion) arising from a design flaw inherited from the acquisition of ABB Group's turbine business, in addition to losses in other business sectors."@en ;
           rdfs:label "Alstom"@en ;
           skos:altLabel "AOMD"@en .


###  http://dbpedia.org/resource/Alstom_Coradia_Lint
dbr:Alstom_Coradia_Lint rdf:type owl:NamedIndividual ,
                                 holy:PassengerTrain ;
                        rdfs:comment "The Alstom Coradia LINT is an articulated railcar manufactured by Alstom since 1999, offered in diesel and hydrogen fuel models.The acronym LINT is short for the German \"leichter innovativer Nahverkehrstriebwagen\" (light innovative local transport rail vehicle). It was designed by Linke-Hofmann-Busch (LHB; acquired 1996 by Alstom) and has been distributed as part of Alstom's Coradia family."@en ;
                        rdfs:label "Alstom Coradia Lint"@en ;
                        skos:altLabel "Coradia Lint"@en .


###  http://dbpedia.org/resource/Alstom_Coradia_iLint
dbr:Alstom_Coradia_iLint rdf:type owl:NamedIndividual ,
                                  holy:PassengerTrain ;
                         holy:isProvidedBy dbr:Alstom ;
                         dct:references <https://www.alstom.com/solutions/rolling-stock/coradia-ilinttm-worlds-1st-hydrogen-powered-train> ;
                         rdfs:label "Coradia iLintTM"@en ;
                         skos:altLabel "Alstom Coradia iLint"@en ,
                                       "Coradia iLint"@en ;
                         skos:definition "The Coradia iLintTM is the world's first passenger train powered by a hydrogen fuel cell, which produces electrical power for traction."@en .


###  http://dbpedia.org/resource/Ambazonia
dbr:Ambazonia rdf:type owl:NamedIndividual ;
              owl:sameAs holy:Ambazonia .


###  http://purl.org/holy/ns#Ambazonia

###  http://dbpedia.org/resource/Andorra
dbr:Andorra rdf:type owl:NamedIndividual ;
            owl:sameAs holy:Andorra .


###  http://purl.org/holy/ns#Andorra

###  http://dbpedia.org/resource/Angola
dbr:Angola rdf:type owl:NamedIndividual ;
           owl:sameAs holy:Angola .


###  http://purl.org/holy/ns#Angola

###  http://dbpedia.org/resource/Antigua_and_Barbuda
dbr:Antigua_and_Barbuda rdf:type owl:NamedIndividual ;
                        owl:sameAs holy:Antigua_and_Barbuda .


###  http://purl.org/holy/ns#Antigua_and_Barbuda

###  http://dbpedia.org/resource/Argentina
dbr:Argentina rdf:type owl:NamedIndividual ;
              owl:sameAs holy:Argentina .


###  http://purl.org/holy/ns#Argentina

###  http://dbpedia.org/resource/Armenia
dbr:Armenia rdf:type owl:NamedIndividual ;
            owl:sameAs holy:Armenia .


###  http://purl.org/holy/ns#Armenia

###  http://dbpedia.org/resource/Asia
dbr:Asia rdf:type owl:NamedIndividual ;
         owl:sameAs holy:Asia .


###  http://purl.org/holy/ns#Asia

###  http://dbpedia.org/resource/Asia-Pacific
dbr:Asia-Pacific rdf:type owl:NamedIndividual ,
                          holy:GeographicMarket .


###  http://dbpedia.org/resource/Australia
dbr:Australia rdf:type owl:NamedIndividual ;
              owl:sameAs holy:Australia .


###  http://purl.org/holy/ns#Australia

###  http://dbpedia.org/resource/Austria
dbr:Austria rdf:type owl:NamedIndividual ;
            owl:sameAs holy:Austria .


###  http://purl.org/holy/ns#Austria

###  http://dbpedia.org/resource/Azerbaijan
dbr:Azerbaijan rdf:type owl:NamedIndividual ;
               owl:sameAs holy:Azerbaijan .


###  http://purl.org/holy/ns#Azerbaijan

###  http://dbpedia.org/resource/Bahrain
dbr:Bahrain rdf:type owl:NamedIndividual ;
            owl:sameAs holy:Bahrain .


###  http://purl.org/holy/ns#Bahrain

###  http://dbpedia.org/resource/Ballard_Power_Systems
dbr:Ballard_Power_Systems rdf:type owl:NamedIndividual ,
                                   holy:ManufacturingOrganization ;
                          rdfs:comment "Ballard Power Systems Inc. is a developer and manufacturer of proton exchange membrane (PEM) fuel cell products for markets such as heavy-duty motive (consisting of bus and tram applications), portable power, material handling as well as engineering services. Ballard has designed and shipped over 400 MW of fuel cell products to date."@en ;
                          rdfs:label "Ballard Power Systems"@en ;
                          skos:altLabel "Ballard_Power"@en ,
                                        "Ballard_Power_Systems,_Inc."@en ,
                                        "Ballard_Power_Systems_Inc."@en .


###  http://dbpedia.org/resource/Bangladesh
dbr:Bangladesh rdf:type owl:NamedIndividual ;
               owl:sameAs holy:Bangladesh .


###  http://purl.org/holy/ns#Bangladesh

###  http://dbpedia.org/resource/Barbados
dbr:Barbados rdf:type owl:NamedIndividual ;
             owl:sameAs holy:Barbados .


###  http://purl.org/holy/ns#Barbados

###  http://dbpedia.org/resource/Battery_electric_vehicle
dbr:Battery_electric_vehicle rdf:type owl:NamedIndividual ,
                                      holy:RoadApplication .


###  http://dbpedia.org/resource/Belarus
dbr:Belarus rdf:type owl:NamedIndividual ;
            owl:sameAs holy:Belarus .


###  http://purl.org/holy/ns#Belarus

###  http://dbpedia.org/resource/Belgium
dbr:Belgium rdf:type owl:NamedIndividual ;
            owl:sameAs holy:Belgium .


###  http://purl.org/holy/ns#Belgium

###  http://dbpedia.org/resource/Belize
dbr:Belize rdf:type owl:NamedIndividual ;
           owl:sameAs holy:Belize .


###  http://purl.org/holy/ns#Belize

###  http://dbpedia.org/resource/Benin
dbr:Benin rdf:type owl:NamedIndividual ;
          owl:sameAs holy:Benin .


###  http://purl.org/holy/ns#Benin

###  http://dbpedia.org/resource/Bhutan
dbr:Bhutan rdf:type owl:NamedIndividual ;
           owl:sameAs holy:Bhutan .


###  http://purl.org/holy/ns#Bhutan

###  http://dbpedia.org/resource/Boeing_Phantom_Eye
dbr:Boeing_Phantom_Eye rdf:type owl:NamedIndividual ,
                                holy:Aircraft ;
                       rdfs:comment "The Boeing Phantom Eye was a high altitude, long endurance (HALE) liquid hydrogen-powered unmanned aerial vehicle developed by Boeing Phantom Works. The aircraft was Boeing's proposal to meet the demand from the US military for unmanned drones designed to provide advanced intelligence and reconnaissance work, driven by the combat conditions in Afghanistan in particular. In August 2016, the Phantom Eye demonstrator was disassembled for display at the Air Force Flight Test Museum."@en .


###  http://dbpedia.org/resource/Bolivia
dbr:Bolivia rdf:type owl:NamedIndividual ;
            owl:sameAs holy:Bolivia .


###  http://purl.org/holy/ns#Bolivia

###  http://dbpedia.org/resource/Bosnia_and_Herzegovina
dbr:Bosnia_and_Herzegovina rdf:type owl:NamedIndividual ;
                           owl:sameAs holy:Bosnia_and_Herzegovina .


###  http://purl.org/holy/ns#Bosnia_and_Herzegovina

###  http://dbpedia.org/resource/Botswana
dbr:Botswana rdf:type owl:NamedIndividual ;
             owl:sameAs holy:Botswana .


###  http://purl.org/holy/ns#Botswana

###  http://dbpedia.org/resource/Brazil
dbr:Brazil rdf:type owl:NamedIndividual ;
           owl:sameAs holy:Brazil .


###  http://purl.org/holy/ns#Brazil

###  http://dbpedia.org/resource/British_Rail_Class_799
dbr:British_Rail_Class_799 rdf:type owl:NamedIndividual ,
                                    holy:PassengerTrain ;
                           rdfs:comment "The British Rail Class 799 are tri-mode multiple units prototype adapted from Class 319 electric multiple units (319001/382). The existing 25 kV AC and 750 V DC equipment has been retained with a hydrogen fuel cell added, currently taking up one of the carriages."@en ;
                           rdfs:label "British Rail Class 799"@en .


###  http://dbpedia.org/resource/Brunei
dbr:Brunei rdf:type owl:NamedIndividual ;
           owl:sameAs holy:Brunei .


###  http://purl.org/holy/ns#Brunei

###  http://dbpedia.org/resource/Bulgaria
dbr:Bulgaria rdf:type owl:NamedIndividual ;
             owl:sameAs holy:Bulgaria .


###  http://purl.org/holy/ns#Bulgaria

###  http://dbpedia.org/resource/Burkina_Faso
dbr:Burkina_Faso rdf:type owl:NamedIndividual ;
                 owl:sameAs holy:Burkina_Faso .


###  http://purl.org/holy/ns#Burkina_Faso

###  http://dbpedia.org/resource/Burundi
dbr:Burundi rdf:type owl:NamedIndividual ;
            owl:sameAs holy:Burundi .


###  http://purl.org/holy/ns#Burundi

###  http://dbpedia.org/resource/Cambodia
dbr:Cambodia rdf:type owl:NamedIndividual ;
             owl:sameAs holy:Cambodia .


###  http://purl.org/holy/ns#Cambodia

###  http://dbpedia.org/resource/Cameroon
dbr:Cameroon rdf:type owl:NamedIndividual ;
             owl:sameAs holy:Cameroon .


###  http://purl.org/holy/ns#Cameroon

###  http://dbpedia.org/resource/Canada
dbr:Canada rdf:type owl:NamedIndividual ;
           owl:sameAs holy:Canada .


###  http://purl.org/holy/ns#Canada

###  http://dbpedia.org/resource/Cape_Verde
dbr:Cape_Verde rdf:type owl:NamedIndividual ;
               owl:sameAs holy:Cape_Verde .


###  http://purl.org/holy/ns#Cape_Verde

###  http://dbpedia.org/resource/Central_African_Republic
dbr:Central_African_Republic rdf:type owl:NamedIndividual ;
                             owl:sameAs holy:Central_African_Republic .


###  http://purl.org/holy/ns#Central_African_Republic

###  http://dbpedia.org/resource/Central_America
dbr:Central_America rdf:type owl:NamedIndividual ,
                             holy:GeographicMarket .


###  http://dbpedia.org/resource/Central_Asia
dbr:Central_Asia rdf:type owl:NamedIndividual ;
                 owl:sameAs holy:Asia .


###  http://purl.org/holy/ns#Asia

###  http://dbpedia.org/resource/Chad
dbr:Chad rdf:type owl:NamedIndividual ;
         owl:sameAs holy:Chad .


###  http://purl.org/holy/ns#Chad

###  http://dbpedia.org/resource/Chile
dbr:Chile rdf:type owl:NamedIndividual ;
          owl:sameAs holy:Chile .


###  http://purl.org/holy/ns#Chile

###  http://dbpedia.org/resource/China
dbr:China rdf:type owl:NamedIndividual ;
          owl:sameAs holy:China ;
          rdfs:comment "China (Chinese: 中国; pinyin: Zhōngguó), officially the People's Republic of China (PRC; Chinese: 中华人民共和国; pinyin: Zhōnghuá Rénmín Gònghéguó), is a country in East Asia. It is the world's most populous country, with a population of more than 1.4 billion. China spans five geographical time zones and borders 14 different countries, the second most of any country in the world after Russia. Covering an area of approximately 9.6 million square kilometers (3,700,000 sq mi), it is the world's third or fourth largest country. The country consists of 23 provinces, five autonomous regions, four municipalities, and two Special Administrative Regions (Hong Kong and Macau). The national capital is Beijing."@en .


###  http://purl.org/holy/ns#China

###  http://dbpedia.org/resource/Colombia
dbr:Colombia rdf:type owl:NamedIndividual ;
             owl:sameAs holy:Colombia .


###  http://purl.org/holy/ns#Colombia

###  http://dbpedia.org/resource/Comoros
dbr:Comoros rdf:type owl:NamedIndividual ;
            owl:sameAs holy:Comoros .


###  http://purl.org/holy/ns#Comoros

###  http://dbpedia.org/resource/Cook_Islands
dbr:Cook_Islands rdf:type owl:NamedIndividual ;
                 owl:sameAs holy:Cook_Islands .


###  http://purl.org/holy/ns#Cook_Islands

###  http://dbpedia.org/resource/Costa_Rica
dbr:Costa_Rica rdf:type owl:NamedIndividual ;
               owl:sameAs holy:Costa_Rica .


###  http://purl.org/holy/ns#Costa_Rica

###  http://dbpedia.org/resource/Croatia
dbr:Croatia rdf:type owl:NamedIndividual ;
            owl:sameAs holy:Croatia .


###  http://purl.org/holy/ns#Croatia

###  http://dbpedia.org/resource/Cuba
dbr:Cuba rdf:type owl:NamedIndividual ;
         owl:sameAs holy:Cuba .


###  http://purl.org/holy/ns#Cuba

###  http://dbpedia.org/resource/Cyprus
dbr:Cyprus rdf:type owl:NamedIndividual ;
           owl:sameAs holy:Cyprus .


###  http://purl.org/holy/ns#Cyprus

###  http://dbpedia.org/resource/Czech_Republic
dbr:Czech_Republic rdf:type owl:NamedIndividual ;
                   owl:sameAs holy:Czech_Republic .


###  http://purl.org/holy/ns#Czech_Republic

###  http://dbpedia.org/resource/Daimler_AG
dbr:Daimler_AG rdf:type owl:NamedIndividual ,
                        holy:ManufacturingOrganization ;
               rdfs:comment "Daimler AG (previously named Daimler-Benz and DaimlerChrysler; commonly known and referred to as Mercedes-Benz or simply Daimler) is a German multinational automotive corporation headquartered in Stuttgart, Baden-Württemberg, Germany. It is one of the world's leading car and truck manufacturers. Daimler-Benz was formed with the merger of Benz & Cie. and Daimler Motoren Gesellschaft in 1926."@en ;
               rdfs:label "Daimler AG"@en .


###  http://dbpedia.org/resource/Democratic_Republic_of_the_Congo
dbr:Democratic_Republic_of_the_Congo rdf:type owl:NamedIndividual ;
                                     owl:sameAs holy:Democratic_Republic_of_the_Congo .


###  http://purl.org/holy/ns#Democratic_Republic_of_the_Congo

###  http://dbpedia.org/resource/Denmark
dbr:Denmark rdf:type owl:NamedIndividual ;
            owl:sameAs holy:Denmark .


###  http://purl.org/holy/ns#Denmark

###  http://dbpedia.org/resource/Direct_carbon_fuel_cell
dbr:Direct_carbon_fuel_cell rdf:type owl:NamedIndividual ,
                                     holy:SubstituteFuelCell .


###  http://dbpedia.org/resource/Direct_methanol_fuel_cell
dbr:Direct_methanol_fuel_cell rdf:type owl:NamedIndividual ,
                                       holy:MethanolFuelCell .


###  http://dbpedia.org/resource/Djibouti
dbr:Djibouti rdf:type owl:NamedIndividual ;
             owl:sameAs holy:Djibouti .


###  http://purl.org/holy/ns#Djibouti

###  http://dbpedia.org/resource/Dominica
dbr:Dominica rdf:type owl:NamedIndividual ;
             owl:sameAs holy:Dominica .


###  http://purl.org/holy/ns#Dominica

###  http://dbpedia.org/resource/Dominican_Republic
dbr:Dominican_Republic rdf:type owl:NamedIndividual ;
                       owl:sameAs holy:Dominican_Republic .


###  http://purl.org/holy/ns#Dominican_Republic

###  http://dbpedia.org/resource/East_Germany
dbr:East_Germany rdf:type owl:NamedIndividual ;
                 owl:sameAs holy:Germany .


###  http://purl.org/holy/ns#Germany

###  http://dbpedia.org/resource/East_Timor
dbr:East_Timor rdf:type owl:NamedIndividual ;
               owl:sameAs holy:East_Timor .


###  http://purl.org/holy/ns#East_Timor

###  http://dbpedia.org/resource/Eastern_Europe
dbr:Eastern_Europe rdf:type owl:NamedIndividual ;
                   owl:sameAs holy:Europe ;
                   rdfs:label "Eastern Europe"@en ;
                   skos:definition "Eastern Europe is the eastern region of Europe. There is no consistent definition of the precise area it covers, partly because the term has a wide range of geopolitical, geographical, ethnic, cultural, and socioeconomic connotations. Russia, located in Eastern Europe, is both the largest and most populous country of Europe, spanning roughly 40% of the continent's total landmass, with over 15% of its total population. According to the Center for Educational Technologies at Wheeling Jesuit University, there are \"almost as many definitions of Eastern Europe as there are scholars of the region\". A related United Nations paper adds that \"every assessment of spatial identities is essentially a social and cultural construct\". One definition describes Eastern Europe as a cultural entity: the region lying in Europe with the main characteristics consisting of East Slavic, Greek, Byzantine, Eastern Orthodox, and some Ottoman cultural influences. Another definition was created during the Cold War and used more or less alike with the term Eastern Bloc. A similar definition names the formerly communist European states outside the Soviet Union as Eastern Europe. Such definitions are often seen as outdated, but they are still sometimes used for statistical purposes. (en)"@en .


###  http://purl.org/holy/ns#Europe

###  http://dbpedia.org/resource/Ecuador
dbr:Ecuador rdf:type owl:NamedIndividual ;
            owl:sameAs holy:Ecuador .


###  http://purl.org/holy/ns#Ecuador

###  http://dbpedia.org/resource/Egypt
dbr:Egypt rdf:type owl:NamedIndividual ;
          owl:sameAs holy:Egypt .


###  http://purl.org/holy/ns#Egypt

###  http://dbpedia.org/resource/El_Salvador
dbr:El_Salvador rdf:type owl:NamedIndividual ;
                owl:sameAs holy:El_Salvador .


###  http://purl.org/holy/ns#El_Salvador

###  http://dbpedia.org/resource/Electric_bicycle
dbr:Electric_bicycle rdf:type owl:NamedIndividual ,
                              holy:Bike ;
                     rdfs:comment "An electric bicycle (e-bike, eBike, etc.) is a motorized bicycle with an integrated electric motor used to assist propulsion. Many kinds of e-bikes are available worldwide, but they generally fall into two broad categories: bikes that assist the rider's pedal-power (i.e. pedelecs) and bikes that add a throttle, integrating moped-style functionality. Both retain the ability to be pedaled by the rider and are therefore not electric motorcycles."@en .


###  http://dbpedia.org/resource/Equatorial_Guinea
dbr:Equatorial_Guinea rdf:type owl:NamedIndividual ;
                      owl:sameAs holy:Equatorial_Guinea .


###  http://purl.org/holy/ns#Equatorial_Guinea

###  http://dbpedia.org/resource/Eritrea
dbr:Eritrea rdf:type owl:NamedIndividual ;
            owl:sameAs holy:Eritrea .


###  http://purl.org/holy/ns#Eritrea

###  http://dbpedia.org/resource/Estonia
dbr:Estonia rdf:type owl:NamedIndividual ;
            owl:sameAs holy:Estonia .


###  http://purl.org/holy/ns#Estonia

###  http://dbpedia.org/resource/Eswatini
dbr:Eswatini rdf:type owl:NamedIndividual ;
             owl:sameAs holy:Eswatini .


###  http://purl.org/holy/ns#Eswatini

###  http://dbpedia.org/resource/Ethiopia
dbr:Ethiopia rdf:type owl:NamedIndividual ;
             owl:sameAs holy:Ethiopia .


###  http://purl.org/holy/ns#Ethiopia

###  http://dbpedia.org/resource/Europe
dbr:Europe rdf:type owl:NamedIndividual ;
           owl:sameAs holy:Europe ;
           rdfs:comment "Europe is a continent, also recognised as part of Eurasia, located entirely in the Northern Hemisphere and mostly in the Eastern Hemisphere. Comprising the westernmost peninsulas of the continental landmass of Eurasia, it shares the continental landmass of Afro-Eurasia with both Asia and Africa. It is bordered by the Arctic Ocean to the north, the Atlantic Ocean to the west, the Mediterranean Sea to the south and Asia to the east. Europe is commonly considered to be separated from Asia by the watershed of the Ural Mountains, the Ural River, the Caspian Sea, the Greater Caucasus, the Black Sea and the waterways of the Turkish Straits."@en ;
           rdfs:label "Europe"@en .


###  http://purl.org/holy/ns#Europe

###  http://dbpedia.org/resource/European_Union
dbr:European_Union rdf:type owl:NamedIndividual ;
                   owl:sameAs holy:Europe ;
                   rdfs:comment "The European Union (EU) is a political and economic union of 27 member states that are located primarily in Europe. The union has a total area of 4,233,255.3 km2 (1,634,469.0 sq mi) and an estimated total population of about 447 million. An internal single market has been established through a standardised system of laws that apply in all member states in those matters, and only those matters, where the states have agreed to act as one. EU policies aim to ensure the free movement of people, goods, services and capital within the internal market; enact legislation in justice and home affairs; and maintain common policies on trade, agriculture, fisheries and regional development. Passport controls have been abolished for travel within the Schengen Area."@en ;
                   rdfs:label "European Union"@en ;
                   skos:altLabel "EU"@en .


###  http://purl.org/holy/ns#Europe

###  http://dbpedia.org/resource/European_microstates
dbr:European_microstates rdf:type owl:NamedIndividual ;
                         owl:sameAs holy:European_microstates .


###  http://purl.org/holy/ns#European_microstates

###  http://dbpedia.org/resource/EvoBus
dbr:EvoBus rdf:type owl:NamedIndividual ,
                    holy:ManufacturingOrganization ;
           org:subOrganizationOf dbr:Daimler_AG ;
           rdfs:comment "EvoBus GmbH is a German bus and coach manufacturer headquartered in Stuttgart, Germany and a wholly owned subsidiary of . Its products go to market under the brands Setra or Mercedes-Benz."@en ;
           rdfs:label "EvoBus"@en ;
           skos:altLabel "EvoBus GmbH"@en .


###  http://dbpedia.org/resource/FCDO
dbr:FCDO rdf:type owl:NamedIndividual ,
                  holy:PublicAdministrationAndDefenseOrganization ;
         owl:sameAs <http://dbpedia.org/resource/Foreign,_Commonwealth_and_Development_Office> .


###  http://dbpedia.org/resource/Foreign,_Commonwealth_and_Development_Office

###  http://dbpedia.org/resource/Federal_Ministry_of_Transport_and_Digital_Infrastructure
dbr:Federal_Ministry_of_Transport_and_Digital_Infrastructure rdf:type owl:NamedIndividual ,
                                                                      holy:PublicAdministrationAndDefenseOrganization ;
                                                             m4i:inProject holy:NationalInnovationProgrammeHydrogenandFuelCellTechnology ;
                                                             org:hasSubOrganization dbr:Federal_Railway_Authority ;
                                                             ebg:isStateOwned "true"^^xsd:boolean ;
                                                             rdfs:comment "The Federal Ministry of Transport and Digital Infrastructure (German: Bundesministerium für Verkehr und digitale Infrastruktur), abbreviated BMVI, is a cabinet-level ministry of the Federal Republic of Germany. Its main office is located in Berlin, while the majority of its civil servants and employees work in Bonn, the secondary seat."@en ;
                                                             rdfs:label "Federal Ministry of Transport and Digital Infrastructure"@en ;
                                                             skos:altLabel "BMVI"@en ,
                                                                           """Federal Ministry of Transport and Digital Infrastructure
Bundesministerium für Verkehr und digitale Infrastruktur (BMVI)"""@en .


###  http://dbpedia.org/resource/Federal_Railway_Authority
dbr:Federal_Railway_Authority rdf:type owl:NamedIndividual ,
                                       holy:PublicAdministrationAndDefenseOrganization ;
                              ebg:isStateOwned "false"^^xsd:boolean ;
                              rdfs:comment "The German Federal Railway Authority (German: Eisenbahn-Bundesamt, EBA) has been the independent federal authority for the regulation of the railways in Germany since 1 January 1994. It is under the supervision and direction of the Federal Ministry for Digital and Transport and is headed by a president."@en ;
                              rdfs:label "Federal Railway Authority"@en ;
                              skos:altLabel """Eisenbahn-Bundesamt
Federal Railway Authority"""@en .


###  http://dbpedia.org/resource/Federated_States_of_Micronesia
dbr:Federated_States_of_Micronesia rdf:type owl:NamedIndividual ;
                                   owl:sameAs holy:Federated_States_of_Micronesia .


###  http://purl.org/holy/ns#Federated_States_of_Micronesia

###  http://dbpedia.org/resource/Fiat_Panda_Hydrogen
dbr:Fiat_Panda_Hydrogen rdf:type owl:NamedIndividual ,
                                 holy:Car ;
                        rdfs:comment "The Panda Hydrogen is a prototype fuel cell-type hydrogen vehicle based on the Fiat Panda introduced in 2006. The fuel, gaseous Hydrogen, is stored in underfloor hydrogen tanks at 350 bar. A \"Andromeda II\" fuel cell stack generates energy to power an electric motor directly, i.e. without a battery. Panda Hydrogen produces 40 kW (54 hp) power and it can achieve top speed of 130 km/h (81 mph). Operating range is over 200 km (120 mi) in urban driving."@en .


###  http://dbpedia.org/resource/Fiji
dbr:Fiji rdf:type owl:NamedIndividual ;
         owl:sameAs holy:Fiji .


###  http://purl.org/holy/ns#Fiji

###  http://dbpedia.org/resource/Finland
dbr:Finland rdf:type owl:NamedIndividual ;
            owl:sameAs holy:Finland .


###  http://purl.org/holy/ns#Finland

###  http://dbpedia.org/resource/Ford_F-250_Super_Chief
dbr:Ford_F-250_Super_Chief rdf:type owl:NamedIndividual ,
                                    holy:PickupTruck ;
                           holy:isProvidedBy dbr:Ford_Motor_Company ;
                           rdfs:label "Ford F-250 Super Chief"@en ;
                           skos:definition "The Ford F-250 Super Chief is a concept truck built by Ford. It featured a tri-flex fueling system that allows users to use three different fuels including gasoline, E85 ethanol or hydrogen. This is intended to make the Super Chief more attractive to customers who are concerned about finding fuel as the ethanol and hydrogen infrastructures are developing. In a tri-flex fueling system owners can utilize any given option at any one time. It comes with a stock bed cover and liner, it is a Ford crew cab. The back doors have been converted to suicide doors."@en .


###  http://dbpedia.org/resource/Ford_Motor_Company
dbr:Ford_Motor_Company rdf:type owl:NamedIndividual ,
                                holy:ManufacturingOrganization ;
                       holy:providesApplication dbr:Ford_F-250_Super_Chief ;
                       rdfs:comment "Ford Motor Company (commonly known as Ford) is an American multinational automobile manufacturer headquartered in Dearborn, Michigan, United States. It was founded by Henry Ford and incorporated on June 16, 1903. The company sells automobiles and commercial vehicles under the Ford brand, and luxury cars under its Lincoln luxury brand. Ford also owns Brazilian SUV manufacturer Troller, an 8% stake in Aston Martin of the United Kingdom and a 32% stake in China's Jiangling Motors. It also has joint-ventures in China (Changan Ford), Taiwan (Ford Lio Ho), Thailand (AutoAlliance Thailand), Turkey (Ford Otosan), and Russia (Ford Sollers). The company is listed on the New York Stock Exchange and is controlled by the Ford family; they have minority ownership but the majority of the voting power."@en ;
                       rdfs:label "Ford Motor Company"@en ;
                       skos:altLabel "FMC1"@en ,
                                     "Ford"@en .


###  http://dbpedia.org/resource/Forklift
dbr:Forklift rdf:type owl:NamedIndividual ,
                      holy:MaterialHandlingVehicle ;
             rdfs:comment "A forklift (also called lift truck, jitney, fork truck, fork hoist, and forklift truck) is a powered industrial truck used to lift and move materials over short distances."@en ;
             rdfs:label "Forklift"@en .


###  http://dbpedia.org/resource/France
dbr:France rdf:type owl:NamedIndividual ;
           owl:sameAs holy:France .


###  http://purl.org/holy/ns#France

###  http://dbpedia.org/resource/Fuel-cell_stack
dbr:Fuel-cell_stack rdf:type owl:NamedIndividual ,
                             holy:FuelCellStack ;
                    rdfs:label "Fuel-cell stack"@en .


###  http://dbpedia.org/resource/FuelCell_Energy
dbr:FuelCell_Energy rdf:type owl:NamedIndividual ,
                             holy:ManufacturingOrganization ;
                    holy:producesProduct holy:SureSource1500TM ,
                                         holy:SureSource3000TM ,
                                         holy:SureSource4000TM ;
                    ebg:isPubliclyTraded "true"^^xsd:boolean ;
                    rdfs:comment "FuelCell Energy, Inc. is a publicly traded fuel cell company, headquartered in Danbury, Connecticut. It designs, manufactures, operates and services Direct Fuel Cell power plants (a type of molten carbonate fuel cell). The company's fuel cell technology is an alternative to traditional combustion-based power generation, and is complementary to intermittent sources of energy, such as solar and wind turbines. As one of the biggest publicly traded fuel cell manufacturers in the U.S., the company provides clean energy in over 50 locations all over the world. It operates the world's largest fuel cell park, Gyeonggi Green Energy Fuel cell park, which is located in South Korea. The park consists of 21 power plants providing 59 Megawatt of electricity plus district heating to a number of customers"@en ;
                    rdfs:label "FuelCell Energy"@en ;
                    skos:altLabel "FCEL"@en ,
                                  "FuelCell Energy, Inc."@en ,
                                  "FuelCell_Energy"@en ,
                                  "Fuelcell Energy Inc"@en .


###  http://dbpedia.org/resource/Fuel_Cell_Bus_Club
dbr:Fuel_Cell_Bus_Club rdf:type owl:NamedIndividual ,
                                org:Organization ;
                       rdfs:comment "The Fuel Cell Bus Club comprised the participants of the projects (2001-2006), (2001-2005) and (2001-2005) which were pioneering demonstration projects for fuel cell bus fleets in Europe and Australia. The projects have been successfully completed. There were three buses in each of the 11 cities in the trial. The buses were a Mercedes-Benz Citaro and used hydrogen fuel cells from Ballard Power Systems. At the time they claimed to be the largest fleet of fuel cell buses in the world. The buses were estimated to cost US$ 1.2 million each and have a range of 300 kilometres (186.4 mi) and carry around 70 passengers."@en ;
                       rdfs:label "Fuel Cell Bus Club"@en .


###  http://dbpedia.org/resource/Fuel_cell_bus
dbr:Fuel_cell_bus rdf:type owl:NamedIndividual ,
                           holy:Bus ;
                  rdfs:comment "A fuel cell bus is a bus that uses a hydrogen fuel cell as its power source for electrically driven wheels, sometimes augmented in a hybrid fashion with batteries or a supercapacitor."@en ;
                  rdfs:label "Fuel cell bus"@en .


###  http://dbpedia.org/resource/Gabon
dbr:Gabon rdf:type owl:NamedIndividual ;
          owl:sameAs holy:Gabon .


###  http://purl.org/holy/ns#Gabon

###  http://dbpedia.org/resource/Germany
dbr:Germany rdf:type owl:NamedIndividual ;
            owl:sameAs holy:Germany .


###  http://purl.org/holy/ns#Germany

###  http://dbpedia.org/resource/Ghana
dbr:Ghana rdf:type owl:NamedIndividual ;
          owl:sameAs holy:Ghana .


###  http://purl.org/holy/ns#Ghana

###  http://dbpedia.org/resource/Greece
dbr:Greece rdf:type owl:NamedIndividual ;
           owl:sameAs holy:Greece .


###  http://purl.org/holy/ns#Greece

###  http://dbpedia.org/resource/Grenada
dbr:Grenada rdf:type owl:NamedIndividual ;
            owl:sameAs holy:Grenada .


###  http://purl.org/holy/ns#Grenada

###  http://dbpedia.org/resource/Guatemala
dbr:Guatemala rdf:type owl:NamedIndividual ;
              owl:sameAs holy:Guatemala .


###  http://purl.org/holy/ns#Guatemala

###  http://dbpedia.org/resource/Guinea
dbr:Guinea rdf:type owl:NamedIndividual ;
           owl:sameAs holy:Guinea .


###  http://purl.org/holy/ns#Guinea

###  http://dbpedia.org/resource/Guinea-Bissau
dbr:Guinea-Bissau rdf:type owl:NamedIndividual ;
                  owl:sameAs holy:Guinea-Bissau .


###  http://purl.org/holy/ns#Guinea-Bissau

###  http://dbpedia.org/resource/Guyana
dbr:Guyana rdf:type owl:NamedIndividual ;
           owl:sameAs holy:Guyana .


###  http://purl.org/holy/ns#Guyana

###  http://dbpedia.org/resource/Haiti
dbr:Haiti rdf:type owl:NamedIndividual ;
          owl:sameAs holy:Haiti .


###  http://purl.org/holy/ns#Haiti

###  http://dbpedia.org/resource/Honduras
dbr:Honduras rdf:type owl:NamedIndividual ;
             owl:sameAs holy:Honduras .


###  http://purl.org/holy/ns#Honduras

###  http://dbpedia.org/resource/Horizon_Fuel_Cell_Technolgies
dbr:Horizon_Fuel_Cell_Technolgies rdf:type owl:NamedIndividual ,
                                           holy:ManufacturingOrganization ;
                                  org:hasSubOrganization dbr:Hyzon_Motors ;
                                  rdfs:comment "Horizon Fuel Cell Technologies is a company founded in 2003 in Singapore, serving a diverse range of industries with various fuel cell electric energy solutions and products. Horizon Fuel Cell Technologies products and solutions are enabled by in-house manufacturing of micro-size to multi-kilowatt scale proton exchange membrane fuel cells, combined with a choice of proprietary on-demand hydrogen storage and production methods including hydrolysis, electrolysis and reformer-based solutions."@en ;
                                  rdfs:label "Horizon Fuel Cell Technologies"@en .


###  http://dbpedia.org/resource/Hungary
dbr:Hungary rdf:type owl:NamedIndividual ;
            owl:sameAs holy:Hungary .


###  http://purl.org/holy/ns#Hungary

###  http://dbpedia.org/resource/Hybrid_electric_vehicle
dbr:Hybrid_electric_vehicle rdf:type owl:NamedIndividual ,
                                     holy:RoadApplication ;
                            rdfs:comment "A hybrid electric vehicle (HEV) is a type of hybrid vehicle that combines a conventional internal combustion engine (ICE) system with an electric propulsion system (hybrid vehicle drivetrain). The presence of the electric powertrain is intended to achieve either better fuel economy than a conventional vehicle or better performance. There is a variety of HEV types and the degree to which each function as an electric vehicle (EV) also varies. The most common form of HEV is the hybrid electric car, although hybrid electric trucks (pickups and tractors), buses, boats and aircraft also exist."@en .


###  http://dbpedia.org/resource/Hybrid_train
dbr:Hybrid_train rdf:type owl:NamedIndividual ,
                          holy:Train ;
                 rdfs:comment "A hybrid train is a locomotive, railcar or train that uses an onboard rechargeable energy storage system (RESS), placed between the power source (often a diesel engine prime mover) and the traction transmission system connected to the wheels. Since most diesel locomotives are diesel-electric, they have all the components of a series hybrid transmission except the storage battery, making this a relatively simple prospect."@en .


###  http://dbpedia.org/resource/Hydrogen-powered_aircraft
dbr:Hydrogen-powered_aircraft rdf:type owl:NamedIndividual ,
                                       holy:Aircraft ;
                              rdfs:comment "A hydrogen-powered aircraft is an aeroplane that uses hydrogen fuel as a power source. Hydrogen can either be burned in a jet engine or another kind of internal combustion engine, or can be used to power a fuel cell to generate electricity to power a propeller. Unlike most aircraft, which store fuel in the wings, hydrogen-powered aircraft are usually designed with the hydrogen fuel tanks inside the fuselage."@en ;
                              rdfs:label "Hydrogen-powered aircraft"@en .


###  http://dbpedia.org/resource/Hydrogen_Fuel_Cell
dbr:Hydrogen_Fuel_Cell rdf:type owl:NamedIndividual ,
                                holy:HydrogenReconversion ;
                       rdfs:label "Hydrogen Fuel Cell"@en .


###  http://dbpedia.org/resource/Hydrogen_Tank
dbr:Hydrogen_Tank rdf:type owl:NamedIndividual ,
                           holy:HydrogenStorage ;
                  holy:isUsedIn holy:ZEROeBlendedWingBody ;
                  rdfs:comment "A hydrogen tank (other names- cartridge or canister) is used for hydrogen storage. The first type IV hydrogen tanks for compressed hydrogen at 700 bars (70 MPa; 10,000 psi) were demonstrated in 2001, the first fuel cell vehicles on the road with type IV tanks are the Toyota FCHV, Mercedes-Benz F-Cell and the GM HydroGen4."@en ;
                  rdfs:label "Hydrogen Tank"@en .


###  http://dbpedia.org/resource/Hydrogen_engine
dbr:Hydrogen_engine rdf:type owl:NamedIndividual ,
                             holy:HydrogenReconversion ;
                    holy:isUsedIn holy:ZEROeBlendedWingBody ;
                    rdfs:label "Hydrogen engine"@en .


###  http://dbpedia.org/resource/Hydrogen_technologies
dbr:Hydrogen_technologies rdf:type owl:NamedIndividual ,
                                   holy:HydrogenProduct ;
                          rdfs:comment "Hydrogen technologies are technologies that relate to the production and use of hydrogen. Hydrogen technologies are applicable for many uses. Some hydrogen technologies are carbon neutral and could have a role in preventing climate change and a possible future hydrogen economy. Hydrogen is a chemical widely used in various applications including ammonia production, oil refining and energy. The most common methods for producing hydrogen on an industrial scale are: Steam reforming, , coal gasification, water electrolysis. Hydrogen is not a primary energy source, because it is not naturally occurring as a fuel. It is, however, widely regarded as an ideal energy storage medium, due to the ease with which electricity can convert water into hydrogen and oxygen through electrolysis and can be con"@en .


###  http://dbpedia.org/resource/Hyundai_Motor_Company
dbr:Hyundai_Motor_Company rdf:type owl:NamedIndividual ,
                                   holy:ManufacturingOrganization ;
                          holy:providesApplication dbr:Hyundai_Nexo ,
                                                   dbr:Hyundai_ix35_FCEV ;
                          rdfs:comment "Hyundai Motor Company, often abbreviated to Hyundai Motors (Korean: 현대자동차; Hanja: 現代自動車; RR: Hyeondae Jadongcha ) and commonly known as Hyundai (Korean: 현대; Hanja: 現代; RR: Hyeondae, IPA: [ˈhjəːndɛ]; lit. 'modernity'), is a South Korean multinational automotive manufacturer headquartered in Seoul, South Korea. Hyundai Motor Company was founded in 1967. Currently, the company owns 33.88 percent of Kia Corporation, and also fully owns two marques including its luxury cars subsidiary, Genesis Motor, and an electric vehicle sub-brand, Ioniq. Those three brands altogether comprise the Hyundai Motor Group."@en ;
                          rdfs:label "Hyundai Motor Company"@en .


###  http://dbpedia.org/resource/Hyundai_Nexo
dbr:Hyundai_Nexo rdf:type owl:NamedIndividual ,
                          holy:Car ;
                 holy:isProvidedBy dbr:Hyundai_Motor_Company ;
                 rdfs:comment "The Hyundai Nexo (Korean: 현대 넥쏘, romanized: Hyeondae Negso) is a hydrogen fuel cell powered crossover SUV that was revealed at the 2018 Consumer Electronics Show on January 8, 2018. Replacing the Hyundai Tucson FCEV, the Nexo is the flagship for Hyundai's \"eco car\" portfolio."@en .


###  http://dbpedia.org/resource/Hyundai_ix35_FCEV
dbr:Hyundai_ix35_FCEV rdf:type owl:NamedIndividual ,
                               holy:Car ;
                      holy:isProvidedBy dbr:Hyundai_Motor_Company ;
                      rdfs:comment "The Hyundai ix35 FCEV or Tucson FCEV is a hydrogen fuel cell electric vehicle developed by Hyundai. The model is a left-hand drive only conversion to the SUV platform it is based on and was the first of its type to be mass-produced and sold commercially in the world. Different versions are known, the previous version was based on the Hyundai Tucson FCEV, and the upcoming model is based on the current ix35 FCEV. The first generation was introduced in 2001, with the Hyundai Santa Fe FCEV, and had a range of 100 miles (160 km), with a top speed of 78 mph (126 km/h)."@en .


###  http://dbpedia.org/resource/Hyzon_Motors
dbr:Hyzon_Motors rdf:type owl:NamedIndividual ,
                          holy:ManufacturingOrganization ;
                 holy:producesProduct dbr:Proton-exchange_membrane_fuel_cell ,
                                      holy:Hyzon_hybrid_bi-polar_plate_technology ;
                 holy:providesApplication holy:HyzonClass8 ,
                                          holy:HyzonDrayage ,
                                          holy:HyzonHymaxSeries ,
                                          holy:OWLNamedIndividual_7f4f3263_d74c_4f58_a998_c670b97905fa ;
                 rdfs:comment "Hyzon Motors is a supplier of zero-emissions hydrogen fuel cell powered commercial vehicles, including heavy duty trucks, buses and coaches. Hyzon was established as a new business of Horizon Fuel Cell Technologies."@en ;
                 rdfs:label "Hyzon Motors"@en ;
                 skos:altLabel "Hyzon"@en ,
                               "Hyzon Inc"@en ,
                               "Hyzon Motors Inc"@en .


###  http://dbpedia.org/resource/Iceland
dbr:Iceland rdf:type owl:NamedIndividual ;
            owl:sameAs holy:Iceland .


###  http://purl.org/holy/ns#Iceland

###  http://dbpedia.org/resource/Icelandic_New_Energy
dbr:Icelandic_New_Energy rdf:type owl:NamedIndividual ,
                                  org:Organization ;
                         m4i:inProject <http://purl.org/holy/ns#TheHydrogenUtilization&GreenEnergyProject> ;
                         rdfs:comment "Icelandic New Energy Ltd (Íslensk NýOrka ehf) is a company that promotes the use of hydrogen fuel in Iceland founded in 1999 following a decision in 1998 by the Icelandic Parliament to convert vehicle and fishing fleets to hydrogen produced from renewable energy by 2050. Together with SEV, and the authorities in the Faroe Islands and Greenland, Icelandic New Energy has established the to investigate hydrogen technology."@en ;
                         rdfs:label "Icelandic New Energy"@en ;
                         skos:altLabel "Icelandic New Energy Ltd"@en ,
                                       "Íslensk NýOrka ehf"@en .


###  http://dbpedia.org/resource/India
dbr:India rdf:type owl:NamedIndividual ;
          owl:sameAs holy:India .


###  http://purl.org/holy/ns#India

###  http://dbpedia.org/resource/Indonesia
dbr:Indonesia rdf:type owl:NamedIndividual ;
              owl:sameAs holy:Indonesia .


###  http://purl.org/holy/ns#Indonesia

###  http://dbpedia.org/resource/Ionic_liquid_piston_compressor
dbr:Ionic_liquid_piston_compressor rdf:type owl:NamedIndividual ,
                                            holy:HydrogenStorage ;
                                   rdfs:comment "An ionic liquid piston compressor, ionic compressor or ionic liquid piston pump is a hydrogen compressor based on an ionic liquid piston instead of a metal piston as in a piston-metal diaphragm compressor."@en ;
                                   rdfs:label "Ionic liquid piston compressor"@en ;
                                   skos:altLabel "Ionic compressor"@en .


###  http://dbpedia.org/resource/Iran
dbr:Iran rdf:type owl:NamedIndividual ;
         owl:sameAs holy:Iran .


###  http://purl.org/holy/ns#Iran

###  http://dbpedia.org/resource/Iraq
dbr:Iraq rdf:type owl:NamedIndividual ;
         owl:sameAs holy:Iraq .


###  http://purl.org/holy/ns#Iraq

###  http://dbpedia.org/resource/Israel
dbr:Israel rdf:type owl:NamedIndividual ;
           owl:sameAs holy:Israel .


###  http://purl.org/holy/ns#Israel

###  http://dbpedia.org/resource/Italy
dbr:Italy rdf:type owl:NamedIndividual ;
          owl:sameAs holy:Italy .


###  http://purl.org/holy/ns#Italy

###  http://dbpedia.org/resource/Ivory_Coast
dbr:Ivory_Coast rdf:type owl:NamedIndividual ;
                owl:sameAs holy:Ivory_Coast .


###  http://purl.org/holy/ns#Ivory_Coast

###  http://dbpedia.org/resource/Jamaica
dbr:Jamaica rdf:type owl:NamedIndividual ;
            owl:sameAs holy:Jamaica .


###  http://purl.org/holy/ns#Jamaica

###  http://dbpedia.org/resource/Jordan
dbr:Jordan rdf:type owl:NamedIndividual ;
           owl:sameAs holy:Jordan .


###  http://purl.org/holy/ns#Jordan

###  http://dbpedia.org/resource/Kazakhstan
dbr:Kazakhstan rdf:type owl:NamedIndividual ;
               owl:sameAs holy:Kazakhstan .


###  http://purl.org/holy/ns#Kazakhstan

###  http://dbpedia.org/resource/Keihin_Corporation
dbr:Keihin_Corporation rdf:type owl:NamedIndividual ,
                                holy:ManufacturingOrganization ;
                       rdfs:comment "The Keihin Corporation (株式会社ケーヒン, Kabushiki-gaisha Keihin) was founded December 19, 1956, and maintains its head office in Shinjuku Ward, Tokyo, Japan. It produces carburetors and fuel injection, and is a major supplier to Honda."@en ;
                       rdfs:label "Keihin Corporation"@en .


###  http://dbpedia.org/resource/Kenya
dbr:Kenya rdf:type owl:NamedIndividual ;
          owl:sameAs holy:Kenya .


###  http://purl.org/holy/ns#Kenya

###  http://dbpedia.org/resource/Kiribati
dbr:Kiribati rdf:type owl:NamedIndividual ;
             owl:sameAs holy:Kiribati .


###  http://purl.org/holy/ns#Kiribati

###  http://dbpedia.org/resource/Kosovo
dbr:Kosovo rdf:type owl:NamedIndividual ;
           owl:sameAs holy:Kosovo .


###  http://purl.org/holy/ns#Kosovo

###  http://dbpedia.org/resource/Kuwait
dbr:Kuwait rdf:type owl:NamedIndividual ;
           owl:sameAs holy:Kuwait .


###  http://purl.org/holy/ns#Kuwait

###  http://dbpedia.org/resource/Kyrgyzstan
dbr:Kyrgyzstan rdf:type owl:NamedIndividual ;
               owl:sameAs holy:Kyrgyzstan .


###  http://purl.org/holy/ns#Kyrgyzstan

###  http://dbpedia.org/resource/Laos
dbr:Laos rdf:type owl:NamedIndividual ;
         owl:sameAs holy:Laos .


###  http://purl.org/holy/ns#Laos

###  http://dbpedia.org/resource/Latin_America
dbr:Latin_America rdf:type owl:NamedIndividual ,
                           holy:GeographicMarket ;
                  owl:sameAs holy:South_America .


###  http://purl.org/holy/ns#South_America

###  http://dbpedia.org/resource/Latvia
dbr:Latvia rdf:type owl:NamedIndividual ;
           owl:sameAs holy:Latvia .


###  http://purl.org/holy/ns#Latvia

###  http://dbpedia.org/resource/Lebanon
dbr:Lebanon rdf:type owl:NamedIndividual ;
            owl:sameAs holy:Lebanon .


###  http://purl.org/holy/ns#Lebanon

###  http://dbpedia.org/resource/Lesotho
dbr:Lesotho rdf:type owl:NamedIndividual ;
            owl:sameAs holy:Lesotho .


###  http://purl.org/holy/ns#Lesotho

###  http://dbpedia.org/resource/Liberia
dbr:Liberia rdf:type owl:NamedIndividual ;
            owl:sameAs holy:Liberia .


###  http://purl.org/holy/ns#Liberia

###  http://dbpedia.org/resource/Libya
dbr:Libya rdf:type owl:NamedIndividual ;
          owl:sameAs holy:Libya .


###  http://purl.org/holy/ns#Libya

###  http://dbpedia.org/resource/Liechtenstein
dbr:Liechtenstein rdf:type owl:NamedIndividual ;
                  owl:sameAs holy:Liechtenstein .


###  http://purl.org/holy/ns#Liechtenstein

###  http://dbpedia.org/resource/Linde_plc
dbr:Linde_plc rdf:type owl:NamedIndividual ,
                       holy:ManufacturingOrganization ;
              holy:producesProduct dbr:Ionic_liquid_piston_compressor ,
                                   holy:CryogenicPistonPump ,
                                   holy:IonicCompressor50 ;
              ebg:isPubliclyTraded "true"^^xsd:boolean ;
              rdfs:comment "Linde plc is a global multinational chemical company founded in Germany and, since 2018, domiciled in Ireland and headquartered in the United Kingdom. Linde is the world's largest industrial gas company by market share and revenue. It serves customers in the healthcare, petroleum refining, manufacturing, food, beverage carbonation, fiber-optics, steel making, aerospace, chemicals, electronics and water treatment industries. The company's primary business is the manufacturing and distribution of atmospheric gases, including oxygen, nitrogen, argon, rare gases, and process gases, including carbon dioxide, helium, hydrogen, ammonia, electronic gases, specialty gases, and acetylene."@en ;
              rdfs:label "Linde plc"@en ;
              skos:altLabel "(LIN)"@en ,
                            "(NYSE:LIN)"@en ,
                            "Linde Engineering"@en .


###  http://dbpedia.org/resource/List_of_fuel_cell_manufacturers
dbr:List_of_fuel_cell_manufacturers rdf:type owl:NamedIndividual ,
                                             holy:ManufacturingOrganization ;
                                    rdfs:comment "A fuel cell is an electrochemical energy conversion device. Fuel cells differ from batteries in that they are designed for continuous replenishment of the reactants consumed. This is a partial list of companies currently producing commercially available fuel cell systems for use in residential, commercial, or industrial settings. Fuel cell systems from these manufacturers are currently being used to generate AC or DC electricity, heat, water, or any combination of the three."@en .


###  http://dbpedia.org/resource/List_of_fuel_cell_vehicles
dbr:List_of_fuel_cell_vehicles rdf:type owl:NamedIndividual ,
                                        holy:RoadApplication ;
                               rdfs:comment "A fuel cell vehicle is a vehicle that uses a fuel cell to power an electric drive system. There are also hybrid vehicles meaning that they are fitted with a fuel cell and a battery or a fuel cell and an ultracapacitor. For HICEV see List of hydrogen internal combustion engine vehicles. For a discussion of the advantages and disadvantages of fuel cell vehicles, see fuel cell vehicle."@en .


###  http://dbpedia.org/resource/Lithuania
dbr:Lithuania rdf:type owl:NamedIndividual ;
              owl:sameAs holy:Lithuania .


###  http://purl.org/holy/ns#Lithuania

###  http://dbpedia.org/resource/Luxembourg
dbr:Luxembourg rdf:type owl:NamedIndividual ;
               owl:sameAs holy:Luxembourg .


###  http://purl.org/holy/ns#Luxembourg

###  http://dbpedia.org/resource/Madagascar
dbr:Madagascar rdf:type owl:NamedIndividual ;
               owl:sameAs holy:Madagascar .


###  http://purl.org/holy/ns#Madagascar

###  http://dbpedia.org/resource/Mainland_Southeast_Asia
dbr:Mainland_Southeast_Asia rdf:type owl:NamedIndividual ,
                                     holy:GeographicMarket ;
                            owl:sameAs holy:Asia .


###  http://purl.org/holy/ns#Asia

###  http://dbpedia.org/resource/Malawi
dbr:Malawi rdf:type owl:NamedIndividual ;
           owl:sameAs holy:Malawi .


###  http://purl.org/holy/ns#Malawi

###  http://dbpedia.org/resource/Malaysia
dbr:Malaysia rdf:type owl:NamedIndividual ;
             owl:sameAs holy:Malaysia .


###  http://purl.org/holy/ns#Malaysia

###  http://dbpedia.org/resource/Maldives
dbr:Maldives rdf:type owl:NamedIndividual ;
             owl:sameAs holy:Maldives .


###  http://purl.org/holy/ns#Maldives

###  http://dbpedia.org/resource/Mali
dbr:Mali rdf:type owl:NamedIndividual ;
         owl:sameAs holy:Mali .


###  http://purl.org/holy/ns#Mali

###  http://dbpedia.org/resource/Malta
dbr:Malta rdf:type owl:NamedIndividual ;
          owl:sameAs holy:Malta .


###  http://purl.org/holy/ns#Malta

###  http://dbpedia.org/resource/Marshall_Islands
dbr:Marshall_Islands rdf:type owl:NamedIndividual ;
                     owl:sameAs holy:Marshall_Islands .


###  http://purl.org/holy/ns#Marshall_Islands

###  http://dbpedia.org/resource/Mauritania
dbr:Mauritania rdf:type owl:NamedIndividual ;
               owl:sameAs holy:Mauritania .


###  http://purl.org/holy/ns#Mauritania

###  http://dbpedia.org/resource/Mauritius
dbr:Mauritius rdf:type owl:NamedIndividual ;
              owl:sameAs holy:Mauritius .


###  http://purl.org/holy/ns#Mauritius

###  http://dbpedia.org/resource/Mercedes-Benz_Cito
dbr:Mercedes-Benz_Cito rdf:type owl:NamedIndividual ,
                                holy:Bus ;
                       holy:isProvidedBy dbr:EvoBus ;
                       rdfs:comment "The Mercedes-Benz Cito (coded as O520) was a low-floor midibus built by EvoBus for Continental Europe between 1999 and 2003. Unusual for buses at that time, it had a diesel-electric transmission and was planned to have a hybrid engine or a fuel cell at a later stage. The Diesel engine was positioned above the rear axle.It is planned to build a fuel cell type By The next few years."@en ;
                       rdfs:label "Mercedes-Benz Cito"@en .


###  http://dbpedia.org/resource/Mexico
dbr:Mexico rdf:type owl:NamedIndividual ;
           owl:sameAs holy:Mexico .


###  http://purl.org/holy/ns#Mexico

###  http://dbpedia.org/resource/Microbial_fuel_cell
dbr:Microbial_fuel_cell rdf:type owl:NamedIndividual ,
                                 holy:SubstituteProduct .


###  http://dbpedia.org/resource/Moldova
dbr:Moldova rdf:type owl:NamedIndividual ;
            owl:sameAs holy:Moldova .


###  http://purl.org/holy/ns#Moldova

###  http://dbpedia.org/resource/Monaco
dbr:Monaco rdf:type owl:NamedIndividual ;
           owl:sameAs holy:Monaco .


###  http://purl.org/holy/ns#Monaco

###  http://dbpedia.org/resource/Mongolia
dbr:Mongolia rdf:type owl:NamedIndividual ;
             owl:sameAs holy:Mongolia .


###  http://purl.org/holy/ns#Mongolia

###  http://dbpedia.org/resource/Montenegro
dbr:Montenegro rdf:type owl:NamedIndividual ;
               owl:sameAs holy:Montenegro .


###  http://purl.org/holy/ns#Montenegro

###  http://dbpedia.org/resource/Morocco
dbr:Morocco rdf:type owl:NamedIndividual ;
            owl:sameAs holy:Morocco .


###  http://purl.org/holy/ns#Morocco

###  http://dbpedia.org/resource/Mozambique
dbr:Mozambique rdf:type owl:NamedIndividual ;
               owl:sameAs holy:Mozambique .


###  http://purl.org/holy/ns#Mozambique

###  http://dbpedia.org/resource/Myanmar
dbr:Myanmar rdf:type owl:NamedIndividual ;
            owl:sameAs holy:Myanmar .


###  http://purl.org/holy/ns#Myanmar

###  http://dbpedia.org/resource/Namibia
dbr:Namibia rdf:type owl:NamedIndividual ;
            owl:sameAs holy:Namibia .


###  http://purl.org/holy/ns#Namibia

###  http://dbpedia.org/resource/Natural_gas_vehicle
dbr:Natural_gas_vehicle rdf:type owl:NamedIndividual ,
                                 holy:RoadApplication ;
                        rdfs:comment "A natural gas vehicle (NGV) is an alternative fuel vehicle that uses compressed natural gas (CNG) or liquefied natural gas (LNG). Natural gas vehicles should not be confused with autogas vehicles powered by liquefied petroleum gas (LPG), mainly propane, a fuel with a fundamentally different composition. Worldwide, there were almost 28 million NGVs by 2019. In 2016, the market was led by China (5.4 million), Iran (4 million), India (3 million), Pakistan (3 million), Argentina (2.2 million), Brazil (1.8 million), and Italy (1.1 million)."@en .


###  http://dbpedia.org/resource/Nauru
dbr:Nauru rdf:type owl:NamedIndividual ;
          owl:sameAs holy:Nauru .


###  http://purl.org/holy/ns#Nauru

###  http://dbpedia.org/resource/Nepal
dbr:Nepal rdf:type owl:NamedIndividual ;
          owl:sameAs holy:Nepal .


###  http://purl.org/holy/ns#Nepal

###  http://dbpedia.org/resource/Netherlands
dbr:Netherlands rdf:type owl:NamedIndividual ;
                owl:sameAs holy:Netherlands .


###  http://purl.org/holy/ns#Netherlands

###  http://dbpedia.org/resource/New_Sunshine_Project
dbr:New_Sunshine_Project rdf:type owl:NamedIndividual ,
                                  schema:ResearchProject ;
                         rdfs:comment "The New Sunshine Project (NSS) is a Japanese project to develop the technologies for new energy and global environment, integrating the Sunshine, the Moonlight (Energy-saving technology R & D) and the Global Environment Technology Projects since 1993. It is the successor of the 1974 MITI Sunshine Project, and focuses on the development of photovoltaic, geothermal and hydrogen technology."@en .


###  http://dbpedia.org/resource/New_Zealand
dbr:New_Zealand rdf:type owl:NamedIndividual ;
                owl:sameAs holy:New_Zealand .


###  http://purl.org/holy/ns#New_Zealand

###  http://dbpedia.org/resource/Nicaragua
dbr:Nicaragua rdf:type owl:NamedIndividual ;
              owl:sameAs holy:Nicaragua .


###  http://purl.org/holy/ns#Nicaragua

###  http://dbpedia.org/resource/Niger
dbr:Niger rdf:type owl:NamedIndividual ;
          owl:sameAs holy:Niger .


###  http://purl.org/holy/ns#Niger

###  http://dbpedia.org/resource/Nigeria
dbr:Nigeria rdf:type owl:NamedIndividual ;
            owl:sameAs holy:Nigeria .


###  http://purl.org/holy/ns#Nigeria

###  http://dbpedia.org/resource/Niue
dbr:Niue rdf:type owl:NamedIndividual ;
         owl:sameAs holy:Niue .


###  http://purl.org/holy/ns#Niue

###  http://dbpedia.org/resource/North_America
dbr:North_America rdf:type owl:NamedIndividual ;
                  owl:sameAs holy:North_America .


###  http://purl.org/holy/ns#North_America

###  http://dbpedia.org/resource/North_Macedonia
dbr:North_Macedonia rdf:type owl:NamedIndividual ;
                    owl:sameAs holy:North_Macedonia .


###  http://purl.org/holy/ns#North_Macedonia

###  http://dbpedia.org/resource/Norway
dbr:Norway rdf:type owl:NamedIndividual ;
           owl:sameAs holy:Norway .


###  http://purl.org/holy/ns#Norway

###  http://dbpedia.org/resource/Oceania
dbr:Oceania rdf:type owl:NamedIndividual ,
                     holy:GeographicMarket ;
            owl:sameAs holy:Oceania ;
            rdfs:comment "Oceania (UK: /ˌoʊsiˈɑːniə, ˌoʊʃi-, -ˈeɪn-/, US: /ˌoʊʃiˈæniə/, /-ˈɑːn-/) is a geographic region that includes Australasia, Melanesia, Micronesia and Polynesia. Spanning the Eastern and Western Hemispheres, Oceania has a land area of 8,525,989 square kilometres (3,291,903 sq mi) and a population of over 41 million. When compared with the continents, the region of Oceania is the smallest in land area and the second smallest in population after Antarctica."@en ;
            rdfs:label "Oceania"@en .


###  http://purl.org/holy/ns#Oceania

###  http://dbpedia.org/resource/Oman
dbr:Oman rdf:type owl:NamedIndividual ;
         owl:sameAs holy:Oman .


###  http://purl.org/holy/ns#Oman

###  http://dbpedia.org/resource/Pakistan
dbr:Pakistan rdf:type owl:NamedIndividual ;
             owl:sameAs holy:Pakistan .


###  http://purl.org/holy/ns#Pakistan

###  http://dbpedia.org/resource/Palau
dbr:Palau rdf:type owl:NamedIndividual ;
          owl:sameAs holy:Palau .


###  http://purl.org/holy/ns#Palau

###  http://dbpedia.org/resource/Pallet_jack
dbr:Pallet_jack rdf:type owl:NamedIndividual ,
                         holy:MaterialHandlingVehicle ;
                rdfs:comment "A pallet jack, also known as a pallet truck, pallet pump, pump truck, scooter, dog, or jigger is a tool used to lift and move pallets. Pallet jacks are the most basic form of a forklift and are intended to move pallets within a warehouse."@en ;
                rdfs:label "Pallet jack"@en ;
                skos:altLabel "Pallet Truck"@en .


###  http://dbpedia.org/resource/Panama
dbr:Panama rdf:type owl:NamedIndividual ;
           owl:sameAs holy:Panama .


###  http://purl.org/holy/ns#Panama

###  http://dbpedia.org/resource/Papua_New_Guinea
dbr:Papua_New_Guinea rdf:type owl:NamedIndividual ;
                     owl:sameAs holy:Papua_New_Guinea .


###  http://purl.org/holy/ns#Papua_New_Guinea

###  http://dbpedia.org/resource/Paraguay
dbr:Paraguay rdf:type owl:NamedIndividual ;
             owl:sameAs holy:Paraguay .


###  http://purl.org/holy/ns#Paraguay

###  http://dbpedia.org/resource/Peru
dbr:Peru rdf:type owl:NamedIndividual ;
         owl:sameAs holy:Peru .


###  http://purl.org/holy/ns#Peru

###  http://dbpedia.org/resource/Philippines
dbr:Philippines rdf:type owl:NamedIndividual ;
                owl:sameAs holy:Philippines .


###  http://purl.org/holy/ns#Philippines

###  http://dbpedia.org/resource/Plug_Power
dbr:Plug_Power rdf:type owl:NamedIndividual ,
                        holy:ManufacturingOrganization ;
               holy:producesProduct holy:GenSureFuelCellSystem ;
               rdfs:label "Plug Power Inc."@en ;
               skos:altLabel "PLUG"@en ,
                             "Plug Power"@en ;
               skos:definition "Plug Power Inc. is an American company engaged in the development of hydrogen fuel cell systems that replace conventional batteries in equipment and vehicles powered by electricity. The company is headquartered in Latham, New York, and has facilities in Spokane, Washington, and Rochester, New York."@en .


###  http://dbpedia.org/resource/Poland
dbr:Poland rdf:type owl:NamedIndividual ;
           owl:sameAs holy:Poland .


###  http://purl.org/holy/ns#Poland

###  http://dbpedia.org/resource/Portugal
dbr:Portugal rdf:type owl:NamedIndividual ;
             owl:sameAs holy:Portugal .


###  http://purl.org/holy/ns#Portugal

###  http://dbpedia.org/resource/Proton-exchange_membrane_fuel_cell
dbr:Proton-exchange_membrane_fuel_cell rdf:type owl:NamedIndividual ,
                                                holy:PolymerElectrolyteMembraneFuelCell ;
                                       holy:isUsedIn holy:HyzonClass8 ,
                                                     holy:HyzonHymaxSeries ;
                                       holy:producesProduct dbr:Hyzon_Motors ;
                                       rdfs:comment "Proton-exchange membrane fuel cells (PEMFC), also known as polymer electrolyte membrane (PEM) fuel cells, are a type of fuel cell being developed mainly for transport applications, as well as for stationary fuel-cell applications and portable fuel-cell applications. Their distinguishing features include lower temperature/pressure ranges (50 to 100 °C) and a special proton-conducting polymer electrolyte membrane. PEMFCs generate electricity and operate on the opposite principle to PEM electrolysis, which consumes electricity. They are a leading candidate to replace the aging alkaline fuel-cell technology, which was used in the Space Shuttle."@en ;
                                       rdfs:label "Proton-exchange membrane fuel cell"@en ;
                                       skos:altLabel "PEM Fuel Cell"@en ,
                                                     "PMEFC"@en .


###  http://dbpedia.org/resource/Qatar
dbr:Qatar rdf:type owl:NamedIndividual ;
          owl:sameAs holy:Qatar .


###  http://purl.org/holy/ns#Qatar

###  http://dbpedia.org/resource/Republic_of_Ireland
dbr:Republic_of_Ireland rdf:type owl:NamedIndividual ;
                        owl:sameAs holy:Republic_of_Ireland .


###  http://purl.org/holy/ns#Republic_of_Ireland

###  http://dbpedia.org/resource/Republic_of_the_Congo
dbr:Republic_of_the_Congo rdf:type owl:NamedIndividual ;
                          owl:sameAs holy:Republic_of_the_Congo .


###  http://purl.org/holy/ns#Republic_of_the_Congo

###  http://dbpedia.org/resource/Romania
dbr:Romania rdf:type owl:NamedIndividual ;
            owl:sameAs holy:Romania .


###  http://purl.org/holy/ns#Romania

###  http://dbpedia.org/resource/Russia
dbr:Russia rdf:type owl:NamedIndividual ;
           owl:sameAs holy:Russia .


###  http://purl.org/holy/ns#Russia

###  http://dbpedia.org/resource/Rwanda
dbr:Rwanda rdf:type owl:NamedIndividual ;
           owl:sameAs holy:Rwanda .


###  http://purl.org/holy/ns#Rwanda

###  http://dbpedia.org/resource/Sahrawi_Arab_Democratic_Republic
dbr:Sahrawi_Arab_Democratic_Republic rdf:type owl:NamedIndividual ;
                                     owl:sameAs holy:Sahrawi_Arab_Democratic_Republic .


###  http://purl.org/holy/ns#Sahrawi_Arab_Democratic_Republic

###  http://dbpedia.org/resource/Saint_Kitts_and_Nevis
dbr:Saint_Kitts_and_Nevis rdf:type owl:NamedIndividual ;
                          owl:sameAs holy:Saint_Kitts_and_Nevis .


###  http://purl.org/holy/ns#Saint_Kitts_and_Nevis

###  http://dbpedia.org/resource/Saint_Lucia
dbr:Saint_Lucia rdf:type owl:NamedIndividual ;
                owl:sameAs holy:Saint_Lucia .


###  http://purl.org/holy/ns#Saint_Lucia

###  http://dbpedia.org/resource/Saint_Vincent_and_the_Grenadines
dbr:Saint_Vincent_and_the_Grenadines rdf:type owl:NamedIndividual ;
                                     owl:sameAs holy:Saint_Vincent_and_the_Grenadines .


###  http://purl.org/holy/ns#Saint_Vincent_and_the_Grenadines

###  http://dbpedia.org/resource/Samoa
dbr:Samoa rdf:type owl:NamedIndividual ;
          owl:sameAs holy:Samoa .


###  http://purl.org/holy/ns#Samoa

###  http://dbpedia.org/resource/San_Marino
dbr:San_Marino rdf:type owl:NamedIndividual ;
               owl:sameAs holy:San_Marino .


###  http://purl.org/holy/ns#San_Marino

###  http://dbpedia.org/resource/Saudi_Arabia
dbr:Saudi_Arabia rdf:type owl:NamedIndividual ;
                 owl:sameAs holy:Saudi_Arabia .


###  http://purl.org/holy/ns#Saudi_Arabia

###  http://dbpedia.org/resource/Senegal
dbr:Senegal rdf:type owl:NamedIndividual ;
            owl:sameAs holy:Senegal .


###  http://purl.org/holy/ns#Senegal

###  http://dbpedia.org/resource/Serbia
dbr:Serbia rdf:type owl:NamedIndividual ;
           owl:sameAs holy:Serbia .


###  http://purl.org/holy/ns#Serbia

###  http://dbpedia.org/resource/Seychelles
dbr:Seychelles rdf:type owl:NamedIndividual ;
               owl:sameAs holy:Seychelles .


###  http://purl.org/holy/ns#Seychelles

###  http://dbpedia.org/resource/Sierra_Leone
dbr:Sierra_Leone rdf:type owl:NamedIndividual ;
                 owl:sameAs holy:Sierra_Leone .


###  http://purl.org/holy/ns#Sierra_Leone

###  http://dbpedia.org/resource/Singapore
dbr:Singapore rdf:type owl:NamedIndividual ;
              owl:sameAs holy:Singapore .


###  http://purl.org/holy/ns#Singapore

###  http://dbpedia.org/resource/Slovakia
dbr:Slovakia rdf:type owl:NamedIndividual ;
             owl:sameAs holy:Slovakia .


###  http://purl.org/holy/ns#Slovakia

###  http://dbpedia.org/resource/Slovenia
dbr:Slovenia rdf:type owl:NamedIndividual ;
             owl:sameAs holy:Slovenia .


###  http://purl.org/holy/ns#Slovenia

###  http://dbpedia.org/resource/Solid_oxide_fuel_cell
dbr:Solid_oxide_fuel_cell rdf:type owl:NamedIndividual ,
                                   holy:SolidOxideFuelCell ;
                          rdfs:label "Solid oxide fuel cell"@en .


###  http://dbpedia.org/resource/Solomon_Islands
dbr:Solomon_Islands rdf:type owl:NamedIndividual ;
                    owl:sameAs holy:Solomon_Islands .


###  http://purl.org/holy/ns#Solomon_Islands

###  http://dbpedia.org/resource/Somalia
dbr:Somalia rdf:type owl:NamedIndividual ;
            owl:sameAs holy:Somalia .


###  http://purl.org/holy/ns#Somalia

###  http://dbpedia.org/resource/Somaliland
dbr:Somaliland rdf:type owl:NamedIndividual ;
               owl:sameAs holy:Somaliland .


###  http://purl.org/holy/ns#Somaliland

###  http://dbpedia.org/resource/South_Africa
dbr:South_Africa rdf:type owl:NamedIndividual ;
                 owl:sameAs holy:South_Africa .


###  http://purl.org/holy/ns#South_Africa

###  http://dbpedia.org/resource/South_America
dbr:South_America rdf:type owl:NamedIndividual ;
                  owl:sameAs holy:South_America .


###  http://purl.org/holy/ns#South_America

###  http://dbpedia.org/resource/South_Sudan
dbr:South_Sudan rdf:type owl:NamedIndividual ;
                owl:sameAs holy:South_Sudan .


###  http://purl.org/holy/ns#South_Sudan

###  http://dbpedia.org/resource/Spain
dbr:Spain rdf:type owl:NamedIndividual ;
          owl:sameAs holy:Spain .


###  http://purl.org/holy/ns#Spain

###  http://dbpedia.org/resource/Sri_Lanka
dbr:Sri_Lanka rdf:type owl:NamedIndividual ;
              owl:sameAs holy:Sri_Lanka .


###  http://purl.org/holy/ns#Sri_Lanka

###  http://dbpedia.org/resource/Stationary_fuel-cell_applications
dbr:Stationary_fuel-cell_applications rdf:type owl:NamedIndividual ,
                                               holy:PowerGeneration ;
                                      rdfs:comment "Definition from dbpedia: Stationary fuel-cell applications (or stationary fuel-cell power systems) are applications for fuel cells that are either connected to the electric grid (distributed generation) to provide supplemental power and as emergency power system for critical areas, or installed as a grid-independent generator for on-site service."@en ;
                                      rdfs:label "Stationary fuel-cell applications"@en .


###  http://dbpedia.org/resource/Sudan
dbr:Sudan rdf:type owl:NamedIndividual ;
          owl:sameAs holy:Sudan .


###  http://purl.org/holy/ns#Sudan

###  http://dbpedia.org/resource/Suriname
dbr:Suriname rdf:type owl:NamedIndividual ;
             owl:sameAs holy:Suriname .


###  http://purl.org/holy/ns#Suriname

###  http://dbpedia.org/resource/Sweden
dbr:Sweden rdf:type owl:NamedIndividual ;
           owl:sameAs holy:Sweden .


###  http://purl.org/holy/ns#Sweden

###  http://dbpedia.org/resource/Switzerland
dbr:Switzerland rdf:type owl:NamedIndividual ;
                owl:sameAs holy:Switzerland .


###  http://purl.org/holy/ns#Switzerland

###  http://dbpedia.org/resource/Syria
dbr:Syria rdf:type owl:NamedIndividual ;
          owl:sameAs holy:Syria .


###  http://purl.org/holy/ns#Syria

###  http://dbpedia.org/resource/Tajikistan
dbr:Tajikistan rdf:type owl:NamedIndividual ;
               owl:sameAs holy:Tajikistan .


###  http://purl.org/holy/ns#Tajikistan

###  http://dbpedia.org/resource/Tank_Truck
dbr:Tank_Truck rdf:type owl:NamedIndividual ,
                        holy:Truck ;
               rdfs:comment "A tank truck, gas truck, fuel truck, or tanker truck (United States usage) or tanker (United Kingdom usage), is a motor vehicle designed to carry liquids or gases on roads. The largest such vehicles are similar to railroad tank cars which are also designed to carry liquid loads. Many variants exist due to the wide variety of liquids that can be transported. Tank trucks tend to be large; they may be insulated or non-insulated; pressurized or non-pressurized; and designed for single or multiple loads (often by means of internal divisions in their tank). Some are semi-trailer trucks. They are difficult to drive and highly susceptible to rollover due to their high center of gravity, and potentially the free surface effect of liquids sloshing in a partially filled tank."@en ;
               rdfs:label "Tank Truck"@en ;
               skos:altLabel "Liquid hydrogen tank truck"@en ,
                             "fuel truck"@en ,
                             "gas truck"@en ,
                             "tanker truck"@en .


###  http://dbpedia.org/resource/Tanzania
dbr:Tanzania rdf:type owl:NamedIndividual ;
             owl:sameAs holy:Tanzania .


###  http://purl.org/holy/ns#Tanzania

###  http://dbpedia.org/resource/Thailand
dbr:Thailand rdf:type owl:NamedIndividual ;
             owl:sameAs holy:Thailand .


###  http://purl.org/holy/ns#Thailand

###  http://dbpedia.org/resource/The_Bahamas
dbr:The_Bahamas rdf:type owl:NamedIndividual ;
                owl:sameAs holy:The_Bahamas .


###  http://purl.org/holy/ns#The_Bahamas

###  http://dbpedia.org/resource/The_Gambia
dbr:The_Gambia rdf:type owl:NamedIndividual ;
               owl:sameAs holy:The_Gambia .


###  http://purl.org/holy/ns#The_Gambia

###  http://dbpedia.org/resource/Tiger_Cub_Economies
dbr:Tiger_Cub_Economies rdf:type owl:NamedIndividual ;
                        owl:sameAs holy:Tiger_Cub_Economies .


###  http://purl.org/holy/ns#Tiger_Cub_Economies

###  http://dbpedia.org/resource/Togo
dbr:Togo rdf:type owl:NamedIndividual ;
         owl:sameAs holy:Togo .


###  http://purl.org/holy/ns#Togo

###  http://dbpedia.org/resource/Tonga
dbr:Tonga rdf:type owl:NamedIndividual ;
          owl:sameAs holy:Tonga .


###  http://purl.org/holy/ns#Tonga

###  http://dbpedia.org/resource/Toyota_FCHV-4
dbr:Toyota_FCHV-4 rdf:type owl:NamedIndividual ,
                           holy:Car .


###  http://dbpedia.org/resource/Toyota_Fuel_Cell_Hybrid_Vehicle-Advanced
dbr:Toyota_Fuel_Cell_Hybrid_Vehicle-Advanced rdf:type owl:NamedIndividual ,
                                                      holy:Car ;
                                             rdfs:comment "The Toyota Fuel Cell Hybrid Vehicle-Advanced (FCHV-adv) is a fuel cell vehicle based on the first generation Toyota FCHV. The proposed FCHV-adv uses four hydrogen fuel tanks, which store high-pressure compressed hydrogen at up to 70 MPa (10,153 psi/700 bar) and feed it into a fuel stack to produce electricity via a chemical reaction between hydrogen and oxygen. This electricity then powers an electric motor, capable of 90 kW (122 ps/121 hp) and 260 Nm (26.5 kgf/192 lb·ft) of torque, and charges a nickel–metal hydride battery. Cruising range is approximately 760 km (472 mi) to 830 km (516 mi), and top speed is stated to be 155 km/h (96 mph)."@en ;
                                             skos:altLabel "Toyota FCHV-adv"@en .


###  http://dbpedia.org/resource/Trinidad_and_Tobago
dbr:Trinidad_and_Tobago rdf:type owl:NamedIndividual ;
                        owl:sameAs holy:Trinidad_and_Tobago .


###  http://purl.org/holy/ns#Trinidad_and_Tobago

###  http://dbpedia.org/resource/Tunisia
dbr:Tunisia rdf:type owl:NamedIndividual ;
            owl:sameAs holy:Tunisia .


###  http://purl.org/holy/ns#Tunisia

###  http://dbpedia.org/resource/Turkey
dbr:Turkey rdf:type owl:NamedIndividual ;
           owl:sameAs holy:Turkey .


###  http://purl.org/holy/ns#Turkey

###  http://dbpedia.org/resource/Turkmenistan
dbr:Turkmenistan rdf:type owl:NamedIndividual ;
                 owl:sameAs holy:Turkmenistan .


###  http://purl.org/holy/ns#Turkmenistan

###  http://dbpedia.org/resource/Tuvalu
dbr:Tuvalu rdf:type owl:NamedIndividual ;
           owl:sameAs holy:Tuvalu .


###  http://purl.org/holy/ns#Tuvalu

###  http://dbpedia.org/resource/Uganda
dbr:Uganda rdf:type owl:NamedIndividual ;
           owl:sameAs holy:Uganda .


###  http://purl.org/holy/ns#Uganda

###  http://dbpedia.org/resource/Ukraine
dbr:Ukraine rdf:type owl:NamedIndividual ;
            owl:sameAs holy:Ukraine .


###  http://purl.org/holy/ns#Ukraine

###  http://dbpedia.org/resource/United_Arab_Emirates
dbr:United_Arab_Emirates rdf:type owl:NamedIndividual ;
                         owl:sameAs holy:United_Arab_Emirates .


###  http://purl.org/holy/ns#United_Arab_Emirates

###  http://dbpedia.org/resource/United_Kingdom
dbr:United_Kingdom rdf:type owl:NamedIndividual ;
                   owl:sameAs holy:United_Kingdom .


###  http://purl.org/holy/ns#United_Kingdom

###  http://dbpedia.org/resource/United_States
dbr:United_States rdf:type owl:NamedIndividual ;
                  owl:sameAs holy:United_States .


###  http://purl.org/holy/ns#United_States

###  http://dbpedia.org/resource/Uruguay
dbr:Uruguay rdf:type owl:NamedIndividual ;
            owl:sameAs holy:Uruguay .


###  http://purl.org/holy/ns#Uruguay

###  http://dbpedia.org/resource/Uzbekistan
dbr:Uzbekistan rdf:type owl:NamedIndividual ;
               owl:sameAs holy:Uzbekistan .


###  http://purl.org/holy/ns#Uzbekistan

###  http://dbpedia.org/resource/Vacuum_truck
dbr:Vacuum_truck rdf:type owl:NamedIndividual ,
                          holy:RegionalTruck ;
                 rdfs:comment "A vacuum truck or vacuum tanker is a tank truck that has a pump and a tank. The pump is designed to pneumatically suck liquids, sludges, slurries, or the like from a location (often underground) into the tank of the truck. The objective is to enable transport of the liquid material via road to another location. Vacuum trucks transport the collected material to a treatment or disposal site, for example a sewage treatment plant. Vacuum trucks can be equipped with a high pressure pump if they are used to clean out sewers from sand."@en ;
                 rdfs:label "Vacuum truck"@en .


###  http://dbpedia.org/resource/Van_Hool
dbr:Van_Hool rdf:type owl:NamedIndividual ,
                      holy:ManufacturingOrganization ;
             rdfs:label "Van Hool"@en ;
             skos:altLabel "Vanhool"@en .


###  http://dbpedia.org/resource/Vanuatu
dbr:Vanuatu rdf:type owl:NamedIndividual ;
            owl:sameAs holy:Vanuatu .


###  http://purl.org/holy/ns#Vanuatu

###  http://dbpedia.org/resource/Vatican_City
dbr:Vatican_City rdf:type owl:NamedIndividual ;
                 owl:sameAs holy:Vatican_City .


###  http://purl.org/holy/ns#Vatican_City

###  http://dbpedia.org/resource/Venezuela
dbr:Venezuela rdf:type owl:NamedIndividual ;
              owl:sameAs holy:Venezuela .


###  http://purl.org/holy/ns#Venezuela

###  http://dbpedia.org/resource/Vietnam
dbr:Vietnam rdf:type owl:NamedIndividual ;
            owl:sameAs holy:Vietnam .


###  http://purl.org/holy/ns#Vietnam

###  http://dbpedia.org/resource/West_Germany
dbr:West_Germany rdf:type owl:NamedIndividual ,
                          holy:GeographicMarket ;
                 owl:sameAs holy:Germany .


###  http://purl.org/holy/ns#Germany

###  http://dbpedia.org/resource/Western_Europe
dbr:Western_Europe rdf:type owl:NamedIndividual ,
                            holy:GeographicMarket ;
                   owl:sameAs holy:Europe ;
                   rdfs:label "Western Europe"@en ;
                   skos:definition "Western Europe is the European region farthest from Asia. The region's countries and territories vary depending on context. Beginning with foreign exploration during the Age of Discovery, roughly from the 15th century, the concept of Europe as \"the West\" gradually became distinguished from and eventually replaced the dominant use of \"Christendom\" as the preferred endonym within the region. Later, during the Age of Enlightenment, the concept of \"Eastern Europe\" was created to juxtapose that of \"Western Europe\"."@en .


###  http://purl.org/holy/ns#Europe

###  http://dbpedia.org/resource/Western_Sahara
dbr:Western_Sahara rdf:type owl:NamedIndividual ;
                   owl:sameAs holy:Western_Sahara .


###  http://purl.org/holy/ns#Western_Sahara

###  http://dbpedia.org/resource/Western_world
dbr:Western_world rdf:type owl:NamedIndividual ,
                           holy:GeographicMarket .


###  http://dbpedia.org/resource/World
dbr:World rdf:type owl:NamedIndividual ,
                   holy:GeographicMarket .


###  http://dbpedia.org/resource/Yemen
dbr:Yemen rdf:type owl:NamedIndividual ;
          owl:sameAs holy:Yemen .


###  http://purl.org/holy/ns#Yemen

###  http://dbpedia.org/resource/Zambia
dbr:Zambia rdf:type owl:NamedIndividual ;
           owl:sameAs holy:Zambia .


###  http://purl.org/holy/ns#Zambia

###  http://dbpedia.org/resource/Zimbabwe
dbr:Zimbabwe rdf:type owl:NamedIndividual ;
             owl:sameAs holy:Zimbabwe .


###  http://purl.org/holy/ns#Zimbabwe

###  http://dbpedia.org/resource/combined_heat_and_power_station
dbr:combined_heat_and_power_station rdf:type owl:NamedIndividual ,
                                             holy:Heating ;
                                    rdfs:label "Combined heat and power station"@en ;
                                    skos:altLabel "Combined heat and power generation"@en ,
                                                  "Combined heat/power generation"@en .


###  http://dbpedia.org/resource/Foreign,_Commonwealth_and_Development_Office
<http://dbpedia.org/resource/Foreign,_Commonwealth_and_Development_Office> rdf:type owl:NamedIndividual ,
                                                                                    holy:PublicAdministrationAndDefenseOrganization ;
                                                                           holy:participatesIn holy:United_Kingdom ;
                                                                           ebg:isStateOwned "true"^^xsd:boolean ;
                                                                           rdfs:comment "The Foreign, Commonwealth & Development Office (FCDO) is a department of the Government of the United Kingdom. It was created on 2 September 2020 through the merger of the Foreign & Commonwealth Office (FCO) and the Department for International Development (DFID). The FCO, itself created in 1968 by the merger of the Foreign Office (FO) and the Commonwealth Office, was responsible for protecting and promoting British interests worldwide. The expenditure, administration and policy of the FCDO are scrutinised by the Foreign Affairs Select Committee."@en ;
                                                                           rdfs:label "Foreign, Commonwealth and Development Office"@en .


###  http://dbpedia.org/resource/Georgia_(country)
<http://dbpedia.org/resource/Georgia_(country)> rdf:type owl:NamedIndividual ;
                                                owl:sameAs <http://purl.org/holy/ns#Georgia_(country)> .


###  http://purl.org/holy/ns#Georgia_(country)

###  http://fraunhofer.de/dataKoreaWesternPowerCompanyLimited
<http://fraunhofer.de/dataKoreaWesternPowerCompanyLimited> rdf:type owl:NamedIndividual ,
                                                                    holy:EnergySectorOrganization ;
                                                           holy:participatesIn <http://fraunhofer.de/dataRepublicofKorea> ;
                                                           dct:references <https://www.iwest.co.kr/eng/835/subview.do> ;
                                                           rdfs:label "Korea Western Power Company Limited"@en ;
                                                           skos:altLabel "KOWEPO"@en ;
                                                           skos:definition "Korea Western Power Co., Ltd.(KOWEPO), a leading supplier and innovator in the 21st century Korean power industry, started its power business in April 2001. KOWEPO takes up approximately 8.7% of the national generating capacity mostly comprised of thermal and combined cycle. KOWEPO was initiated in separation from Korea Electric Power Corporation under the Korea Power Industry Restructuring Act. KOWEPO is now in the process of deregulation and privatization process. KOWEPO has about 2,350 employees and its head office is located in Taean-gun, Chungcheongnam-do, Republic of Korea."@en .


###  http://fraunhofer.de/dataRepublicofKorea
<http://fraunhofer.de/dataRepublicofKorea> rdf:type owl:NamedIndividual ,
                                                    schema:Country ;
                                           holy:hasOrganization <http://fraunhofer.de/dataKoreaWesternPowerCompanyLimited> ;
                                           rdfs:label "Republic of Korea"@en .


###  http://fraunhofer.de/dataSmartFarmFuelCellPowerGenerationProject
<http://fraunhofer.de/dataSmartFarmFuelCellPowerGenerationProject> rdf:type owl:NamedIndividual ,
                                                                            holy:CircularEconomyProject ;
                                                                   dct:references <https://fuelcellsworks.com/news/korea/korea-western-power-promotes-smart-farm-fuel-cell-power-generation-project/> ;
                                                                   rdfs:label "Smart Farm Fuel Cell Power Generation Project"@en ;
                                                                   skos:altLabel "Sangju Smart Farm Innovation Valley"@en .


###  http://purl.org/holy/ns#A12FuelCell
holy:A12FuelCell rdf:type owl:NamedIndividual ,
                          holy:Bus ;
                 rdfs:label "A12 Fuel Cell"@en ;
                 skos:definition "A city bus designed and produced by the company vanhool."@en .


###  http://purl.org/holy/ns#A13FuelCell
holy:A13FuelCell rdf:type owl:NamedIndividual ,
                          holy:Bus ;
                 rdfs:label "A13 Fuel Cell"@en ;
                 skos:definition "A city bus designed and produced by the company vanhool."@en .


###  http://purl.org/holy/ns#A18FuelCell
holy:A18FuelCell rdf:type owl:NamedIndividual ,
                          holy:Bus ;
                 rdfs:label "A18 Fuel Cell"@en ;
                 skos:definition "A city bus designed and produced by the company vanhool."@en .


###  http://purl.org/holy/ns#A330FuelCell
holy:A330FuelCell rdf:type owl:NamedIndividual ,
                           holy:Bus ;
                  rdfs:label "A330 Fuel Cell"@en ;
                  skos:definition "A city bus designed and produced by the company vanhool."@en .


###  http://purl.org/holy/ns#Afghanistan
holy:Afghanistan rdf:type owl:NamedIndividual ,
                          schema:Country ;
                 dbo:continent holy:Asia ;
                 rdfs:label "Afghanistan"@en .


###  http://purl.org/holy/ns#Africa
holy:Africa rdf:type owl:NamedIndividual ,
                     schema:Continent ;
            rdfs:label "Africa"@en ;
            skos:definition "African as a subclass of Geographic Market or Continent refers to markets on the African continent."@en .


###  http://purl.org/holy/ns#Albania
holy:Albania rdf:type owl:NamedIndividual ,
                      schema:Country ;
             dbo:continent holy:Europe ;
             rdfs:label "Albania"@en .


###  http://purl.org/holy/ns#Algeria
holy:Algeria rdf:type owl:NamedIndividual ,
                      schema:Country ;
             dbo:continent holy:Africa ;
             rdfs:label "Algeria"@en .


###  http://purl.org/holy/ns#Ambazonia
holy:Ambazonia rdf:type owl:NamedIndividual ,
                        schema:Country ;
               dbo:continent holy:Africa ;
               rdfs:label "Ambazonia"@en .


###  http://purl.org/holy/ns#Andorra
holy:Andorra rdf:type owl:NamedIndividual ,
                      schema:Country ;
             dbo:continent holy:Europe ;
             rdfs:label "Andorra"@en .


###  http://purl.org/holy/ns#Angola
holy:Angola rdf:type owl:NamedIndividual ,
                     schema:Country ;
            dbo:continent holy:Africa ;
            rdfs:label "Angola"@en .


###  http://purl.org/holy/ns#Antigua_and_Barbuda
holy:Antigua_and_Barbuda rdf:type owl:NamedIndividual ,
                                  schema:Country ;
                         dbo:continent holy:North_America ;
                         rdfs:label "Antigua and Barbuda"@en .


###  http://purl.org/holy/ns#Argentina
holy:Argentina rdf:type owl:NamedIndividual ,
                        schema:Country ;
               dbo:continent holy:South_America ;
               rdfs:label "Argentina"@en .


###  http://purl.org/holy/ns#Armenia
holy:Armenia rdf:type owl:NamedIndividual ,
                      schema:Country ;
             dbo:continent holy:Europe ;
             rdfs:label "Armenia"@en .


###  http://purl.org/holy/ns#Asia
holy:Asia rdf:type owl:NamedIndividual ,
                   schema:Continent ;
          rdfs:label "Asia"@en .


###  http://purl.org/holy/ns#Australia
holy:Australia rdf:type owl:NamedIndividual ,
                        schema:Country ;
               dbo:continent holy:Oceania ;
               rdfs:label "Australia"@en .


###  http://purl.org/holy/ns#Austria
holy:Austria rdf:type owl:NamedIndividual ,
                      schema:Country ;
             dbo:continent holy:Europe ;
             rdfs:label "Austria"@en .


###  http://purl.org/holy/ns#AutomatedGuidedVehicle
holy:AutomatedGuidedVehicle rdf:type owl:NamedIndividual ,
                                     holy:MaterialHandlingVehicle ;
                            rdfs:label "Automated Guided Vehicle"@en .


###  http://purl.org/holy/ns#Azerbaijan
holy:Azerbaijan rdf:type owl:NamedIndividual ,
                         schema:Country ;
                dbo:continent holy:Europe ;
                rdfs:label "Azerbaijan"@en .


###  http://purl.org/holy/ns#Bahrain
holy:Bahrain rdf:type owl:NamedIndividual ,
                      schema:Country ;
             dbo:continent holy:Asia ;
             rdfs:label "Bahrain"@en .


###  http://purl.org/holy/ns#Bangladesh
holy:Bangladesh rdf:type owl:NamedIndividual ,
                         schema:Country ;
                dbo:continent holy:Asia ;
                rdfs:label "Bangladesh"@en .


###  http://purl.org/holy/ns#Barbados
holy:Barbados rdf:type owl:NamedIndividual ,
                       schema:Country ;
              dbo:continent holy:North_America ;
              rdfs:label "Barbados"@en .


###  http://purl.org/holy/ns#Belarus
holy:Belarus rdf:type owl:NamedIndividual ,
                      schema:Country ;
             dbo:continent holy:Europe ;
             rdfs:label "Belarus"@en .


###  http://purl.org/holy/ns#Belgium
holy:Belgium rdf:type owl:NamedIndividual ,
                      schema:Country ;
             dbo:continent holy:Europe ;
             rdfs:label "Belgium"@en .


###  http://purl.org/holy/ns#Belize
holy:Belize rdf:type owl:NamedIndividual ,
                     schema:Country ;
            dbo:continent holy:North_America ;
            rdfs:label "Belize"@en .


###  http://purl.org/holy/ns#Benin
holy:Benin rdf:type owl:NamedIndividual ,
                    schema:Country ;
           dbo:continent holy:Africa ;
           rdfs:label "Benin"@en .


###  http://purl.org/holy/ns#Bhutan
holy:Bhutan rdf:type owl:NamedIndividual ,
                     schema:Country ;
            dbo:continent holy:Asia ;
            rdfs:label "Bhutan"@en .


###  http://purl.org/holy/ns#Bolivia
holy:Bolivia rdf:type owl:NamedIndividual ,
                      schema:Country ;
             dbo:continent holy:South_America ;
             rdfs:label "Bolivia"@en .


###  http://purl.org/holy/ns#Bosnia_and_Herzegovina
holy:Bosnia_and_Herzegovina rdf:type owl:NamedIndividual ,
                                     schema:Country ;
                            dbo:continent holy:Europe ;
                            rdfs:label "Bosnia and Herzegovina"@en .


###  http://purl.org/holy/ns#Botswana
holy:Botswana rdf:type owl:NamedIndividual ,
                       schema:Country ;
              dbo:continent holy:Africa ;
              rdfs:label "Botswana"@en .


###  http://purl.org/holy/ns#Brazil
holy:Brazil rdf:type owl:NamedIndividual ,
                     schema:Country ;
            dbo:continent holy:South_America ;
            rdfs:label "Brazil"@en .


###  http://purl.org/holy/ns#Brunei
holy:Brunei rdf:type owl:NamedIndividual ,
                     schema:Country ;
            dbo:continent holy:Asia ;
            rdfs:label "Brunei"@en .


###  http://purl.org/holy/ns#Bulgaria
holy:Bulgaria rdf:type owl:NamedIndividual ,
                       schema:Country ;
              dbo:continent holy:Europe ;
              rdfs:label "Bulgaria"@en .


###  http://purl.org/holy/ns#Burkina_Faso
holy:Burkina_Faso rdf:type owl:NamedIndividual ,
                           schema:Country ;
                  dbo:continent holy:Africa ;
                  rdfs:label "Burkina Faso"@en .


###  http://purl.org/holy/ns#Burundi
holy:Burundi rdf:type owl:NamedIndividual ,
                      schema:Country ;
             dbo:continent holy:Africa ;
             rdfs:label "Burundi"@en .


###  http://purl.org/holy/ns#CUTE
holy:CUTE rdf:type owl:NamedIndividual ,
                   holy:InfrastructureProject ;
          holy:hasProject holy:Germany ,
                          holy:Netherlands ,
                          holy:Portugal ,
                          holy:Spain ,
                          holy:Sweden ,
                          holy:United_Kingdom ;
          holy:relatesToApplication dbr:Mercedes-Benz_Cito ;
          m4i:projectParticipant dbr:EvoBus ;
          dct:references <https://www.fuelcellbuses.eu/wiki/history-fuel-cell-electric-buses/cute-clean-urban-transport-europe-2001-2006> ;
          rdfs:label "CUTE"@en ;
          skos:altLabel "Clean Urban Transport for Europe"@en ;
          skos:definition """The Clean urban Transport for Europe (CUTE) was a European project which saw the deployment and testing of 27 Citaro fuel cell buses – three buses in each of nine cities in Europe (Hamburg, London, Barcelona, Stockholm, Porto, Stuttgart, Amsterdam, Luxembourg, and Madrid).
The aim of the project was to demonstrate the feasibility of an innovative, highly energy-efficient, clean urban public transport system. Different hydrogen production and refueling infrastructures were established in each of the cities. The project saw practical applications of renewable energy sources to the transport system.
The project greatly improved public acceptance of the hydrogen fuel cell transport system, and contributed to the development of a more secure energy supply for the EU."""@en .


###  http://purl.org/holy/ns#Cambodia
holy:Cambodia rdf:type owl:NamedIndividual ,
                       schema:Country ;
              dbo:continent holy:Asia ;
              rdfs:label "Cambodia"@en .


###  http://purl.org/holy/ns#Cameroon
holy:Cameroon rdf:type owl:NamedIndividual ,
                       schema:Country ;
              dbo:continent holy:Africa ;
              rdfs:label "Cameroon"@en .


###  http://purl.org/holy/ns#Canada
holy:Canada rdf:type owl:NamedIndividual ,
                     schema:Country ;
            dbo:continent holy:North_America ;
            rdfs:label "Canada"@en .


###  http://purl.org/holy/ns#Cape_Verde
holy:Cape_Verde rdf:type owl:NamedIndividual ,
                         schema:Country ;
                dbo:continent holy:Africa ;
                rdfs:label "Cape Verde"@en .


###  http://purl.org/holy/ns#Central_African_Republic
holy:Central_African_Republic rdf:type owl:NamedIndividual ,
                                       schema:Country ;
                              dbo:continent holy:Africa ;
                              rdfs:label "Central African Republic"@en .


###  http://purl.org/holy/ns#Ceres_Power_Holding
holy:Ceres_Power_Holding rdf:type owl:NamedIndividual ,
                                  holy:ManufacturingOrganization ;
                         holy:producesProduct holy:SteelCell ;
                         ebg:isPubliclyTraded "true"^^xsd:boolean ;
                         rdfs:label "Ceres Power Holding"@en ;
                         skos:altLabel "Ceres"@en ,
                                       "Ceres Power Holding Inc."@en ,
                                       "Ceres Power Holding plc"@en ,
                                       "LON:CWR"@en ,
                                       "LSE:CWR.L"@en ,
                                       "OTCMKTS:CPWHF"@en ;
                         skos:definition "Ceres Power Holdings plc is a United Kingdom-based fuel cell technology and engineering company. The Company is focused on developing power generation and hydrogen technologies. It operates through the solid oxide fuel cell (SOFC) technology segment. Its SteelCell technology can generate power from conventional fuels, such as natural gas and from sustainable fuels, which have biogas, ethanol or hydrogen. The Company's SteelCell technology is applicable to markets that have combined heat and power (CHP) for commercial and residential buildings. It also focuses to embed its technology in a range of market energy products for the commercial, residential and transportation markets. The Company's wholly owned subsidiary is Ceres Power Intermediate Holdings Ltd, which is engaged in the provision of overseas license and royalty services."@en .


###  http://purl.org/holy/ns#Chad
holy:Chad rdf:type owl:NamedIndividual ,
                   schema:Country ;
          dbo:continent holy:Africa ;
          rdfs:label "Chad"@en .


###  http://purl.org/holy/ns#Chile
holy:Chile rdf:type owl:NamedIndividual ,
                    schema:Country ;
           dbo:continent holy:South_America ;
           rdfs:label "Chile"@en .


###  http://purl.org/holy/ns#China
holy:China rdf:type owl:NamedIndividual ,
                    schema:Country ;
           dbo:continent holy:Asia ;
           rdfs:label "China"@en ;
           skos:altLabel "The People's Republic of China"@en .


###  http://purl.org/holy/ns#Colombia
holy:Colombia rdf:type owl:NamedIndividual ,
                       schema:Country ;
              dbo:continent holy:South_America ;
              rdfs:label "Colombia"@en .


###  http://purl.org/holy/ns#Comoros
holy:Comoros rdf:type owl:NamedIndividual ,
                      schema:Country ;
             dbo:continent holy:Africa ;
             rdfs:label "Comoros"@en .


###  http://purl.org/holy/ns#Cook_Islands
holy:Cook_Islands rdf:type owl:NamedIndividual ,
                           schema:Country ;
                  dbo:continent holy:Oceania ;
                  rdfs:label "Cook Islands"@en .


###  http://purl.org/holy/ns#Costa_Rica
holy:Costa_Rica rdf:type owl:NamedIndividual ,
                         schema:Country ;
                dbo:continent holy:North_America ;
                rdfs:label "Costa Rica"@en .


###  http://purl.org/holy/ns#Croatia
holy:Croatia rdf:type owl:NamedIndividual ,
                      schema:Country ;
             dbo:continent holy:Europe ;
             rdfs:label "Croatia"@en .


###  http://purl.org/holy/ns#CryogenicPistonPump
holy:CryogenicPistonPump rdf:type owl:NamedIndividual ,
                                  holy:HydrogenStorage ;
                         rdfs:label "Cryogenic piston pump"@en ;
                         skos:altLabel "CP model"@en ,
                                       "Cryo Pump"@en .


###  http://purl.org/holy/ns#Cuba
holy:Cuba rdf:type owl:NamedIndividual ,
                   schema:Country ;
          dbo:continent holy:North_America ;
          rdfs:label "Cuba"@en .


###  http://purl.org/holy/ns#Cyprus
holy:Cyprus rdf:type owl:NamedIndividual ,
                     schema:Country ;
            dbo:continent holy:Europe ;
            rdfs:label "Cyprus"@en .


###  http://purl.org/holy/ns#Czech_Republic
holy:Czech_Republic rdf:type owl:NamedIndividual ,
                             schema:Country ;
                    dbo:continent holy:Europe ;
                    rdfs:label "Czech Republic"@en .


###  http://purl.org/holy/ns#Democratic_Republic_of_the_Congo
holy:Democratic_Republic_of_the_Congo rdf:type owl:NamedIndividual ,
                                               schema:Country ;
                                      dbo:continent holy:Africa ;
                                      rdfs:label "Democratic Republic of the Congo"@en .


###  http://purl.org/holy/ns#Denmark
holy:Denmark rdf:type owl:NamedIndividual ,
                      schema:Country ;
             dbo:continent holy:Europe ;
             rdfs:label "Denmark"@en .


###  http://purl.org/holy/ns#Djibouti
holy:Djibouti rdf:type owl:NamedIndividual ,
                       schema:Country ;
              dbo:continent holy:Africa ;
              rdfs:label "Djibouti"@en .


###  http://purl.org/holy/ns#Dominica
holy:Dominica rdf:type owl:NamedIndividual ,
                       schema:Country ;
              dbo:continent holy:North_America ;
              rdfs:label "Dominica"@en .


###  http://purl.org/holy/ns#Dominican_Republic
holy:Dominican_Republic rdf:type owl:NamedIndividual ,
                                 schema:Country ;
                        dbo:continent holy:North_America ;
                        rdfs:label "Dominican Republic"@en .


###  http://purl.org/holy/ns#ECTOS
holy:ECTOS rdf:type owl:NamedIndividual ,
                    holy:InfrastructureProject ;
           holy:hasProject holy:Iceland ;
           holy:relatesToApplication dbr:Fuel_cell_bus ;
           m4i:projectParticipant dbr:Icelandic_New_Energy ;
           dct:references <https://en.wikipedia.org/wiki/Fuel_Cell_Bus_Club#CUTE> ;
           rdfs:label "ECTOS"@en ;
           skos:altLabel "Ecological City Transport System"@en ;
           skos:definition "ECTOS stands for Ecological City Transport System.[15][16] Icelandic New Energy was responsible for this project, the aim of which was to demonstrate \"state-of-the-art\" hydrogen technology by running part of the public transport system with fuel cell buses in the city Reykjavík, the capital of Iceland. Hydrogen was produced from domestic geothermal and hydro-powered energy sources by electrolysis. The project ran from 2001-2005.[8]"@en .


###  http://purl.org/holy/ns#East_Timor
holy:East_Timor rdf:type owl:NamedIndividual ,
                         schema:Country ;
                dbo:continent holy:Asia ;
                rdfs:label "East Timor"@en .


###  http://purl.org/holy/ns#Ecuador
holy:Ecuador rdf:type owl:NamedIndividual ,
                      schema:Country ;
             dbo:continent holy:South_America ;
             rdfs:label "Ecuador"@en .


###  http://purl.org/holy/ns#Egypt
holy:Egypt rdf:type owl:NamedIndividual ,
                    schema:Country ;
           dbo:continent holy:Africa ;
           rdfs:label "Egypt"@en .


###  http://purl.org/holy/ns#El_Salvador
holy:El_Salvador rdf:type owl:NamedIndividual ,
                          schema:Country ;
                 dbo:continent holy:North_America ;
                 rdfs:label "El Salvador"@en .


###  http://purl.org/holy/ns#Equatorial_Guinea
holy:Equatorial_Guinea rdf:type owl:NamedIndividual ,
                                schema:Country ;
                       dbo:continent holy:Africa ;
                       rdfs:label "Equatorial Guinea"@en .


###  http://purl.org/holy/ns#Eritrea
holy:Eritrea rdf:type owl:NamedIndividual ,
                      schema:Country ;
             dbo:continent holy:Africa ;
             rdfs:label "Eritrea"@en .


###  http://purl.org/holy/ns#Estonia
holy:Estonia rdf:type owl:NamedIndividual ,
                      schema:Country ;
             dbo:continent holy:Europe ;
             rdfs:label "Estonia"@en .


###  http://purl.org/holy/ns#Eswatini
holy:Eswatini rdf:type owl:NamedIndividual ,
                       schema:Country ;
              dbo:continent holy:Africa ;
              rdfs:label "Eswatini"@en .


###  http://purl.org/holy/ns#Ethiopia
holy:Ethiopia rdf:type owl:NamedIndividual ,
                       schema:Country ;
              dbo:continent holy:Africa ;
              rdfs:label "Ethiopia"@en .


###  http://purl.org/holy/ns#Europe
holy:Europe rdf:type owl:NamedIndividual ,
                     schema:Continent ;
            rdfs:label "Europe"@en ;
            skos:definition "European Market as a subclass of Geographic Market refers to markets on the European continent."@en .


###  http://purl.org/holy/ns#EuropeanCleanHydrogenAlliance
holy:EuropeanCleanHydrogenAlliance rdf:type owl:NamedIndividual ,
                                            schema:Project ;
                                   dct:references <https://ec.europa.eu/growth/industry/strategy/industrial-alliances/european-clean-hydrogen-alliance_en> ;
                                   rdfs:label "European Clean Hydrogen Alliance"@en ;
                                   skos:definition """The European Clean Hydrogen Alliance supports the large-scale deployment of clean hydrogen technologies by 2030 by bringing together renewable and low-carbon hydrogen production, demand in industry, mobility and other sectors, and hydrogen transmission and distribution. It aims to promote investments and stimulate the roll-out of clean hydrogen production and use. Set up in July 2020, the European Clean Hydrogen Alliance is part of EU efforts to ensure industrial leadership and accelerate the decarbonisation of industry in line with its climate change objectives.

The European Clean Hydrogen Alliance brings together industry, public authorities, civil society and other stakeholders. Alliance members meet twice a year in the Hydrogen Forum to discuss the large-scale deployment of clean hydrogen technologies and what this requires. Six thematic working groups (roundtablesSearch for available translations of the preceding linkEN•••) meet throughout the year and focus on the hydrogen value chain parts. See their report identifying the main barriers to the large-scale deployment of clean hydrogen and proposed mitigation measures under the related links section below.

On the occasion of its third Hydrogen Forum, the European Clean Hydrogen Alliance published a pipeline of projectsSearch for available translations of the preceding linkEN••• that European industry is undertaking to create the European hydrogen economy at a large scale. Featuring more than 750 projects, the pipeline is testimony to the size and dynamism of the European hydrogen economy. Projects are located in all four corners of Europe and range from clean hydrogen production to its use in industry, mobility, energy, and buildings.

Since the publication of the pipeline, the Commission entered agreements with the European Investment Bank and EIT InnoEnergy to advise project promoters individually on bankability and de-risking strategies, investment readiness, and due diligence preparations. They may also invest in individual projects and profile these to the financial investment community.

The alliance is open to all public and private actors with activities in renewable or low-carbon hydrogen that want to meet the membership criteria and actively contribute to the objectives set out in the declaration of the alliance. To join the alliance, an organisation must sign the declaration, which commits it to share the alliance's vision and contribute to its operational work."""@en .


###  http://purl.org/holy/ns#European_microstates
holy:European_microstates rdf:type owl:NamedIndividual ,
                                   schema:Country ;
                          dbo:continent holy:Europe ;
                          rdfs:label "European microstates"@en .


###  http://purl.org/holy/ns#Exqui.City18FuelCell
holy:Exqui.City18FuelCell rdf:type owl:NamedIndividual ,
                                   holy:Bus ;
                          rdfs:label "Exqui.City18 Fuel Cell"@en ;
                          skos:definition "A city bus series designed and produced by the company vanhool."@en .


###  http://purl.org/holy/ns#Exqui.City24FuelCell
holy:Exqui.City24FuelCell rdf:type owl:NamedIndividual ,
                                   holy:Bus ;
                          rdfs:label "Exqui.City24 Fuel Cell"@en ;
                          skos:definition "A city bus series designed and produced by the company vanhool."@en .


###  http://purl.org/holy/ns#Federated_States_of_Micronesia
holy:Federated_States_of_Micronesia rdf:type owl:NamedIndividual ,
                                             schema:Country ;
                                    dbo:continent holy:Oceania ;
                                    rdfs:label "Federated States of Micronesia"@en .


###  http://purl.org/holy/ns#Fiji
holy:Fiji rdf:type owl:NamedIndividual ,
                   schema:Country ;
          dbo:continent holy:Oceania ;
          rdfs:label "Fiji"@en .


###  http://purl.org/holy/ns#Finland
holy:Finland rdf:type owl:NamedIndividual ,
                      schema:Country ;
             dbo:continent holy:Europe ;
             rdfs:label "Finland"@en .


###  http://purl.org/holy/ns#Flags_of_Africa
holy:Flags_of_Africa rdf:type owl:NamedIndividual ,
                              schema:Country ;
                     dbo:continent holy:Africa ;
                     rdfs:label "Flags of Africa"@en .


###  http://purl.org/holy/ns#France
holy:France rdf:type owl:NamedIndividual ,
                     schema:Country ;
            dbo:continent holy:Europe ;
            rdfs:label "France"@en .


###  http://purl.org/holy/ns#Gabon
holy:Gabon rdf:type owl:NamedIndividual ,
                    schema:Country ;
           dbo:continent holy:Africa ;
           rdfs:label "Gabon"@en .


###  http://purl.org/holy/ns#GenSureFuelCellSystem
holy:GenSureFuelCellSystem rdf:type owl:NamedIndividual ,
                                    holy:HydrogenReconversion ;
                           holy:isUsedIn dbc:Material_Handling ;
                           holy:producesProduct dbr:Plug_Power ;
                           rdfs:label "GenSure fuel cell system"@en .


###  http://purl.org/holy/ns#Germany
holy:Germany rdf:type owl:NamedIndividual ,
                      schema:Country ;
             dbo:continent holy:Europe ;
             rdfs:label "Germany"@en .


###  http://purl.org/holy/ns#Ghana
holy:Ghana rdf:type owl:NamedIndividual ,
                    schema:Country ;
           dbo:continent holy:Africa ;
           rdfs:label "Ghana"@en .


###  http://purl.org/holy/ns#Greece
holy:Greece rdf:type owl:NamedIndividual ,
                     schema:Country ;
            dbo:continent holy:Europe ;
            rdfs:label "Greece"@en .


###  http://purl.org/holy/ns#Grenada
holy:Grenada rdf:type owl:NamedIndividual ,
                      schema:Country ;
             dbo:continent holy:North_America ;
             rdfs:label "Grenada"@en .


###  http://purl.org/holy/ns#Guatemala
holy:Guatemala rdf:type owl:NamedIndividual ,
                        schema:Country ;
               dbo:continent holy:North_America ;
               rdfs:label "Guatemala"@en .


###  http://purl.org/holy/ns#Guinea
holy:Guinea rdf:type owl:NamedIndividual ,
                     schema:Country ;
            dbo:continent holy:Africa ;
            rdfs:label "Guinea"@en .


###  http://purl.org/holy/ns#Guinea-Bissau
holy:Guinea-Bissau rdf:type owl:NamedIndividual ,
                            schema:Country ;
                   dbo:continent holy:Africa ;
                   rdfs:label "Guinea-Bissau"@en .


###  http://purl.org/holy/ns#Guyana
holy:Guyana rdf:type owl:NamedIndividual ,
                     schema:Country ;
            dbo:continent holy:South_America ;
            rdfs:label "Guyana"@en .


###  http://purl.org/holy/ns#Haiti
holy:Haiti rdf:type owl:NamedIndividual ,
                    schema:Country ;
           dbo:continent holy:North_America ;
           rdfs:label "Haiti"@en .


###  http://purl.org/holy/ns#Honduras
holy:Honduras rdf:type owl:NamedIndividual ,
                       schema:Country ;
              dbo:continent holy:North_America ;
              rdfs:label "Honduras"@en .


###  http://purl.org/holy/ns#Hungary
holy:Hungary rdf:type owl:NamedIndividual ,
                      schema:Country ;
             dbo:continent holy:Europe ;
             rdfs:label "Hungary"@en .


###  http://purl.org/holy/ns#Hydroflex
holy:Hydroflex rdf:type owl:NamedIndividual ,
                        holy:PassengerTrain .


###  http://purl.org/holy/ns#HyzonClass8
holy:HyzonClass8 rdf:type owl:NamedIndividual ,
                          holy:LongHaulTruck ;
                 holy:applicationSoldIn holy:North_America ;
                 holy:isProvidedBy dbr:Hyzon_Motors ;
                 holy:usesProduct dbr:Proton-exchange_membrane_fuel_cell ;
                 holy:usesTechnology holy:Hyzon_hybrid_bi-polar_plate_technology ;
                 rdfs:label "Hyzon Class 8"@en ;
                 skos:definition "Long Haul Truck manufactured by Hyzon Motors having a driving range up to 500 miles. Power: 450 kW/603 hp peak/ 15 minute refueling time"@en .


###  http://purl.org/holy/ns#HyzonDrayage
holy:HyzonDrayage rdf:type owl:NamedIndividual ,
                           holy:LongHaulTruck ;
                  holy:applicationSoldIn holy:North_America ;
                  holy:isProvidedBy dbr:Hyzon_Motors .


###  http://purl.org/holy/ns#HyzonEconicRefuse
holy:HyzonEconicRefuse rdf:type owl:NamedIndividual ,
                                holy:RegionalTruck ;
                       holy:applicationSoldIn dbr:Europe ,
                                              holy:North_America ;
                       rdfs:label "Hyzon Econic Refuse"@en ;
                       skos:definition "Truck with a 125 mile range and 435 hp."@en .


###  http://purl.org/holy/ns#HyzonHighFloorCoach
holy:HyzonHighFloorCoach rdf:type owl:NamedIndividual ,
                                  holy:Bus ;
                         holy:applicationSoldIn dbr:Europe ,
                                                holy:Asia ,
                                                holy:North_America ;
                         holy:isProvidedBy dbr:Hyzon_Motors ;
                         rdfs:label "Hyzon High-Floor Coach"@en ;
                         skos:definition "A bus with a range of 200-250 miles and 261 hp."@en .


###  http://purl.org/holy/ns#HyzonHymaxSeries
holy:HyzonHymaxSeries rdf:type owl:NamedIndividual ,
                               holy:LongHaulTruck ;
                      holy:applicationSoldIn dbr:Europe ,
                                             holy:Asia ;
                      holy:isProvidedBy dbr:Hyzon_Motors ;
                      holy:usesProduct dbr:Proton-exchange_membrane_fuel_cell ;
                      holy:usesTechnology holy:Hyzon_hybrid_bi-polar_plate_technology ;
                      rdfs:label "Hyzon Hymax Series"@en ;
                      skos:definition "Long Haul Truck manufactured by Hyzon Motors having a driving range up to 400-560 kilometers"@en .


###  http://purl.org/holy/ns#Hyzon_hybrid_bi-polar_plate_technology
holy:Hyzon_hybrid_bi-polar_plate_technology rdf:type owl:NamedIndividual ,
                                                     holy:BipolarPlate ;
                                            holy:isUsedIn holy:HyzonClass8 ,
                                                          holy:HyzonHymaxSeries ;
                                            holy:producesProduct dbr:Hyzon_Motors ;
                                            dct:references <https://www.hyzonmotors.com/innovation> ;
                                            rdfs:label "Hyzon's hybrid bi-polar plate technology"@en ;
                                            skos:altLabel "Hyzon bi-polar plate"@en ;
                                            skos:definition "A proprietary technology of Hyzon Motors for its PEM fuel cells."@en .


###  http://purl.org/holy/ns#Iceland
holy:Iceland rdf:type owl:NamedIndividual ,
                      schema:Country ;
             dbo:continent holy:Europe ;
             holy:hasProject holy:ECTOS ;
             rdfs:label "Iceland"@en .


###  http://purl.org/holy/ns#India
holy:India rdf:type owl:NamedIndividual ,
                    schema:Country ;
           dbo:continent holy:Asia ;
           rdfs:label "India"@en .


###  http://purl.org/holy/ns#Indonesia
holy:Indonesia rdf:type owl:NamedIndividual ,
                        schema:Country ;
               dbo:continent holy:Asia ;
               rdfs:label "Indonesia"@en .


###  http://purl.org/holy/ns#IonicCompressor50
holy:IonicCompressor50 rdf:type owl:NamedIndividual ,
                                holy:HydrogenStorage ;
                       dct:references <https://www.linde-engineering.com/en/images/DS_IC%2050_tcm19-523715.pdf> ;
                       rdfs:label "Ionic Compressor 50"@en ;
                       skos:altLabel "IC family"@en ,
                                     "IC model"@en ;
                       skos:definition "Linde's ground-breaking ionic compression technology leads the way to the next generation of safe, fast and efficient hydrogen fuelling. The ionic compressor 50 is a high-performance, easy-to-maintain solution with a listed design. It allows for quick, safe, highly efficient and economical fuelling of hydrogen vehicles at 25MPa and 35 MPa. This is achieved by an innovative compression system, the ionic compressor, where, instead of a mechanical piston, a column of ionic fluid is in direct contact with the gaseous hydrogen. This allows for the continuous high-performance, fast fuelling of hydrogen vehicles. It is designed to fuel 25-MPa and 35-MPa vehicles with the highest filling levels while considerably reducing operating costs. It is used for gaseous hydrogen."@en .


###  http://purl.org/holy/ns#Iran
holy:Iran rdf:type owl:NamedIndividual ,
                   schema:Country ;
          dbo:continent holy:Asia ;
          rdfs:label "Iran"@en .


###  http://purl.org/holy/ns#Iraq
holy:Iraq rdf:type owl:NamedIndividual ,
                   schema:Country ;
          dbo:continent holy:Asia ;
          rdfs:label "Iraq"@en .


###  http://purl.org/holy/ns#Israel
holy:Israel rdf:type owl:NamedIndividual ,
                     schema:Country ;
            dbo:continent holy:Asia ;
            rdfs:label "Israel"@en .


###  http://purl.org/holy/ns#Italy
holy:Italy rdf:type owl:NamedIndividual ,
                    schema:Country ;
           dbo:continent holy:Europe ;
           rdfs:label "Italy"@en .


###  http://purl.org/holy/ns#Ivory_Coast
holy:Ivory_Coast rdf:type owl:NamedIndividual ,
                          schema:Country ;
                 dbo:continent holy:Africa ;
                 rdfs:label "Ivory Coast"@en .


###  http://purl.org/holy/ns#Jamaica
holy:Jamaica rdf:type owl:NamedIndividual ,
                      schema:Country ;
             dbo:continent holy:North_America ;
             rdfs:label "Jamaica"@en .


###  http://purl.org/holy/ns#Jordan
holy:Jordan rdf:type owl:NamedIndividual ,
                     schema:Country ;
            dbo:continent holy:Asia ;
            rdfs:label "Jordan"@en .


###  http://purl.org/holy/ns#Kazakhstan
holy:Kazakhstan rdf:type owl:NamedIndividual ,
                         schema:Country ;
                dbo:continent holy:Asia ;
                rdfs:label "Kazakhstan"@en .


###  http://purl.org/holy/ns#Kenya
holy:Kenya rdf:type owl:NamedIndividual ,
                    schema:Country ;
           dbo:continent holy:Africa ;
           rdfs:label "Kenya"@en .


###  http://purl.org/holy/ns#Kiribati
holy:Kiribati rdf:type owl:NamedIndividual ,
                       schema:Country ;
              dbo:continent holy:Oceania ;
              rdfs:label "Kiribati"@en .


###  http://purl.org/holy/ns#Kosovo
holy:Kosovo rdf:type owl:NamedIndividual ,
                     schema:Country ;
            dbo:continent holy:Europe ;
            rdfs:label "Kosovo"@en .


###  http://purl.org/holy/ns#Kuwait
holy:Kuwait rdf:type owl:NamedIndividual ,
                     schema:Country ;
            dbo:continent holy:Asia ;
            rdfs:label "Kuwait"@en .


###  http://purl.org/holy/ns#Kyrgyzstan
holy:Kyrgyzstan rdf:type owl:NamedIndividual ,
                         schema:Country ;
                dbo:continent holy:Asia ;
                rdfs:label "Kyrgyzstan"@en .


###  http://purl.org/holy/ns#Laos
holy:Laos rdf:type owl:NamedIndividual ,
                   schema:Country ;
          dbo:continent holy:Asia ;
          rdfs:label "Laos"@en .


###  http://purl.org/holy/ns#Latvia
holy:Latvia rdf:type owl:NamedIndividual ,
                     schema:Country ;
            dbo:continent holy:Europe ;
            rdfs:label "Latvia"@en .


###  http://purl.org/holy/ns#Lebanon
holy:Lebanon rdf:type owl:NamedIndividual ,
                      schema:Country ;
             dbo:continent holy:Asia ;
             rdfs:label "Lebanon"@en .


###  http://purl.org/holy/ns#Lesotho
holy:Lesotho rdf:type owl:NamedIndividual ,
                      schema:Country ;
             dbo:continent holy:Africa ;
             rdfs:label "Lesotho"@en .


###  http://purl.org/holy/ns#Liberia
holy:Liberia rdf:type owl:NamedIndividual ,
                      schema:Country ;
             dbo:continent holy:Africa ;
             rdfs:label "Liberia"@en .


###  http://purl.org/holy/ns#Libya
holy:Libya rdf:type owl:NamedIndividual ,
                    schema:Country ;
           dbo:continent holy:Africa ;
           rdfs:label "Libya"@en .


###  http://purl.org/holy/ns#Liechtenstein
holy:Liechtenstein rdf:type owl:NamedIndividual ,
                            schema:Country ;
                   dbo:continent holy:Europe ;
                   rdfs:label "Liechtenstein"@en .


###  http://purl.org/holy/ns#Lithuania
holy:Lithuania rdf:type owl:NamedIndividual ,
                        schema:Country ;
               dbo:continent holy:Europe ;
               rdfs:label "Lithuania"@en .


###  http://purl.org/holy/ns#Luxembourg
holy:Luxembourg rdf:type owl:NamedIndividual ,
                         schema:Country ;
                dbo:continent holy:Europe ;
                rdfs:label "Luxembourg"@en .


###  http://purl.org/holy/ns#Madagascar
holy:Madagascar rdf:type owl:NamedIndividual ,
                         schema:Country ;
                dbo:continent holy:Africa ;
                rdfs:label "Madagascar"@en .


###  http://purl.org/holy/ns#Malawi
holy:Malawi rdf:type owl:NamedIndividual ,
                     schema:Country ;
            dbo:continent holy:Africa ;
            rdfs:label "Malawi"@en .


###  http://purl.org/holy/ns#Malaysia
holy:Malaysia rdf:type owl:NamedIndividual ,
                       schema:Country ;
              dbo:continent holy:Asia ;
              rdfs:label "Malaysia"@en .


###  http://purl.org/holy/ns#Maldives
holy:Maldives rdf:type owl:NamedIndividual ,
                       schema:Country ;
              dbo:continent holy:Asia ;
              rdfs:label "Maldives"@en .


###  http://purl.org/holy/ns#Mali
holy:Mali rdf:type owl:NamedIndividual ,
                   schema:Country ;
          dbo:continent holy:Africa ;
          rdfs:label "Mali"@en .


###  http://purl.org/holy/ns#Malta
holy:Malta rdf:type owl:NamedIndividual ,
                    schema:Country ;
           dbo:continent holy:Europe ;
           rdfs:label "Malta"@en .


###  http://purl.org/holy/ns#ManUpOrderpicker
holy:ManUpOrderpicker rdf:type owl:NamedIndividual ,
                               holy:MaterialHandlingVehicle ;
                      rdfs:label "Man-Up Orderpicker"@en .


###  http://purl.org/holy/ns#Marshall_Islands
holy:Marshall_Islands rdf:type owl:NamedIndividual ,
                               schema:Country ;
                      dbo:continent holy:Oceania ;
                      rdfs:label "Marshall Islands"@en .


###  http://purl.org/holy/ns#Mauritania
holy:Mauritania rdf:type owl:NamedIndividual ,
                         schema:Country ;
                dbo:continent holy:Africa ;
                rdfs:label "Mauritania"@en .


###  http://purl.org/holy/ns#Mauritius
holy:Mauritius rdf:type owl:NamedIndividual ,
                        schema:Country ;
               dbo:continent holy:Africa ;
               rdfs:label "Mauritius"@en .


###  http://purl.org/holy/ns#Mexico
holy:Mexico rdf:type owl:NamedIndividual ,
                     schema:Country ;
            dbo:continent holy:North_America ;
            rdfs:label "Mexico"@en .


###  http://purl.org/holy/ns#Moldova
holy:Moldova rdf:type owl:NamedIndividual ,
                      schema:Country ;
             dbo:continent holy:Europe ;
             rdfs:label "Moldova"@en .


###  http://purl.org/holy/ns#Monaco
holy:Monaco rdf:type owl:NamedIndividual ,
                     schema:Country ;
            dbo:continent holy:Europe ;
            rdfs:label "Monaco"@en .


###  http://purl.org/holy/ns#Mongolia
holy:Mongolia rdf:type owl:NamedIndividual ,
                       schema:Country ;
              dbo:continent holy:Asia ;
              rdfs:label "Mongolia"@en .


###  http://purl.org/holy/ns#Montenegro
holy:Montenegro rdf:type owl:NamedIndividual ,
                         schema:Country ;
                dbo:continent holy:Europe ;
                rdfs:label "Montenegro"@en .


###  http://purl.org/holy/ns#Morocco
holy:Morocco rdf:type owl:NamedIndividual ,
                      schema:Country ;
             dbo:continent holy:Africa ;
             rdfs:label "Morocco"@en .


###  http://purl.org/holy/ns#Mozambique
holy:Mozambique rdf:type owl:NamedIndividual ,
                         schema:Country ;
                dbo:continent holy:Africa ;
                rdfs:label "Mozambique"@en .


###  http://purl.org/holy/ns#Myanmar
holy:Myanmar rdf:type owl:NamedIndividual ,
                      schema:Country ;
             dbo:continent holy:Asia ;
             rdfs:label "Myanmar"@en .


###  http://purl.org/holy/ns#Namibia
holy:Namibia rdf:type owl:NamedIndividual ,
                      schema:Country ;
             dbo:continent holy:Africa ;
             rdfs:label "Namibia"@en .


###  http://purl.org/holy/ns#NationalInnovationProgrammeHydrogenandFuelCellTechnology
holy:NationalInnovationProgrammeHydrogenandFuelCellTechnology rdf:type owl:NamedIndividual ,
                                                                       schema:Project ;
                                                              m4i:projectParticipant dbr:Federal_Ministry_of_Transport_and_Digital_Infrastructure ;
                                                              dct:references <https://www.ptj.de/en/project-funding/nip> ;
                                                              rdfs:label "National Innovation Programme Hydrogen and Fuel Cell Technology"@en ;
                                                              skos:altLabel "NIP"@en ;
                                                              skos:definition "The National Innovation Programme Hydrogen and Fuel Cell Technology (NIP) in an interdepartmental programme for research and development funding that has been in place since 2007. The Federal Ministry of Transport and Digital Infrastructure (BMVI) made a significant contribution of 500 million euro between 2007 and 2016. Thus far, the aim of the NIP has been to prepare the market for these types of technologies in accordance with existing research, development and innovation (R&D&I) directives. The long-term, ten-year programme therefore contributed to the emergence of an internationally competitive industrial sector based on stable framework conditions and funding opportunities in Germany. Now that the launch of fuel cell products is in the early stages and a hydrogen infrastructure for transport is being developed, the NIP needs to be realigned in its second phase. The objective is to make hydrogen and fuel cell technology competitive in the transport sector and the energy market by the middle of the next decade. This can only be achieved with a continued joint effort of all stakeholders."@en .


###  http://purl.org/holy/ns#Nauru
holy:Nauru rdf:type owl:NamedIndividual ,
                    schema:Country ;
           dbo:continent holy:Oceania ;
           rdfs:label "Nauru"@en .


###  http://purl.org/holy/ns#Nepal
holy:Nepal rdf:type owl:NamedIndividual ,
                    schema:Country ;
           dbo:continent holy:Asia ;
           rdfs:label "Nepal"@en .


###  http://purl.org/holy/ns#Netherlands
holy:Netherlands rdf:type owl:NamedIndividual ,
                          schema:Country ;
                 dbo:continent holy:Europe ;
                 rdfs:label "Netherlands"@en .


###  http://purl.org/holy/ns#New_Zealand
holy:New_Zealand rdf:type owl:NamedIndividual ,
                          schema:Country ;
                 dbo:continent holy:Oceania ;
                 rdfs:label "New Zealand"@en .


###  http://purl.org/holy/ns#Nicaragua
holy:Nicaragua rdf:type owl:NamedIndividual ,
                        schema:Country ;
               dbo:continent holy:North_America ;
               rdfs:label "Nicaragua"@en .


###  http://purl.org/holy/ns#Niger
holy:Niger rdf:type owl:NamedIndividual ,
                    schema:Country ;
           dbo:continent holy:Africa ;
           rdfs:label "Niger"@en .


###  http://purl.org/holy/ns#Nigeria
holy:Nigeria rdf:type owl:NamedIndividual ,
                      schema:Country ;
             dbo:continent holy:Africa ;
             rdfs:label "Nigeria"@en .


###  http://purl.org/holy/ns#Niue
holy:Niue rdf:type owl:NamedIndividual ,
                   schema:Country ;
          dbo:continent holy:Oceania ;
          rdfs:label "Niue"@en .


###  http://purl.org/holy/ns#North_America
holy:North_America rdf:type owl:NamedIndividual ,
                            schema:Continent ;
                   rdfs:label "North America"@en .


###  http://purl.org/holy/ns#North_Macedonia
holy:North_Macedonia rdf:type owl:NamedIndividual ,
                              schema:Country ;
                     dbo:continent holy:Europe ;
                     rdfs:label "North Macedonia"@en .


###  http://purl.org/holy/ns#NorthernPeripheryandArcticProgramme
holy:NorthernPeripheryandArcticProgramme rdf:type owl:NamedIndividual ,
                                                  org:Organization ;
                                         dct:references <https://www.interreg-npa.eu/about/programme-in-brief/> ;
                                         rdfs:label "Northern Periphery and Arctic Programme"@en ;
                                         skos:definition "The Northern Periphery and Arctic 2014-2020 forms a cooperation between 9 programme partner countries. The NPA 2014-2020 is part of Interreg, supported by the European Regional Development Fund (ERDF) and ERDF equivalent funding from non EU partner countries. Despite geographical differences, the large programme area shares a number of joint challenges and opportunities that can best be overcome and realised by transnational cooperation."@en .


###  http://purl.org/holy/ns#Norway
holy:Norway rdf:type owl:NamedIndividual ,
                     schema:Country ;
            dbo:continent holy:Europe ;
            rdfs:label "Norway"@en .


###  http://purl.org/holy/ns#OWLNamedIndividual_7f4f3263_d74c_4f58_a998_c670b97905fa
holy:OWLNamedIndividual_7f4f3263_d74c_4f58_a998_c670b97905fa rdf:type owl:NamedIndividual ,
                                                                      holy:LongHaulTruck ;
                                                             holy:isProvidedBy dbr:Hyzon_Motors ;
                                                             holy:usesProduct dbr:Proton-exchange_membrane_fuel_cell ;
                                                             holy:usesTechnology holy:Hyzon_hybrid_bi-polar_plate_technology ;
                                                             rdfs:label "Hyzon Vehicle"@en .


###  http://purl.org/holy/ns#Oceania
holy:Oceania rdf:type owl:NamedIndividual ,
                      schema:Continent ;
             rdfs:label "Oceania"@en .


###  http://purl.org/holy/ns#Oman
holy:Oman rdf:type owl:NamedIndividual ,
                   schema:Country ;
          dbo:continent holy:Asia ;
          rdfs:label "Oman"@en .


###  http://purl.org/holy/ns#Pakistan
holy:Pakistan rdf:type owl:NamedIndividual ,
                       schema:Country ;
              dbo:continent holy:Asia ;
              rdfs:label "Pakistan"@en .


###  http://purl.org/holy/ns#Palau
holy:Palau rdf:type owl:NamedIndividual ,
                    schema:Country ;
           dbo:continent holy:Oceania ;
           rdfs:label "Palau"@en .


###  http://purl.org/holy/ns#Panama
holy:Panama rdf:type owl:NamedIndividual ,
                     schema:Country ;
            dbo:continent holy:North_America ;
            rdfs:label "Panama"@en .


###  http://purl.org/holy/ns#Papua_New_Guinea
holy:Papua_New_Guinea rdf:type owl:NamedIndividual ,
                               schema:Country ;
                      dbo:continent holy:Oceania ;
                      rdfs:label "Papua New Guinea"@en .


###  http://purl.org/holy/ns#Paraguay
holy:Paraguay rdf:type owl:NamedIndividual ,
                       schema:Country ;
              dbo:continent holy:South_America ;
              rdfs:label "Paraguay"@en .


###  http://purl.org/holy/ns#Peru
holy:Peru rdf:type owl:NamedIndividual ,
                   schema:Country ;
          dbo:continent holy:South_America ;
          rdfs:label "Peru"@en .


###  http://purl.org/holy/ns#Philippines
holy:Philippines rdf:type owl:NamedIndividual ,
                          schema:Country ;
                 dbo:continent holy:Asia ;
                 rdfs:label "Philippines"@en .


###  http://purl.org/holy/ns#Poland
holy:Poland rdf:type owl:NamedIndividual ,
                     schema:Country ;
            dbo:continent holy:Europe ;
            rdfs:label "Poland"@en .


###  http://purl.org/holy/ns#Portugal
holy:Portugal rdf:type owl:NamedIndividual ,
                       schema:Country ;
              dbo:continent holy:Europe ;
              rdfs:label "Portugal"@en .


###  http://purl.org/holy/ns#Qatar
holy:Qatar rdf:type owl:NamedIndividual ,
                    schema:Country ;
           dbo:continent holy:Asia ;
           rdfs:label "Qatar"@en .


###  http://purl.org/holy/ns#Republic_of_Ireland
holy:Republic_of_Ireland rdf:type owl:NamedIndividual ,
                                  schema:Country ;
                         dbo:continent holy:Europe ;
                         rdfs:label "Republic of Ireland"@en .


###  http://purl.org/holy/ns#Republic_of_the_Congo
holy:Republic_of_the_Congo rdf:type owl:NamedIndividual ,
                                    schema:Country ;
                           dbo:continent holy:Africa ;
                           rdfs:label "Republic of the Congo"@en .


###  http://purl.org/holy/ns#Romania
holy:Romania rdf:type owl:NamedIndividual ,
                      schema:Country ;
             dbo:continent holy:Europe ;
             rdfs:label "Romania"@en .


###  http://purl.org/holy/ns#Russia
holy:Russia rdf:type owl:NamedIndividual ,
                     schema:Country ;
            dbo:continent holy:Asia ;
            rdfs:label "Russia"@en .


###  http://purl.org/holy/ns#Rwanda
holy:Rwanda rdf:type owl:NamedIndividual ,
                     schema:Country ;
            dbo:continent holy:Africa ;
            rdfs:label "Rwanda"@en .


###  http://purl.org/holy/ns#Sahrawi_Arab_Democratic_Republic
holy:Sahrawi_Arab_Democratic_Republic rdf:type owl:NamedIndividual ,
                                               schema:Country ;
                                      dbo:continent holy:Africa ;
                                      rdfs:label "Sahrawi Arab Democratic Republic"@en .


###  http://purl.org/holy/ns#Saint_Kitts_and_Nevis
holy:Saint_Kitts_and_Nevis rdf:type owl:NamedIndividual ,
                                    schema:Country ;
                           dbo:continent holy:North_America ;
                           rdfs:label "Saint Kitts and Nevis"@en .


###  http://purl.org/holy/ns#Saint_Lucia
holy:Saint_Lucia rdf:type owl:NamedIndividual ,
                          schema:Country ;
                 dbo:continent holy:North_America ;
                 rdfs:label "Saint Lucia"@en .


###  http://purl.org/holy/ns#Saint_Vincent_and_the_Grenadines
holy:Saint_Vincent_and_the_Grenadines rdf:type owl:NamedIndividual ,
                                               schema:Country ;
                                      dbo:continent holy:North_America ;
                                      rdfs:label "Saint Vincent and the Grenadines"@en .


###  http://purl.org/holy/ns#Samoa
holy:Samoa rdf:type owl:NamedIndividual ,
                    schema:Country ;
           dbo:continent holy:Oceania ;
           rdfs:label "Samoa"@en .


###  http://purl.org/holy/ns#San_Marino
holy:San_Marino rdf:type owl:NamedIndividual ,
                         schema:Country ;
                dbo:continent holy:Europe ;
                rdfs:label "San Marino"@en .


###  http://purl.org/holy/ns#Saudi_Arabia
holy:Saudi_Arabia rdf:type owl:NamedIndividual ,
                           schema:Country ;
                  dbo:continent holy:Asia ;
                  rdfs:label "Saudi Arabia"@en .


###  http://purl.org/holy/ns#Senegal
holy:Senegal rdf:type owl:NamedIndividual ,
                      schema:Country ;
             dbo:continent holy:Africa ;
             rdfs:label "Senegal"@en .


###  http://purl.org/holy/ns#Serbia
holy:Serbia rdf:type owl:NamedIndividual ,
                     schema:Country ;
            dbo:continent holy:Europe ;
            rdfs:label "Serbia"@en .


###  http://purl.org/holy/ns#Seychelles
holy:Seychelles rdf:type owl:NamedIndividual ,
                         schema:Country ;
                dbo:continent holy:Africa ;
                rdfs:label "Seychelles"@en .


###  http://purl.org/holy/ns#Sierra_Leone
holy:Sierra_Leone rdf:type owl:NamedIndividual ,
                           schema:Country ;
                  dbo:continent holy:Africa ;
                  rdfs:label "Sierra Leone"@en .


###  http://purl.org/holy/ns#Singapore
holy:Singapore rdf:type owl:NamedIndividual ,
                        schema:Country ;
               dbo:continent holy:Asia ;
               rdfs:label "Singapore"@en .


###  http://purl.org/holy/ns#Slovakia
holy:Slovakia rdf:type owl:NamedIndividual ,
                       schema:Country ;
              dbo:continent holy:Europe ;
              rdfs:label "Slovakia"@en .


###  http://purl.org/holy/ns#Slovenia
holy:Slovenia rdf:type owl:NamedIndividual ,
                       schema:Country ;
              dbo:continent holy:Europe ;
              rdfs:label "Slovenia"@en .


###  http://purl.org/holy/ns#Solomon_Islands
holy:Solomon_Islands rdf:type owl:NamedIndividual ,
                              schema:Country ;
                     dbo:continent holy:Oceania ;
                     rdfs:label "Solomon Islands"@en .


###  http://purl.org/holy/ns#Somalia
holy:Somalia rdf:type owl:NamedIndividual ,
                      schema:Country ;
             dbo:continent holy:Africa ;
             rdfs:label "Somalia"@en .


###  http://purl.org/holy/ns#Somaliland
holy:Somaliland rdf:type owl:NamedIndividual ,
                         schema:Country ;
                dbo:continent holy:Africa ;
                rdfs:label "Somaliland"@en .


###  http://purl.org/holy/ns#South_Africa
holy:South_Africa rdf:type owl:NamedIndividual ,
                           schema:Country ;
                  dbo:continent holy:Africa ;
                  rdfs:label "South Africa"@en .


###  http://purl.org/holy/ns#South_America
holy:South_America rdf:type owl:NamedIndividual ,
                            schema:Continent ;
                   rdfs:label "South America"@en .


###  http://purl.org/holy/ns#South_Sudan
holy:South_Sudan rdf:type owl:NamedIndividual ,
                          schema:Country ;
                 dbo:continent holy:Africa ;
                 rdfs:label "South Sudan"@en .


###  http://purl.org/holy/ns#Spain
holy:Spain rdf:type owl:NamedIndividual ,
                    schema:Country ;
           dbo:continent holy:Europe ;
           rdfs:label "Spain"@en .


###  http://purl.org/holy/ns#Sri_Lanka
holy:Sri_Lanka rdf:type owl:NamedIndividual ,
                        schema:Country ;
               dbo:continent holy:Asia ;
               rdfs:label "Sri Lanka"@en .


###  http://purl.org/holy/ns#StandUpCounterbalancedTruck
holy:StandUpCounterbalancedTruck rdf:type owl:NamedIndividual ,
                                          holy:MaterialHandlingVehicle ;
                                 rdfs:label "Stand-Up Counterbalanced Truck"@en .


###  http://purl.org/holy/ns#StandUpReachTruck
holy:StandUpReachTruck rdf:type owl:NamedIndividual ,
                                holy:MaterialHandlingVehicle ;
                       rdfs:label "Stand-Up Reach Truck"@en .


###  http://purl.org/holy/ns#SteelCell
holy:SteelCell rdf:type owl:NamedIndividual ,
                        holy:SolidOxideFuelCell ;
               holy:isUsedIn dbr:combined_heat_and_power_station ;
               rdfs:label "SteelCell®"@en ;
               skos:altLabel "Ceres Steel Cell"@en ,
                             "Steel Cell technology"@en ,
                             "SteelCell technology"@en ,
                             "SteelCell® technology"@en ;
               skos:definition "Definition by Ceres: As a Solid Oxide Fuel Cell (SOFC), the SteelCell® can use conventional fuels like mains natural gas from the existing infrastructure and can make an immediate improvement to energy costs, CO2 emissions and energy security for businesses, homes and vehicles."@en .


###  http://purl.org/holy/ns#Sudan
holy:Sudan rdf:type owl:NamedIndividual ,
                    schema:Country ;
           dbo:continent holy:Africa ;
           rdfs:label "Sudan"@en .


###  http://purl.org/holy/ns#SureSource1500TM
holy:SureSource1500TM rdf:type owl:NamedIndividual ,
                               holy:MoltenCarbonateFuelCell ;
                      dct:references <https://www.fuelcellenergy.com/products/> ;
                      rdfs:label "SureSource 1500TM"@en ;
                      skos:altLabel "Sure Source 1500"@en ;
                      skos:definition "This solution is ideal for on-site power generation for large installations requiring continuous power and value high-quality heat for facility heating and/or absorption chilling. The system is suitable for a wide range of applications, including wastewater treatment plants, manufacturing facilities, hospitals and universities. Output: 1.4 megawatts."@en .


###  http://purl.org/holy/ns#SureSource3000TM
holy:SureSource3000TM rdf:type owl:NamedIndividual ,
                               holy:MoltenCarbonateFuelCell ;
                      dct:references <https://www.fuelcellenergy.com/products/> ;
                      rdfs:label "SureSource 300TM"@en ;
                      skos:altLabel "Sure Source 3000"@en ;
                      skos:definition "Comprised of two 1.4 megawatt (MW) modules, the SureSource 3000 generates 2.8 MW of ultra-clean power. Similar to the SureSource 1500, the system is well-suited for on-site applications and caters to customers with an even greater power load requirement. Ideal applications include large universities, manufacturing facilities, wastewater treatment plants or for multi-plant fuel cell parks to support the electric grid. Output: 2.8 megawatts"@en .


###  http://purl.org/holy/ns#SureSource4000TM
holy:SureSource4000TM rdf:type owl:NamedIndividual ,
                               holy:MoltenCarbonateFuelCell ;
                      dct:references <https://www.fuelcellenergy.com/products/> ;
                      rdfs:label "SureSource 4000TM"@en ;
                      skos:altLabel "Sure Source 4000"@en ;
                      skos:definition "The SureSource 4000 is the largest in the SureSource power plant fleet and generates 3.7 megawatts (MW) of ultra-clean power with an industry-leading electrical efficiency of approximately 60%. This enhanced-efficiency fuel cell system is designed for utilities, large industrial users, data centers and other customers focused on clean and affordable power driven by the benefits and economics of high system electrical efficiency. Output: 3.7 megawatts"@en .


###  http://purl.org/holy/ns#Suriname
holy:Suriname rdf:type owl:NamedIndividual ,
                       schema:Country ;
              dbo:continent holy:South_America ;
              rdfs:label "Suriname"@en .


###  http://purl.org/holy/ns#Sweden
holy:Sweden rdf:type owl:NamedIndividual ,
                     schema:Country ;
            dbo:continent holy:Europe ;
            rdfs:label "Sweden"@en .


###  http://purl.org/holy/ns#Switzerland
holy:Switzerland rdf:type owl:NamedIndividual ,
                          schema:Country ;
                 dbo:continent holy:Europe ;
                 rdfs:label "Switzerland"@en .


###  http://purl.org/holy/ns#Syria
holy:Syria rdf:type owl:NamedIndividual ,
                    schema:Country ;
           dbo:continent holy:Asia ;
           rdfs:label "Syria"@en .


###  http://purl.org/holy/ns#Tajikistan
holy:Tajikistan rdf:type owl:NamedIndividual ,
                         schema:Country ;
                dbo:continent holy:Asia ;
                rdfs:label "Tajikistan"@en .


###  http://purl.org/holy/ns#Tanzania
holy:Tanzania rdf:type owl:NamedIndividual ,
                       schema:Country ;
              dbo:continent holy:Africa ;
              rdfs:label "Tanzania"@en .


###  http://purl.org/holy/ns#Thailand
holy:Thailand rdf:type owl:NamedIndividual ,
                       schema:Country ;
              dbo:continent holy:Asia ;
              rdfs:label "Thailand"@en .


###  http://purl.org/holy/ns#The_Bahamas
holy:The_Bahamas rdf:type owl:NamedIndividual ,
                          schema:Country ;
                 dbo:continent holy:North_America ;
                 rdfs:label "The Bahamas"@en .


###  http://purl.org/holy/ns#The_Gambia
holy:The_Gambia rdf:type owl:NamedIndividual ,
                         schema:Country ;
                dbo:continent holy:Africa ;
                rdfs:label "The Gambia"@en .


###  http://purl.org/holy/ns#Tiger_Cub_Economies
holy:Tiger_Cub_Economies rdf:type owl:NamedIndividual ,
                                  schema:Country ;
                         dbo:continent holy:Asia ;
                         rdfs:label "Tiger Cub Economies"@en .


###  http://purl.org/holy/ns#Togo
holy:Togo rdf:type owl:NamedIndividual ,
                   schema:Country ;
          dbo:continent holy:Africa ;
          rdfs:label "Togo"@en .


###  http://purl.org/holy/ns#Tonga
holy:Tonga rdf:type owl:NamedIndividual ,
                    schema:Country ;
           dbo:continent holy:Oceania ;
           rdfs:label "Tonga"@en .


###  http://purl.org/holy/ns#Trinidad_and_Tobago
holy:Trinidad_and_Tobago rdf:type owl:NamedIndividual ,
                                  schema:Country ;
                         dbo:continent holy:North_America ;
                         rdfs:label "Trinidad and Tobago"@en .


###  http://purl.org/holy/ns#Tunisia
holy:Tunisia rdf:type owl:NamedIndividual ,
                      schema:Country ;
             dbo:continent holy:Africa ;
             rdfs:label "Tunisia"@en .


###  http://purl.org/holy/ns#Turkey
holy:Turkey rdf:type owl:NamedIndividual ,
                     schema:Country ;
            dbo:continent holy:Europe ;
            rdfs:label "Turkey"@en .


###  http://purl.org/holy/ns#Turkmenistan
holy:Turkmenistan rdf:type owl:NamedIndividual ,
                           schema:Country ;
                  dbo:continent holy:Asia ;
                  rdfs:label "Turkmenistan"@en .


###  http://purl.org/holy/ns#TurretTruck
holy:TurretTruck rdf:type owl:NamedIndividual ,
                          holy:MaterialHandlingVehicle ;
                 rdfs:label "Turret Truck"@en .


###  http://purl.org/holy/ns#Tuvalu
holy:Tuvalu rdf:type owl:NamedIndividual ,
                     schema:Country ;
            dbo:continent holy:Oceania ;
            rdfs:label "Tuvalu"@en .


###  http://purl.org/holy/ns#Uganda
holy:Uganda rdf:type owl:NamedIndividual ,
                     schema:Country ;
            dbo:continent holy:Africa ;
            rdfs:label "Uganda"@en .


###  http://purl.org/holy/ns#Ukraine
holy:Ukraine rdf:type owl:NamedIndividual ,
                      schema:Country ;
             dbo:continent holy:Europe ;
             rdfs:label "Ukraine"@en .


###  http://purl.org/holy/ns#United_Arab_Emirates
holy:United_Arab_Emirates rdf:type owl:NamedIndividual ,
                                   schema:Country ;
                          dbo:continent holy:Asia ;
                          rdfs:label "United Arab Emirates"@en .


###  http://purl.org/holy/ns#United_Kingdom
holy:United_Kingdom rdf:type owl:NamedIndividual ,
                             schema:Country ;
                    dbo:continent holy:Europe ;
                    rdfs:label "United Kingdom"@en .


###  http://purl.org/holy/ns#United_States
holy:United_States rdf:type owl:NamedIndividual ,
                            schema:Country ;
                   dbo:continent holy:North_America ;
                   rdfs:label "United States"@en .


###  http://purl.org/holy/ns#Uruguay
holy:Uruguay rdf:type owl:NamedIndividual ,
                      schema:Country ;
             dbo:continent holy:South_America ;
             rdfs:label "Uruguay"@en .


###  http://purl.org/holy/ns#Uzbekistan
holy:Uzbekistan rdf:type owl:NamedIndividual ,
                         schema:Country ;
                dbo:continent holy:Asia ;
                rdfs:label "Uzbekistan"@en .


###  http://purl.org/holy/ns#Vanuatu
holy:Vanuatu rdf:type owl:NamedIndividual ,
                      schema:Country ;
             dbo:continent holy:Oceania ;
             rdfs:label "Vanuatu"@en .


###  http://purl.org/holy/ns#Vatican_City
holy:Vatican_City rdf:type owl:NamedIndividual ,
                           schema:Country ;
                  dbo:continent holy:Europe ;
                  rdfs:label "Vatican City"@en .


###  http://purl.org/holy/ns#Venezuela
holy:Venezuela rdf:type owl:NamedIndividual ,
                        schema:Country ;
               dbo:continent holy:South_America ;
               rdfs:label "Venezuela"@en .


###  http://purl.org/holy/ns#Vietnam
holy:Vietnam rdf:type owl:NamedIndividual ,
                      schema:Country ;
             dbo:continent holy:Asia ;
             rdfs:label "Vietnam"@en .


###  http://purl.org/holy/ns#Western_Sahara
holy:Western_Sahara rdf:type owl:NamedIndividual ,
                             schema:Country ;
                    dbo:continent holy:Africa ;
                    rdfs:label "Western Sahara"@en .


###  http://purl.org/holy/ns#Yemen
holy:Yemen rdf:type owl:NamedIndividual ,
                    schema:Country ;
           dbo:continent holy:Asia ;
           rdfs:label "Yemen"@en .


###  http://purl.org/holy/ns#ZEROe
holy:ZEROe rdf:type owl:NamedIndividual ,
                    holy:ProductDevelopmentProject ;
           holy:relatesToApplication holy:ZEROeBlendedWingBody ,
                                     holy:ZEROeTurbofan ,
                                     holy:ZEROeTurboprop ;
           m4i:projectParticipant dbr:Airbus ;
           m4i:endOfProject "2035"@en ;
           m4i:startOfProject "2020"@en ;
           dct:references <https://www.airbus.com/en/innovation/zero-emission/hydrogen/zeroe> ;
           rdfs:label "ZEROe"@en ;
           skos:definition """An project from Airbus to develop the world's first zero-emission commercial aircraft by 2035. It is based on hydrogen propulsion. Airbus is working on three aircraft prototypes.

All three ZEROe concepts are hybrid-hydrogen aircraft. They are powered by hydrogen combustion through modified gas turbine engines. Liquid hydrogen is used as fuel for combustion with oxygen.

In addition, hydrogen fuel cells create electrical power that complements the gas turbine, resulting in a highly efficient hybrid-electric propulsion system. All of these technologies are complementary, and the benefits are additive.

In 2022, we launched our ZEROe demonstrator with the aim to test hydrogen combustion technology on an A380 multimodal platform. A mature technology readiness level for a hydrogen-combustion propulsion system is expected to be achieved by 2025."""@en .


###  http://purl.org/holy/ns#ZEROeBlendedWingBody
holy:ZEROeBlendedWingBody rdf:type owl:NamedIndividual ,
                                   holy:Aircraft ;
                          holy:relatesToApplication holy:ZEROe ;
                          holy:usesProduct dbr:Hydrogen_Tank ,
                                           dbr:Hydrogen_engine ;
                          dct:references <https://www.airbus.com/en/innovation/zero-emission/hydrogen/zeroe> ;
                          rdfs:label "ZEROe Blended-Wing Body"@en ;
                          skos:definition """Concept passenger aircraft. The exceptionally wide interior opens up multiple options for hydrogen storage and distribution. Here, the liquid hydrogen storage tanks are stored underneath the wings. Two hybrid-hydrogen turbofan engines provide thrust.

Range: 2000nm
Passengers: <200"""@en .


###  http://purl.org/holy/ns#ZEROeTurbofan
holy:ZEROeTurbofan rdf:type owl:NamedIndividual ,
                            holy:Aircraft ;
                   holy:relatesToApplication holy:ZEROe ;
                   dct:references <https://www.airbus.com/en/innovation/zero-emission/hydrogen/zeroe> ;
                   rdfs:label "ZEROe Turbofan"@en ;
                   skos:definition """Passenger Aircraft running on two hybrid-hydrogen turbofan engines providing thrust. The liquid hydrogen storage and distribution system is located behind the rear pressure bulkhead.

Range: +1000 nm
Passengers: <100"""@en .


###  http://purl.org/holy/ns#ZEROeTurboprop
holy:ZEROeTurboprop rdf:type owl:NamedIndividual ,
                             holy:Aircraft ;
                    holy:relatesToApplication holy:ZEROe ;
                    dct:references <https://www.airbus.com/en/innovation/zero-emission/hydrogen/zeroe> ;
                    rdfs:label "ZEROe Turboprop"@en ;
                    skos:definition """Passenger aircraft with two hybrid-hydrogen turboprop engines, which drive eight-bladed propellers, providing thrust. The liquid hydrogen storage and distribution system is located behind the rear pressure bulkhead.

Range: 2000 nm
Passengers: <200"""@en .


###  http://purl.org/holy/ns#Zambia
holy:Zambia rdf:type owl:NamedIndividual ,
                     schema:Country ;
            dbo:continent holy:Africa ;
            rdfs:label "Zambia"@en .


###  http://purl.org/holy/ns#Zimbabwe
holy:Zimbabwe rdf:type owl:NamedIndividual ,
                       schema:Country ;
              dbo:continent holy:Africa ;
              rdfs:label "Zimbabwe"@en .


###  http://purl.org/holy/ns#Georgia_(country)
<http://purl.org/holy/ns#Georgia_(country)> rdf:type owl:NamedIndividual ,
                                                     schema:Country ;
                                            dbo:continent holy:Europe ;
                                            rdfs:label "Georgia"@en .


###  http://purl.org/holy/ns#TheHydrogenUtilization&GreenEnergyProject
<http://purl.org/holy/ns#TheHydrogenUtilization&GreenEnergyProject> rdf:type owl:NamedIndividual ,
                                                                             holy:PurposeBasedProject ;
                                                                    dct:references <https://newenergy.is/en/portfolio/huge/> ;
                                                                    rdfs:label "The Hydrogen Utilization & Green Energy project"@en ;
                                                                    skos:altLabel "HUGE"@en ;
                                                                    skos:definition "The Hydrogen Utilization & Green Energy (HUGE) project is a 1.4 million 3 year project, which started on the 1st of June 2019. The project is funded by the Northern Periphery and Arctic (NPA) Programme, under priority Axis 3 – Energy Efficiency & Renewable Energy. HUGE ambition is to raise awareness of the use of green hydrogen as a viable energy vector for remote and rural communities in housing, transport, and industry. For further details, má finna á vefsíðu þess."@en .


###  Generated by the OWL API (version 4.5.25.2023-02-15T19:15:49Z) https://github.com/owlcs/owlapi
